language_formalisation/syntax/syntax.v
@@ -1,6 +1,7 @@
-Require Export Bool ZArith Int String.
+Require Export Bool ZArith String.
 
-(* Variable Type Definitions *)
+(* ==================== Variable Type Definitions ==================== *)
+
 Definition var_name := string.
 Definition var_n := nat.
 Definition var_id := prod var_name var_n.
@@ -10,7 +11,8 @@ Notation "x == y" := (string_dec x y) (at level 75, no associativity).
 
 Definition int := Z.t.
 
-(* Syntax Definitions *)
+(* ==================== Syntax Definitions ==================== *)
+
 Inductive val : Type :=
 | Var : var_id -> val
 | Unit : val
@@ -60,20 +62,19 @@ with tctx : Type :=
 | TCtxØ : tctx
 | TCtxU : tctx -> vtype -> tctx
 
-with tmpl : Type :=
-| TApp : var_id -> val -> tmpl
-| TAbsurd : val -> tmpl
-| TΠMatch : val -> var_name -> var_name -> tmpl -> tmpl
-| TΣMatch : val -> var_name -> tmpl -> var_name -> tmpl -> tmpl
-| TOp : op_id -> val -> var_name -> tmpl -> tmpl
+with t : Type :=
+| TApp : var_id -> val -> t
+| TAbsurd : val -> t
+| TΠMatch : val -> var_name -> var_name -> t -> t
+| TΣMatch : val -> var_name -> t -> var_name -> t -> t
+| TOp : op_id -> val -> var_name -> t -> t
 
 with eqs : Type := 
 | EqsØ : eqs
-| EqsU : eqs -> ctx -> tctx -> tmpl -> tmpl -> eqs
+| EqsU : eqs -> ctx -> tctx -> t -> t -> eqs
 .
 
-
-(* Auxiliary Function Definitions *)
+(* ==================== Getters and Ctx Modification ==================== *)
 
 Fixpoint get_vtype Γ i :=
   match Γ, i with
@@ -81,6 +82,7 @@ Fixpoint get_vtype Γ i :=
   | CtxU Γ' A, 0 => Some A
   | CtxU Γ' A, S i' =>  get_vtype Γ' i'
   end.
+
 
 Fixpoint get_ttype Z i :=
   match Z, i with
@@ -94,123 +96,39 @@ Fixpoint get_op_type Σ op :=
   match Σ with
   | SigØ => None
   | SigU Σ' op' A B =>
-      if op == op' then Some (A, B)
-      else get_op_type Σ' op
+      if op == op' then Some (A, B) else get_op_type Σ' op
   end.
 
 
-Fixpoint find_op_case h op : option (var_name * var_name * comp) :=
+Fixpoint find_case h op : option (var_name * var_name * comp) :=
   match h with
   | CasesØ => None
-  | CasesU h_others op' x_op k_op c_op =>
-      if op == op' then Some (x_op, k_op, c_op)
-      else find_op_case h_others op
+  | CasesU h' op' x_op k_op c_op =>
+      if op == op' then Some (x_op, k_op, c_op) else find_case h' op
   end.
 
 
-Fixpoint eqs_contain_eq E Γ Z T1 T2 :=
+Fixpoint has_eq E Γ Z T1 T2 :=
   match E with
   | EqsØ => False
   | EqsU E' Γ' Z' T1' T2' =>
-      (Γ = Γ' /\ Z = Z' /\ T1 = T1' /\ T2 = T2') \/ eqs_contain_eq E' Γ Z T1 T2
+      (Γ = Γ' /\ Z = Z' /\ T1 = T1' /\ T2 = T2') \/ has_eq E' Γ Z T1 T2
   end.
 
 
-Fixpoint v_no_var (v:val) (j:nat) :=
-match v with
-| Var (name, num) => not (j = num)
-| Unit => True
-| Int j => True
-| Inl v' => v_no_var v' j
-| Inr v' => v_no_var v' j
-| Pair v1 v2 => (v_no_var v1 j) /\ (v_no_var v2 j)
-| Fun x c => c_no_var c (1+j)
-| Handler x c_ret h => (c_no_var c_ret (1+j)) /\ (h_no_var h j)
-end
-with c_no_var (c:comp) (j:nat) :=
-match c with
-| Ret v => v_no_var v j
-| Absurd v => v_no_var v j 
-| ΠMatch v x y c => (v_no_var v j) /\ c_no_var c (2+j)
-| ΣMatch v xl cl xr cr =>
-    (v_no_var v j) /\ (c_no_var cl (1+j)) /\ (c_no_var cr (1+j))
-| App v1 v2 => (v_no_var v1 j) /\ (v_no_var v2 j)
-| Op op v_arg y c => (v_no_var v_arg j) /\ (c_no_var c (1+j))
-| LetRec f x c1 c2 => (c_no_var c1 (2+j)) /\ (c_no_var c2 (1+j))
-| DoBind x c1 c2 => (c_no_var c1 j) /\ (c_no_var c2 (1+j))
-| Handle v c' => (v_no_var v j) /\ (c_no_var c' j)
-end
-with h_no_var (h:hcases) (j:nat) :=
-match h with
-| CasesØ => True
-| CasesU h op x k c => (h_no_var h j) /\ (c_no_var c (2+j))
-end.
-
-Fixpoint v_under_var (v:val) (j:nat) :=
-match v with
-| Var (name, num) => num < j
-| Unit => True
-| Int j => True
-| Inl v' => v_under_var v' j
-| Inr v' => v_under_var v' j
-| Pair v1 v2 => (v_under_var v1 j) /\ (v_under_var v2 j)
-| Fun x c => c_under_var c (1+j)
-| Handler x c_ret h => (c_under_var c_ret (1+j)) /\ (h_under_var h j)
-end
-with c_under_var (c:comp) (j:nat) :=
-match c with
-| Ret v => v_under_var v j
-| Absurd v => v_under_var v j 
-| ΠMatch v x y c => (v_under_var v j) /\ c_under_var c (2+j)
-| ΣMatch v xl cl xr cr =>
-    (v_under_var v j) /\ (c_under_var cl (1+j)) /\ (c_under_var cr (1+j))
-| App v1 v2 => (v_under_var v1 j) /\ (v_under_var v2 j)
-| Op op v_arg y c => (v_under_var v_arg j) /\ (c_under_var c (1+j))
-| LetRec f x c1 c2 => (c_under_var c1 (2+j)) /\ (c_under_var c2 (1+j))
-| DoBind x c1 c2 => (c_under_var c1 j) /\ (c_under_var c2 (1+j))
-| Handle v c' => (v_under_var v j) /\ (c_under_var c' j)
-end
-with h_under_var (h:hcases) (j:nat) :=
-match h with
-| CasesØ => True
-| CasesU h op x k c => (h_under_var h j) /\ (c_under_var c (2+j))
-end.
-
-Fixpoint tmpl_under_var (T:tmpl) (j:nat) :=
-match T with
-| TApp (name, num) v => v_under_var v j
-| TAbsurd v => v_under_var v j
-| TΠMatch v x y T => v_under_var v j /\ tmpl_under_var T (2+j)
-| TΣMatch v xl Tl xr Tr =>
-    (v_under_var v j) /\ (tmpl_under_var Tl (1+j)) 
-    /\ (tmpl_under_var Tr (1+j))
-| TOp op v_arg y T => (v_under_var v_arg j) /\ (tmpl_under_var T (1+j))
-end.
-
-Fixpoint tmpl_under_tvar_j (T:tmpl) (j:nat) :=
-match T with
-| TApp (name, num) v => num < j
-| TAbsurd v => True
-| TΠMatch v x y T => tmpl_under_tvar_j T j
-| TΣMatch v xl Tl xr Tr => 
-    (tmpl_under_tvar_j Tl j) /\ (tmpl_under_tvar_j Tr j)
-| TOp op v_arg y T => (tmpl_under_tvar_j T j)
-end.
-
-
-Fixpoint ctx_remove_var (Γ:ctx) (i:nat) :=
+Fixpoint ctx_remove (Γ:ctx) (i:nat) :=
   match Γ, i with
   | CtxØ, _ => CtxØ
   | CtxU Γ' A', 0 => Γ'
-  | CtxU Γ' A', S i' => CtxU (ctx_remove_var Γ' i') A'
+  | CtxU Γ' A', S i' => CtxU (ctx_remove Γ' i') A'
   end.
 
 
-Fixpoint ctx_insert_var (Γ:ctx) A (i:nat) :=
+Fixpoint ctx_insert (Γ:ctx) A (i:nat) :=
   match Γ, i with
   | Γ', 0 => CtxU Γ' A
   | CtxØ, _ => CtxØ
-  | CtxU Γ' A', S i' => CtxU (ctx_insert_var Γ' A i') A'
+  | CtxU Γ' A', S i' => CtxU (ctx_insert Γ' A i') A'
   end.
 
 
@@ -239,4 +157,94 @@ Fixpoint join_ctx_tctx Γ Z D :=
   match Z with
   | TCtxØ => Γ
   | TCtxU Z A => CtxU (join_ctx_tctx Γ Z D) (TyFun A D)
+  end.
+
+(* ==================== Term Properties ==================== *)
+
+Fixpoint v_no_var (v:val) (j:nat) :=
+  match v with
+  | Var (name, num) => not (j = num)
+  | Unit => True
+  | Int j => True
+  | Inl v' => v_no_var v' j
+  | Inr v' => v_no_var v' j
+  | Pair v1 v2 => (v_no_var v1 j) /\ (v_no_var v2 j)
+  | Fun x c => c_no_var c (1+j)
+  | Handler x c_ret h => (c_no_var c_ret (1+j)) /\ (h_no_var h j)
+  end
+
+with c_no_var (c:comp) (j:nat) :=
+  match c with
+  | Ret v => v_no_var v j
+  | Absurd v => v_no_var v j 
+  | ΠMatch v x y c => (v_no_var v j) /\ c_no_var c (2+j)
+  | ΣMatch v xl cl xr cr =>
+      (v_no_var v j) /\ (c_no_var cl (1+j)) /\ (c_no_var cr (1+j))
+  | App v1 v2 => (v_no_var v1 j) /\ (v_no_var v2 j)
+  | Op op v_arg y c => (v_no_var v_arg j) /\ (c_no_var c (1+j))
+  | LetRec f x c1 c2 => (c_no_var c1 (2+j)) /\ (c_no_var c2 (1+j))
+  | DoBind x c1 c2 => (c_no_var c1 j) /\ (c_no_var c2 (1+j))
+  | Handle v c' => (v_no_var v j) /\ (c_no_var c' j)
+  end
+
+with h_no_var (h:hcases) (j:nat) :=
+  match h with
+  | CasesØ => True
+  | CasesU h op x k c => (h_no_var h j) /\ (c_no_var c (2+j))
+  end.
+
+
+Fixpoint v_under_var (v:val) (j:nat) :=
+  match v with
+  | Var (name, num) => num < j
+  | Unit => True
+  | Int j => True
+  | Inl v' => v_under_var v' j
+  | Inr v' => v_under_var v' j
+  | Pair v1 v2 => (v_under_var v1 j) /\ (v_under_var v2 j)
+  | Fun x c => c_under_var c (1+j)
+  | Handler x c_ret h => (c_under_var c_ret (1+j)) /\ (h_under_var h j)
+  end
+
+with c_under_var (c:comp) (j:nat) :=
+  match c with
+  | Ret v => v_under_var v j
+  | Absurd v => v_under_var v j 
+  | ΠMatch v x y c => (v_under_var v j) /\ c_under_var c (2+j)
+  | ΣMatch v xl cl xr cr =>
+      (v_under_var v j) /\ (c_under_var cl (1+j)) /\ (c_under_var cr (1+j))
+  | App v1 v2 => (v_under_var v1 j) /\ (v_under_var v2 j)
+  | Op op v_arg y c => (v_under_var v_arg j) /\ (c_under_var c (1+j))
+  | LetRec f x c1 c2 => (c_under_var c1 (2+j)) /\ (c_under_var c2 (1+j))
+  | DoBind x c1 c2 => (c_under_var c1 j) /\ (c_under_var c2 (1+j))
+  | Handle v c' => (v_under_var v j) /\ (c_under_var c' j)
+  end
+
+with h_under_var h j :=
+  match h with
+  | CasesØ => True
+  | CasesU h op x k c => (h_under_var h j) /\ (c_under_var c (2+j))
+  end.
+
+
+Fixpoint t_under_var T j :=
+  match T with
+  | TApp (name, num) v => v_under_var v j
+  | TAbsurd v => v_under_var v j
+  | TΠMatch v x y T => v_under_var v j /\ t_under_var T (2+j)
+  | TΣMatch v xl Tl xr Tr =>
+      (v_under_var v j) /\ (t_under_var Tl (1+j)) 
+      /\ (t_under_var Tr (1+j))
+  | TOp op v_arg y T => (v_under_var v_arg j) /\ (t_under_var T (1+j))
+  end.
+
+
+Fixpoint t_under_tvar T j :=
+  match T with
+  | TApp (name, num) v => num < j
+  | TAbsurd v => True
+  | TΠMatch v x y T => t_under_tvar T j
+  | TΣMatch v xl Tl xr Tr => 
+      (t_under_tvar Tl j) /\ (t_under_tvar Tr j)
+  | TOp op v_arg y T => (t_under_tvar T j)
   end.
