language_formalisation/substitution/substitution_lemmas.v
@@ -1,262 +1,118 @@
-(* Add LoadPath "C:\Users\Ziga\Documents\Ziga_podatki\PHD\language_formalisation\substitution". *)
-(* Add LoadPath "C:\Users\Ziga\Documents\Ziga_podatki\PHD\language_formalisation\syntax". *)
-Add LoadPath "E:\Ziga_Podatki\faks\PHD\language_formalisation\substitution".
-Add LoadPath "E:\Ziga_Podatki\faks\PHD\language_formalisation\syntax".
+Add LoadPath "C:\Users\Ziga\Documents\Ziga_podatki\PHD\language_formalisation\substitution".
+Add LoadPath "C:\Users\Ziga\Documents\Ziga_podatki\PHD\language_formalisation\syntax".
+(* Add LoadPath "E:\Ziga_Podatki\faks\PHD\language_formalisation\substitution". *)
+(* Add LoadPath "E:\Ziga_Podatki\faks\PHD\language_formalisation\syntax". *)
 Require Export substitution syntax_lemmas.
-Require Import Arith Le.
+Require Import Le.
+
+(* ==================== Effects on getters ==================== *)
+
+Lemma shift_find_None h o i j :
+  find_case h o = None <-> find_case (Sub.h_shift h i j) o = None.
+Proof.
+constructor; intro; induction h; auto; simpl in *;
+destruct (o==o0) eqn:cmp; try discriminate; auto.
+Qed.
 
 
-Lemma v_shift_shift n m cut (v:val) :
+Lemma negshift_find_None h o i j :
+  find_case h o = None <-> find_case (Sub.h_negshift h i j) o = None.
+Proof.
+constructor; intro; induction h; auto; simpl in *;
+destruct (o==o0) eqn:cmp; try discriminate; auto.
+Qed.
+
+
+Lemma sub_find_None h o i v_s :
+  find_case h o = None -> 
+  find_case (Sub.h_sub h (i, v_s)) o = None.
+Proof.
+intro; induction h; simpl in *. auto.
+destruct (o==o0) eqn:cmp. discriminate. auto.
+Qed.
+
+
+Lemma shift_find_Some h o i j x k c :
+  find_case h o = Some (x, k, c) -> 
+  find_case (Sub.h_shift h i j) o = Some (x, k, (Sub.c_shift c i (2+j))).
+Proof.
+intro; induction h; simpl in *. discriminate.
+destruct (o==o0) eqn:cmp. inv H. all: auto.
+Qed.
+
+
+Lemma negshift_find_Some h o i j x k c :
+  find_case h o = Some (x, k, c) -> 
+  find_case (Sub.h_negshift h i j) o = Some (x, k, (Sub.c_negshift c i (2+j))).
+Proof.
+intro; induction h; simpl in *. discriminate.
+destruct (o==o0) eqn:cmp. inv H. all: auto.
+Qed.
+
+
+Lemma sub_find_Some h o i v_s x k c :
+  find_case h o = Some (x, k, c) -> 
+    find_case (Sub.h_sub h (i, v_s)) o 
+  = Some (x, k, (Sub.c_sub c (2+i, Sub.v_shift v_s 2 0))).
+Proof.
+intro; induction h; simpl in *. discriminate.
+destruct (o==o0) eqn:cmp. inv H. all: auto.
+Qed.
+
+(* ==================== Shift and Sub interactions ==================== *)
+
+Lemma v_shift_0 cut v : Sub.v_shift v 0 cut = v
+with c_shift_0 cut c  : Sub.c_shift c 0 cut = c
+with h_shift_0 cut h  : Sub.h_shift h 0 cut = h.
+Proof.
+{ revert cut. induction v; intros cut; simpl; try f_equal; auto.
+  destruct v. destruct (cut <=? v0); auto. }
+{ revert cut. induction c; intros cut; simpl; f_equal; auto. }
+{ revert cut. induction h; intros cut; simpl; f_equal; auto. }
+Qed.
+
+
+Lemma v_shift_shift n m cut v :
   Sub.v_shift (Sub.v_shift v n cut) m cut = (Sub.v_shift v (n + m) cut)
-
-with c_shift_shift n m cut (c:comp) :
+with c_shift_shift n m cut c :
   Sub.c_shift (Sub.c_shift c n cut) m cut = (Sub.c_shift c (n + m) cut)
-
-with h_shift_shift n m cut (h:hcases) :
+with h_shift_shift n m cut h :
   Sub.h_shift (Sub.h_shift h n cut) m cut = (Sub.h_shift h (n + m) cut).
 Proof.
 {
-clear v_shift_shift.
-revert cut. induction v; intros cut; simpl; f_equal.
-{ (* The only relevant case. *)
-  destruct v as (name, db_i).
-  destruct (cut <=? db_i) eqn:cmp; simpl.
-  - apply (leb_complete _ _) in cmp.
-    assert (cut <= n + db_i) by omega.
-    apply leb_correct in H. rewrite H.
-    f_equal. f_equal. omega.
-  - rewrite cmp. reflexivity. }
-all : try reflexivity || apply IHv || apply IHv1 || apply IHv2.
-all : try apply c_shift_shift || apply h_shift_shift; assumption.
-}{
-clear c_shift_shift.
-revert cut. induction c; intros cut; try destruct p; simpl; f_equal;
-try apply v_shift_shift || apply IHc || apply IHc1 || apply IHc2.
-}{
-clear h_shift_shift.
-revert cut. induction h; intros cut; simpl; f_equal.
-reflexivity. apply IHh. apply c_shift_shift.
-}
+revert cut. induction v; intros cut; simpl; f_equal; auto.
+destruct v as (name, db_i).
+destruct (cut <=? db_i) eqn:cmp; simpl.
+- apply (leb_complete _ _) in cmp.
+  assert (cut <=? n + db_i = true) by (apply leb_correct; omega).
+  rewrite H. do 2 f_equal. omega.
+- rewrite cmp. reflexivity. }
+{ revert cut. induction c; intros cut; try destruct p; simpl; f_equal; auto. }
+{ revert cut. induction h; intros cut; simpl; f_equal; auto. }
 Qed.
 
 
-(* Lemma v_shift_shift_alt n m cut (v:val) :
-  Sub.v_shift (Sub.v_shift v n cut) m (n+cut) = (Sub.v_shift v (n + m) cut)
+Lemma v_shift_comm n i j d (v:val) :
+  i >= j ->
+  Sub.v_shift (Sub.v_shift v n i) d j = Sub.v_shift (Sub.v_shift v d j) n (d+i)
 
-with c_shift_shift_alt n m cut (c:comp) :
-  Sub.c_shift (Sub.c_shift c n cut) m (n+cut) = (Sub.c_shift c (n + m) cut)
+with c_shift_comm n i j d (c:comp) :
+  i >= j ->
+  Sub.c_shift (Sub.c_shift c n i) d j = Sub.c_shift (Sub.c_shift c d j) n (d+i)
 
-with h_shift_shift_alt n m cut (h:hcases) :
-  Sub.h_shift (Sub.h_shift h n cut) m (n+cut) = (Sub.h_shift h (n + m) cut).
-Proof.
-{
-clear v_shift_shift_alt.
-revert cut. induction v; intros cut; simpl; f_equal.
-{ (* The only relevant case. *)
-  destruct v as (name, db_i).
-  destruct (cut <=? db_i) eqn:cmp; simpl.
-  - apply (leb_complete _ _) in cmp.
-    assert (n+cut <= n+db_i) by omega.
-    apply leb_correct in H. rewrite H.
-    f_equal. f_equal. omega.
-  - assert (n+cut <=? db_i = false).
-    { apply leb_correct_conv. apply leb_complete_conv in cmp. omega. }
-    rewrite H. reflexivity. }
-all : try reflexivity || apply IHv || apply IHv1 || apply IHv2.
-all : assert (S(n+cut)=n + S cut) by omega; try rewrite H.
-all : try apply c_shift_shift_alt || apply h_shift_shift_alt; assumption.
-}{
-clear c_shift_shift_alt.
-revert cut. induction c; intros cut; try destruct p; simpl; f_equal;
-try apply v_shift_shift_alt.
-all : assert (S(n+cut)=n + S cut) by omega; try rewrite H.
-all : assert (S(n+ S cut)=n + S (S cut)) by omega; try rewrite H0.
-all : try apply IHc || apply IHc1 || apply IHc2.
-}{
-clear h_shift_shift_alt.
-revert cut. induction h; intros cut; simpl; f_equal.
-reflexivity. apply IHh.
-assert (S(S(n+cut))=n+S(S cut)) by omega. rewrite H. 
-apply c_shift_shift_alt.
-}
-Qed. *)
-
-Lemma v_shift_makes_no_var v j:
-  v_no_var (Sub.v_shift v 1 j) j
-with c_shift_makes_no_var c j:
-  c_no_var (Sub.c_shift c 1 j) j
-with h_shift_makes_no_var h j:
-  h_no_var (Sub.h_shift h 1 j) j.
-Proof.
-{
-clear v_shift_makes_no_var.
-revert j; induction v; intros j; simpl; auto.
-destruct v as (name, num). simpl.
-destruct (j<=?num) eqn:cmp; simpl.
-+ apply leb_complete in cmp. omega.
-+ apply leb_iff_conv in cmp. omega.
-}{
-revert j; induction c; intros j; try destruct p; simpl; auto.
-}{
-revert j; induction h; intros j; simpl; auto.
-}
-Qed.
-
-
-Lemma v_no_var_shift (v:val) j n cut:
-  v_no_var v j -> (cut <= j) -> v_no_var (Sub.v_shift v n cut) (n+j)
-
-with c_no_var_shift (c:comp) j n cut:
-  c_no_var c j -> (cut <= j) -> c_no_var (Sub.c_shift c n cut) (n+j)
-  
-with h_no_var_shift (h:hcases) j n cut:
-  h_no_var h j -> (cut <= j) -> h_no_var (Sub.h_shift h n cut) (n+j).
-Proof.
-all: assert (forall j, S(n+j)=n+(S j)) as snj by (intro; omega).
-all: assert (forall j, S(S(n+j))=n+(S(S j))) as ssnj by (intro; omega).
-{
-clear v_no_var_shift.
-revert j. induction v; intros j orig_clean j_le_cut; simpl; simpl in orig_clean;
-try constructor; try inv orig_clean; auto.
-+ destruct v as (name, num). destruct (cut <=? num) eqn:cmp; simpl;
-  try rewrite leb_iff_conv in cmp; omega.
-+ rewrite snj. apply c_no_var_shift. assumption. omega. 
-+ rewrite snj. apply c_no_var_shift. assumption. omega.
-}{
-clear c_no_var_shift.
-revert j cut. induction c; intros j cut orig_clean j_le_cut; simpl; simpl in *.
-all: try inv orig_clean; try constructor; try constructor; auto.
-all: try rewrite ssnj; try rewrite snj.
-all: try apply IHc || apply IHc1 || apply IHc2; try omega; auto.
-all: inv H0; assumption.
-}{
-clear h_no_var_shift.
-revert j cut. induction h; intros j cut orig_clean j_le_cut; simpl;
-destruct orig_clean; auto. constructor. auto.
-rewrite ssnj. apply c_no_var_shift. assumption. omega.
-}
-Qed.
-
-
-Lemma v_no_var_subbed (v:val) j v_s :
-  v_no_var v_s j -> v_no_var (Sub.v_sub v (j, v_s)) j
-
-with c_no_var_subbed (c:comp) j v_s :
-  v_no_var v_s j -> c_no_var (Sub.c_sub c (j, v_s)) j
-
-with h_no_var_subbed (h:hcases) j v_s :
-  v_no_var v_s j -> h_no_var (Sub.h_sub h (j, v_s)) j.
-Proof.
-{
-clear v_no_var_subbed.
-revert j. induction v; intros j v_s_clean; try constructor.
-all: try (apply IHv; assumption); auto.
-- destruct v as (x, n). simpl.
-  induction (n =? j) eqn:fits.
-  + assumption.
-  + simpl. apply Nat.eqb_neq in fits. omega.
-- apply c_no_var_subbed. apply v_no_var_shift. assumption. omega.
-- apply c_no_var_subbed. apply v_no_var_shift. assumption. omega.
-}{
-clear c_no_var_subbed.
-revert j v_s. induction c; intros j v_s v_s_clean; simpl; try constructor;
-try destruct p; simpl; try constructor; auto;
-try apply IHc || apply IHc1 || apply IHc2;
-try (apply v_no_var_shift; assumption || omega).
-all:
-assert (v_no_var (Sub.v_shift v_s 1 0) (1 + j)) by
-  (apply v_no_var_shift; auto || omega).
-all: apply (v_no_var_shift _ _ 1 0) in H; try omega.
-all: rewrite v_shift_shift in H; simpl in H; assumption.
-}{
-clear h_no_var_subbed.
-revert j v_s. induction h; intros j v_s v_s_clean; simpl; auto.
-constructor. auto.
-assert (v_no_var (Sub.v_shift v_s 1 0) (1+j)).
-{ apply v_no_var_shift. auto. omega. }
-apply (v_no_var_shift _ _ 1 0) in H.
-rewrite (v_shift_shift _ _ _) in H. auto. omega.
-}
-Qed.
-
-
-Lemma h_shift_find_op_None h o i j :
-  find_op_case h o = None <-> find_op_case (Sub.h_shift h i j) o = None.
-Proof.
-constructor; intro; induction h; auto; simpl in *;
-destruct (o==o0) eqn:cmp; try discriminate; auto.
-Qed.
-
-Lemma h_negshift_find_op_None h o i j :
-  find_op_case h o = None <-> find_op_case (Sub.h_negshift h i j) o = None.
-Proof.
-constructor; intro; induction h; auto; simpl in *;
-destruct (o==o0) eqn:cmp; try discriminate; auto.
-Qed.
-
-Lemma h_shift_find_op_Some h o i j x k cop :
-  find_op_case h o = Some (x, k, cop) -> 
-  find_op_case (Sub.h_shift h i j) o = 
-    Some (x, k, (Sub.c_shift cop i (2+j))).
-Proof.
-intro; induction h.
-+ simpl in H. discriminate.
-+ simpl in *. destruct (o==o0) eqn:cmp. inv H. all: auto.
-Qed.
-
-Lemma h_negshift_find_op_Some h o i j x k cop :
-  find_op_case h o = Some (x, k, cop) -> 
-  find_op_case (Sub.h_negshift h i j) o = 
-    Some (x, k, (Sub.c_negshift cop i (2+j))).
-Proof.
-intro; induction h.
-+ simpl in H. discriminate.
-+ simpl in *. destruct (o==o0) eqn:cmp. inv H. all: auto.
-Qed.
-
-Lemma h_sub_find_op_None h o i v_s :
-  find_op_case h o = None -> 
-  find_op_case (Sub.h_sub h (i, v_s)) o = None.
-Proof.
-intro; induction h.
-+ simpl. reflexivity.
-+ simpl in *. destruct (o==o0) eqn:cmp. discriminate. auto.
-Qed.
-
-Lemma h_sub_find_op_Some h o i v_s x k cop :
-  find_op_case h o = Some (x, k, cop) -> 
-  find_op_case (Sub.h_sub h (i, v_s)) o = 
-    Some (x, k, (Sub.c_sub cop (2+i, Sub.v_shift v_s 2 0))).
-Proof.
-intro; induction h.
-+ simpl in H. discriminate.
-+ simpl in *. destruct (o==o0) eqn:cmp. inv H. all: auto.
-Qed.
-
-
-(* needed for tmpl handling *)
-Lemma v_shift_comm_aux n i j d (v:val) :
-i >= j ->
-Sub.v_shift (Sub.v_shift v n i) d j = Sub.v_shift (Sub.v_shift v d j) n (d+i)
-
-with c_shift_comm_aux n i j d (c:comp) :
-i >= j ->
-Sub.c_shift (Sub.c_shift c n i) d j = Sub.c_shift (Sub.c_shift c d j) n (d+i)
-
-with h_shift_comm_aux n i j d (h:hcases) :
-i >= j ->
-Sub.h_shift (Sub.h_shift h n i) d j = Sub.h_shift (Sub.h_shift h d j) n (d+i).
+with h_shift_comm n i j d (h:hcases) :
+  i >= j ->
+  Sub.h_shift (Sub.h_shift h n i) d j = Sub.h_shift (Sub.h_shift h d j) n (d+i).
 Proof.
 {
 intros cmp. induction v; simpl.
-{ 
-  clear v_shift_comm_aux c_shift_comm_aux h_shift_comm_aux.
+{ clear v_shift_comm c_shift_comm h_shift_comm.
   destruct v as (x, dbi).
   destruct (i<=?dbi) eqn:cmpi; destruct (j<=?dbi) eqn:cmpj; simpl.
   + apply leb_complete in cmpi. apply leb_complete in cmpj.
     assert (j<=?n+dbi=true) by (apply leb_correct; omega).
     assert (d+i<=?d+dbi=true) by (apply leb_correct; omega).
-    rewrite H, H0. f_equal. f_equal. omega.
+    rewrite H, H0. do 2 f_equal. omega.
   + apply leb_complete in cmpi. apply leb_complete_conv in cmpj. omega.
   + apply leb_complete_conv in cmpi. rewrite cmpj. apply leb_complete in cmpj.
     assert (d+i<=?d+dbi=false) by (apply leb_correct_conv; omega).  
@@ -266,53 +122,45 @@ intros cmp. induction v; simpl.
     assert (d+i<=?dbi=false) by (apply leb_correct_conv; omega).
     rewrite H.  reflexivity.
 }
-clear v_shift_comm_aux h_shift_comm_aux.
+clear v_shift_comm h_shift_comm.
 all: f_equal; auto.
 all: assert (S(d+i)=d+S i) by omega; rewrite H. 
-all: eapply c_shift_comm_aux; omega.
+all: eapply c_shift_comm; omega.
 }{
 intros cmp. induction c; simpl; f_equal; auto; 
-clear v_shift_comm_aux h_shift_comm_aux.
-try eapply c_shift_comm_aux; try omega.
-all: assert (S(S(d+i))=d+S(S i)) by omega; try (rewrite H;
-  eapply c_shift_comm_aux; omega).
-all: assert (S(d+i)=d+S i) by omega; try rewrite H0;
-  eapply c_shift_comm_aux; omega.
+clear v_shift_comm h_shift_comm.
+all: assert (S(S(d+i))=d+S(S i)) by omega; 
+  try (rewrite H; eapply c_shift_comm; omega).
+all: assert (S(d+i)=d+S i) by omega; rewrite H0; eapply c_shift_comm; omega.
 }{
-clear v_shift_comm_aux h_shift_comm_aux.
+clear v_shift_comm h_shift_comm.
 intros cmp. induction h; simpl.
 all: f_equal; auto.
-assert (S(S(d+i))=d+S(S i)) by omega;
-rewrite H; eapply c_shift_comm_aux; omega.
+assert (S(S(d+i))=d+S(S i)) by omega; rewrite H; eapply c_shift_comm; omega.
 }
 Qed.
 
 
-Lemma v_negshift_shift (n:nat) (m:nat) (cut:nat) (v:val) :
+Lemma v_negshift_shift n m cut (v:val) :
   (m <= n) ->
   Sub.v_negshift (Sub.v_shift v n cut) m cut = (Sub.v_shift v (n - m) cut)
 
-with c_negshift_shift (n:nat) (m:nat) (cut:nat) (c:comp) :
+with c_negshift_shift n m cut (c:comp) :
   (m <= n) ->
   Sub.c_negshift (Sub.c_shift c n cut) m cut = (Sub.c_shift c (n - m) cut)
 
-with h_negshift_shift (n:nat) (m:nat) (cut:nat) (h:hcases) :
+with h_negshift_shift n m cut (h:hcases) :
   (m <= n) ->  
   Sub.h_negshift (Sub.h_shift h n cut) m cut = (Sub.h_shift h (n - m) cut).
 Proof.
 {
-clear v_negshift_shift.  
-revert cut. induction v; intros cut m_le_n; simpl; f_equal.
-{ (* The only relevant case. *)
-  destruct v as (name, db_i). simpl.
-  induction (cut <=? db_i) eqn:cmp; simpl.
-  - apply (leb_complete _ _) in cmp.
-    assert (cut <= n + db_i) by omega.
-    apply (leb_correct _ _) in H. rewrite H.
-    f_equal. f_equal. omega.
-  - rewrite cmp. reflexivity. }
-all : try reflexivity || apply IHv || apply IHv1 || apply IHv2.
-all : try apply c_negshift_shift || apply h_negshift_shift; assumption.
+clear v_negshift_shift.
+revert cut. induction v; intros cut m_le_n; simpl; f_equal; auto.
+destruct v as (x, i). simpl. destruct (cut <=? i) eqn:cmp; simpl.
+- apply leb_complete in cmp.
+  assert (cut <=? n + i=true) by (apply leb_correct; omega).
+  rewrite H. do 2 f_equal. omega.
+- rewrite cmp. reflexivity.
 }{
 clear c_negshift_shift h_negshift_shift.
 revert cut. induction c; intros cut m_le_n; simpl; f_equal;
@@ -324,147 +172,318 @@ reflexivity. apply IHh. assumption. apply c_negshift_shift. assumption.
 }
 Qed.
 
-Lemma v_shift_negshift_1j v n i j :
-v_no_var v j -> i <= j ->
-  Sub.v_shift (Sub.v_negshift v 1 j) n i 
-= Sub.v_negshift (Sub.v_shift v n i) 1 (n+j) 
-with c_shift_negshift_1j c n i j :
-c_no_var c j -> i <= j ->
-  Sub.c_shift (Sub.c_negshift c 1 j) n i 
-= Sub.c_negshift (Sub.c_shift c n i) 1 (n+j) 
-with h_shift_negshift_1j h n i j :
-h_no_var h j -> i <= j ->
-  Sub.h_shift (Sub.h_negshift h 1 j) n i 
-= Sub.h_negshift (Sub.h_shift h n i) 1 (n+j).
+
+Lemma v_shift_negshift_comm v n i j :
+  v_no_var v j -> i <= j ->
+    Sub.v_shift (Sub.v_negshift v 1 j) n i 
+  = Sub.v_negshift (Sub.v_shift v n i) 1 (n+j)
+
+with c_shift_negshift_comm c n i j :
+  c_no_var c j -> i <= j ->
+    Sub.c_shift (Sub.c_negshift c 1 j) n i 
+  = Sub.c_negshift (Sub.c_shift c n i) 1 (n+j)
+
+with h_shift_negshift_comm h n i j :
+  h_no_var h j -> i <= j ->
+    Sub.h_shift (Sub.h_negshift h 1 j) n i 
+  = Sub.h_negshift (Sub.h_shift h n i) 1 (n+j).
 Proof.
 {
-clear v_shift_negshift_1j.
+clear v_shift_negshift_comm.
 revert j; induction v; intros j novar cmpij; simpl.
 { 
-destruct v as (x, d). simpl.
-destruct (j<=?d) eqn:jd.
-+ apply leb_complete in jd. assert (i<=?d=true) by (apply leb_correct; omega).
-  rewrite H. simpl. assert (n+j<=?n+d=true).
-  { apply leb_correct; omega. }
+destruct v as (x, d). simpl. destruct (j<=?d) eqn:jd.
++ apply leb_complete in jd. 
+  assert (i<=?d=true) by (apply leb_correct; omega).
+  rewrite H. simpl. assert (n+j<=?n+d=true) by (apply leb_correct; omega).
   rewrite H0. assert (i<=?d-1=true).
   { apply leb_correct. simpl in novar. omega. }
   rewrite H1. do 2 f_equal. simpl in novar. omega.
 + apply leb_complete_conv in jd. simpl.
   destruct (i<=?d) eqn:id; simpl.
-  - assert (n+j<=?n+d=false).
-    { apply leb_correct_conv; omega. }
+  - assert (n+j<=?n+d=false) by (apply leb_correct_conv; omega).
     rewrite H. reflexivity.
-  - assert (n+j<=?d=false).
-    { apply leb_correct_conv; omega. }
+  - assert (n+j<=?d=false) by (apply leb_correct_conv; omega).
     rewrite H. reflexivity.
 }
-all : f_equal; try reflexivity || apply IHv || apply IHv1 || apply IHv2.
-all : simpl in novar; try destruct novar; auto.
+all : f_equal; simpl in novar; try destruct novar; auto.
 all : assert (S(n+j)=n+(S j)) as snj by omega; rewrite snj.
-all : apply c_shift_negshift_1j; omega || auto.
+all : apply c_shift_negshift_comm; omega || auto.
 }{
-clear h_shift_negshift_1j.
-revert j. destruct c; intros j novar cmpij; simpl in *; f_equal.
+clear h_shift_negshift_comm.
+revert j. destruct c; intros j novar cmpij; simpl in *; f_equal; auto.
 all : assert (S(S(n+j))=n+(S (S j))) as ssnj by omega; try rewrite ssnj.
 all : assert (S(n+j)=n+(S j)) as snj by omega; try rewrite snj.
-all: apply v_shift_negshift_1j || apply c_shift_negshift_1j.
+all: apply v_shift_negshift_comm || apply c_shift_negshift_comm.
 all: omega || (try destruct novar; auto).
 all: destruct H0; auto.
 }{
-clear h_shift_negshift_1j v_shift_negshift_1j.
+clear h_shift_negshift_comm v_shift_negshift_comm.
 revert j. induction h; intros j novar cmpij; simpl; f_equal. auto.
-+ apply IHh. inv novar. assumption. assumption.
++ inv novar; auto.
 + assert (S(S(n+j))=n+(S (S j))) as ssnj by omega; try rewrite ssnj.
-  apply c_shift_negshift_1j. inv novar. auto. omega.
+  apply c_shift_negshift_comm. inv novar. auto. omega.
+}
+Qed.
+
+(* ==================== novar interactions ==================== *)
+
+Lemma v_shift_makes_no_var v j:
+  v_no_var (Sub.v_shift v 1 j) j
+with c_shift_makes_no_var c j:
+  c_no_var (Sub.c_shift c 1 j) j
+with h_shift_makes_no_var h j:
+  h_no_var (Sub.h_shift h 1 j) j.
+Proof.
+{clear v_shift_makes_no_var.
+revert j; induction v; intros j; simpl; auto.
+destruct v as (name, num). simpl.
+destruct (j<=?num) eqn:cmp; simpl.
++ apply leb_complete in cmp. omega.
++ apply leb_iff_conv in cmp. omega. }
+{revert j; induction c; intros j; try destruct p; simpl; auto. }
+{revert j; induction h; intros j; simpl; auto. }
+Qed.
+
+
+Lemma v_no_var_shift (v:val) j n cut:
+  v_no_var v j -> (cut <= j) -> v_no_var (Sub.v_shift v n cut) (n+j)
+with c_no_var_shift (c:comp) j n cut:
+  c_no_var c j -> (cut <= j) -> c_no_var (Sub.c_shift c n cut) (n+j)
+with h_no_var_shift (h:hcases) j n cut:
+  h_no_var h j -> (cut <= j) -> h_no_var (Sub.h_shift h n cut) (n+j).
+Proof.
+all: assert (forall j, S(n+j)=n+(S j)) as snj by (intro; omega).
+all: assert (forall j, S(S(n+j))=n+(S(S j))) as ssnj by (intro; omega).
+{
+clear v_no_var_shift.
+revert j. induction v; intros j orig cmpjc; simpl; simpl in orig;
+try constructor; try inv orig; auto.
+{ destruct v as (x, i). destruct (cut <=? i) eqn:cmp; simpl;
+  try rewrite leb_iff_conv in cmp; omega. }
+all: rewrite snj; apply c_no_var_shift; omega || assumption.
+}{
+clear c_no_var_shift.
+revert j cut. induction c; intros j cut orig cmpjc; simpl; simpl in *.
+all: try inv orig; try constructor; try constructor; auto.
+all: try rewrite ssnj; try rewrite snj.
+all: try apply IHc || apply IHc1 || apply IHc2; omega || auto.
+all: inv H0; assumption.
+}{
+clear h_no_var_shift.
+revert j cut. induction h; intros j cut orig cmpjc; simpl;
+destruct orig; auto. constructor. auto.
+rewrite ssnj. apply c_no_var_shift. assumption. omega.
 }
 Qed.
 
 
-Lemma v_shift_0 cut v : Sub.v_shift v 0 cut = v
-with c_shift_0 cut c : Sub.c_shift c 0 cut = c
-with h_shift_0 cut h : Sub.h_shift h 0 cut = h.
+Lemma v_sub_makes_no_var (v:val) j v_s :
+  v_no_var v_s j -> v_no_var (Sub.v_sub v (j, v_s)) j
+with c_sub_makes_no_var (c:comp) j v_s :
+  v_no_var v_s j -> c_no_var (Sub.c_sub c (j, v_s)) j
+with h_sub_makes_no_var (h:hcases) j v_s :
+  v_no_var v_s j -> h_no_var (Sub.h_sub h (j, v_s)) j.
 Proof.
 {
-clear v_shift_0.
-revert cut. induction v; intros cut;
-simpl; try (specialize (IHv cut)); try rewrite IHv; try reflexivity.
-+ destruct v. simpl. destruct (cut <=? v0); try reflexivity.
-+ rewrite IHv1, IHv2. reflexivity.
-+ rewrite c_shift_0. reflexivity.
-+ f_equal; try apply c_shift_0 || apply h_shift_0.
+clear v_sub_makes_no_var.
+revert j. induction v; intros j v_s_clean; try constructor.
+all: try (apply IHv; assumption); auto.
+{ destruct v as (x, n). simpl. destruct (n =? j) eqn:nj; auto.
+  simpl. apply Nat.eqb_neq in nj. omega. }
+all: apply c_sub_makes_no_var; apply v_no_var_shift; omega || assumption.
 }{
-clear c_shift_0.
-revert cut. induction c; intros cut; simpl;
-try destruct p; f_equal;
-try apply v_shift_0 || apply IHc || apply IHc1 || apply IHc2.
+clear c_sub_makes_no_var.
+revert j v_s. induction c; intros j v_s v_s_clean; simpl.
+all: try constructor; try constructor; auto.
+all: try apply IHc || apply IHc1 || apply IHc2; auto.
+all: assert (S(S j)=2+j) as ssj by omega; try rewrite ssj.
+all: try apply v_no_var_shift; omega || auto.
 }{
-clear h_shift_0.
-revert cut. induction h; intros cut; simpl; f_equal.
-reflexivity. apply IHh. apply c_shift_0.
+clear h_sub_makes_no_var.
+revert j v_s. induction h; intros j v_s v_s_clean; simpl; auto.
+constructor. auto. assert (S(S j)=2+j) as ssj by omega. rewrite ssj.
+apply c_sub_makes_no_var. apply v_no_var_shift. assumption. omega.
 }
 Qed.
 
+
+Fixpoint v_under_var_shift v j n cut:
+  v_under_var v j -> cut <= j -> v_under_var (Sub.v_shift v n cut) (n+j)
+with c_under_var_shift c j n cut:
+  c_under_var c j -> cut <= j -> c_under_var (Sub.c_shift c n cut) (n+j)
+with h_under_var_shift h j n cut:
+  h_under_var h j -> cut <= j -> h_under_var (Sub.h_shift h n cut) (n+j).
+Proof.
+all: assert (S(n+j)=n+S j) as Snj by omega.
+all: assert (S(S(n+j))=n+S(S j)) as SSnj by omega.
+{
+intros under cmp. destruct v; simpl; simpl in under; auto.
+{ destruct v. destruct (cut <=? v0) eqn:ccmp; simpl; omega. }
+all: try (destruct under; constructor; auto).
+all: rewrite Snj; eapply c_under_var_shift; eauto; omega.
+}{
+intros under cmp. destruct c; simpl; simpl in under; auto.
+all: try (destruct under; constructor; auto).
+all: try rewrite SSnj; try rewrite Snj.
+2: destruct H0; constructor.
+all: eapply c_under_var_shift; eauto; omega.
+}{
+intros under cmp. destruct h; simpl; simpl in under. auto.
+destruct under. constructor. auto.
+rewrite SSnj. eapply c_under_var_shift; eauto; omega.
+}
+Qed.
+
+
+Fixpoint v_shift_too_high v n cut :
+  v_under_var v cut -> Sub.v_shift v n cut = v
+with c_shift_too_high c n cut :
+  c_under_var c cut -> Sub.c_shift c n cut = c
+with h_shift_too_high h n cut :
+  h_under_var h cut -> Sub.h_shift h n cut = h.
+Proof.
+{
+intros under. destruct v; simpl; simpl in under.
+{ destruct v. assert (cut <=? v0 = false) by (apply leb_correct_conv; omega).
+  rewrite H. reflexivity. }
+all: try (destruct under; f_equal; auto) || (f_equal; auto).
+}{
+intros under. destruct c; simpl; simpl in under.
+all: try (destruct under; f_equal; auto) || (f_equal; auto); destruct H0; auto.
+}{
+intros under. destruct h; simpl; simpl in under.
+all: try (destruct under; f_equal; auto) || (f_equal; auto).
+}
+Qed.
+
+
+Fixpoint v_negshift_too_high v n cut :
+  v_under_var v cut -> Sub.v_negshift v n cut = v
+with c_negshift_too_high c n cut :
+  c_under_var c cut -> Sub.c_negshift c n cut = c
+with h_negshift_too_high h n cut :
+  h_under_var h cut -> Sub.h_negshift h n cut = h.
+Proof.
+{
+intros under. destruct v; simpl; simpl in under.
+{ destruct v. assert (cut <=? v0 = false) by (apply leb_correct_conv; omega).
+  rewrite H. reflexivity. }
+all: try (destruct under; f_equal; auto) || (f_equal; auto).
+}{
+intros under. destruct c; simpl; simpl in under.
+all: try (destruct under; f_equal; auto) || (f_equal; auto); destruct H0; auto.
+}{
+intros under. destruct h; simpl; simpl in under.
+all: try (destruct under; f_equal; auto) || (f_equal; auto).
+}
+Qed.
+
+
+Fixpoint v_sub_too_high v i v_s:
+  v_under_var v i -> Sub.v_sub v (i, v_s) = v
+with c_sub_too_high c i v_s:
+  c_under_var c i -> Sub.c_sub c (i, v_s) = c
+with h_sub_too_high h i v_s:
+  h_under_var h i -> Sub.h_sub h (i, v_s) = h.
+Proof.
+{
+intros under. destruct v; simpl; simpl in under.
+{ destruct v. assert (v0=?i=false) by (apply Nat.eqb_neq; omega).
+  rewrite H. reflexivity. }
+all: try (destruct under; f_equal; auto) || (f_equal; auto).
+}{
+intros under. destruct c; simpl; simpl in under.
+all: try (destruct under; f_equal; auto) || (f_equal; auto); destruct H0; auto.
+}{
+intros under. destruct h; simpl; simpl in under.
+all: try (destruct under; f_equal; auto) || (f_equal; auto).
+}
+Qed.
+
+
+Fixpoint v_sub_no_var v v' i {struct v}:
+  v_no_var v i -> Sub.v_sub v (i, v') = v
+with c_sub_no_var c v' i {struct c}:
+  c_no_var c i -> Sub.c_sub c (i, v') = c
+with h_sub_no_var h v' i {struct h}:
+  h_no_var h i -> Sub.h_sub h (i, v') = h.
+Proof.
+all: revert i.
++ intros i novar. destruct v; simpl in novar; try destruct novar. 
+  { destruct v as (x,d). simpl.
+    assert (d=?i=false) by (apply Nat.eqb_neq; omega).
+    rewrite H. reflexivity. }
+  all: simpl in *; f_equal; auto.
++ intros i novar. induction c; simpl in *; try destruct novar.
+  all: f_equal; auto. all: destruct H0; auto.
++ intros i novar. induction h; simpl in *; try destruct novar.
+  all: f_equal; auto.
+Qed.
+
+(* ==================== Sub Interactions ==================== *)
 
 Lemma v_shift_sub v v' i cut j :
   cut <= j ->
-  Sub.v_shift (Sub.v_sub v (j, v')) i cut 
+    Sub.v_shift (Sub.v_sub v (j, v')) i cut 
   = Sub.v_sub (Sub.v_shift v i cut) (i+j, Sub.v_shift v' i cut)
+
 with c_shift_sub c v' i cut j :
   cut <= j ->
-  Sub.c_shift (Sub.c_sub c (j, v')) i cut 
+    Sub.c_shift (Sub.c_sub c (j, v')) i cut 
   = Sub.c_sub (Sub.c_shift c i cut) (i+j, Sub.v_shift v' i cut)
+
 with h_shift_sub h v' i cut j :
   cut <= j ->
-  Sub.h_shift (Sub.h_sub h (j, v')) i cut
+    Sub.h_shift (Sub.h_sub h (j, v')) i cut
   = Sub.h_sub (Sub.h_shift h i cut) (i+j, Sub.v_shift v' i cut).
 Proof.
+all : assert (S(i+j)=i+(S j)) as sij by omega.
+all : assert (S(S(i+j))=i+(S (S j))) as ssij by omega.
 {
-revert i cut j; induction v; intros i cut j cmpcj; simpl.
-{ 
-destruct v as (x, d). simpl.
-destruct (cut<=?d) eqn:cd.
-+ destruct (d=?j) eqn:dj.
-   * apply Nat.eqb_eq in dj. subst. simpl.
-     assert (i+j=?i+j=true) by (apply Nat.eqb_eq; omega).
-     rewrite H. reflexivity.
-   * simpl. rewrite cd. assert (i+d=?i+j=false).
-     { apply Nat.eqb_neq. apply Nat.eqb_neq in dj. omega. }
-     rewrite H. reflexivity.
-+ assert (d=?j=false).
-  { apply Nat.eqb_neq. apply leb_complete_conv in cd. omega. }
-  rewrite H. simpl. rewrite cd.
-  assert (d=?i+j=false).
-  { apply Nat.eqb_neq. apply leb_complete_conv in cd. omega. }
-  rewrite H0. reflexivity.
+revert cut; induction v; intros cut cmpcj; simpl.
+{ destruct v as (x, d). simpl. destruct (cut<=?d) eqn:cd.
+  + destruct (d=?j) eqn:dj.
+    * apply Nat.eqb_eq in dj. subst. simpl.
+      assert (i+j=?i+j=true) by (apply Nat.eqb_eq; omega).
+      rewrite H. reflexivity.
+    * simpl. rewrite cd. assert (i+d=?i+j=false).
+      { apply Nat.eqb_neq. apply Nat.eqb_neq in dj. omega. }
+      rewrite H. reflexivity.
+  + assert (d=?j=false).
+    { apply Nat.eqb_neq. apply leb_complete_conv in cd. omega. }
+    rewrite H. simpl. rewrite cd.
+    assert (d=?i+j=false).
+    { apply Nat.eqb_neq. apply leb_complete_conv in cd. omega. }
+    rewrite H0. reflexivity.
 }
-all : f_equal; try reflexivity || apply IHv || apply IHv1 || apply IHv2; auto.
-all : assert (S(i+j)=i+(S j)) as sij by omega; rewrite sij.
-all : rewrite v_shift_comm_aux, c_shift_sub; try omega || f_equal.
+all : f_equal; auto.
+all : rewrite sij, v_shift_comm, c_shift_sub; try omega || f_equal.
 }{
 clear h_shift_sub.
-revert i cut j; induction c; intros i cut j cmpcj; simpl; f_equal; auto.
-all : assert (S(S(i+j))=i+(S (S j))) as ssij by omega; try rewrite ssij.
-all : assert (S(i+j)=i+(S j)) as sij by omega; try rewrite sij.
-all: rewrite v_shift_comm_aux, c_shift_sub; try omega || f_equal.
+revert cut; induction c; intros cut cmpcj; simpl; f_equal; auto.
+all : try rewrite ssij; try rewrite sij.
+all: rewrite v_shift_comm, c_shift_sub; try omega || f_equal.
 }{
 clear v_shift_sub h_shift_sub.
-revert i cut j; induction h; intros i cut j cmpcj; simpl; f_equal; auto.
-+ assert (S(S(i+j))=i+(S (S j))) as ssij by omega. rewrite ssij.
-  rewrite v_shift_comm_aux, c_shift_sub; try omega || f_equal.
+revert cut; induction h; intros cut cmpcj; simpl; f_equal; auto.
++ rewrite ssij, v_shift_comm, c_shift_sub; try omega || f_equal.
 }
 Qed.
 
 Lemma v_negshift_sub v v' cut j :
   cut < j -> v_no_var v cut -> v_no_var v' cut ->
-  Sub.v_negshift (Sub.v_sub v (j, v')) 1 cut 
+    Sub.v_negshift (Sub.v_sub v (j, v')) 1 cut 
   = Sub.v_sub (Sub.v_negshift v 1 cut) (j-1, Sub.v_negshift v' 1 cut)
+
 with c_negshift_sub c v' cut j :
   cut < j -> c_no_var c cut -> v_no_var v' cut ->
-  Sub.c_negshift (Sub.c_sub c (j, v')) 1 cut 
+    Sub.c_negshift (Sub.c_sub c (j, v')) 1 cut 
   = Sub.c_sub (Sub.c_negshift c 1 cut) (j-1, Sub.v_negshift v' 1 cut)
+
 with h_negshift_sub h v' cut j :
   cut < j -> h_no_var h cut -> v_no_var v' cut ->
-  Sub.h_negshift (Sub.h_sub h (j, v')) 1 cut
+    Sub.h_negshift (Sub.h_sub h (j, v')) 1 cut
   = Sub.h_sub (Sub.h_negshift h 1 cut) (j-1, Sub.v_negshift v' 1 cut).
 Proof.
 {
@@ -486,63 +505,56 @@ destruct (cut<=?d) eqn:cd.
   { apply Nat.eqb_neq. apply leb_complete_conv in cd. omega. }
   rewrite H0. reflexivity.
 }
-all : f_equal; try reflexivity || apply IHv || apply IHv1 || apply IHv2; auto.
-all : simpl in novar; try (destruct novar; auto).
-all : rewrite c_negshift_sub; try omega || (f_equal; f_equal; auto).
+all : simpl in novar; try (destruct novar; auto); f_equal; auto.
+all : rewrite c_negshift_sub; try omega || (f_equal; f_equal; omega || auto).
 all : clear v_negshift_sub c_negshift_sub h_negshift_sub.
-all : try rewrite v_shift_negshift_1j; f_equal || omega || auto.
+all : try rewrite v_shift_negshift_comm; f_equal || omega || auto.
 all : apply v_no_var_shift; omega || auto.
 }{
 clear h_negshift_sub.
 revert cut j; induction c; intros cut j cmpcj novar novar'; simpl.
-all : simpl in novar; f_equal; try destruct novar.
-all : try apply v_negshift_sub; omega || auto.
+all : simpl in novar; try destruct novar; f_equal; auto.
 all : clear v_negshift_sub.
-all : assert (S(S cut)=1+(1+cut)) as ssc by omega; try rewrite ssc.
+all : assert (S(S cut)=2+cut) as ssc by omega; try rewrite ssc.
 all : assert (S cut=1+cut) as sc by omega; try rewrite sc.
 all : try destruct H0.
-all : try rewrite c_negshift_sub; (f_equal; f_equal) || omega || auto.
-all : clear c_negshift_sub.
-all : try rewrite v_shift_negshift_1j; f_equal || omega || auto.
+all : try rewrite c_negshift_sub; (f_equal; f_equal; try omega) || auto.
+all : try rewrite v_shift_negshift_comm; f_equal || omega || auto.
 all : try apply v_no_var_shift; omega || auto.
-all : assert (1+(1+cut)=2+cut) as cc by omega; rewrite cc.
-all : apply v_no_var_shift; omega || auto.
 }{
 clear v_negshift_sub h_negshift_sub.
 revert cut j; induction h; intros cut j cmpcj novar novar'.
 all : simpl; f_equal; simpl in novar; try destruct novar; auto.
-try rewrite c_negshift_sub; (f_equal; f_equal) || omega || auto.
-omega. clear c_negshift_sub.
-rewrite v_shift_negshift_1j; f_equal || omega || auto.
+try rewrite c_negshift_sub. f_equal. f_equal. all: omega || auto.
+rewrite v_shift_negshift_comm. f_equal. assumption. omega.
 assert (S(S cut)=2+cut) as cc by omega; rewrite cc.
-apply v_no_var_shift; omega || auto.
+apply v_no_var_shift. assumption. omega.
 }
 Qed.
 
 
-Lemma v_sub_sub v v' v'' i j :
+Lemma v_sub_sub v v1 v2 i j :
   v_no_var v j ->
-  Sub.v_sub v (i, Sub.v_sub v' (j, v''))
-  = Sub.v_sub (Sub.v_sub v (i, v')) (j, v'')
-with c_sub_sub c v' v'' i j :
+    Sub.v_sub v (i, Sub.v_sub v1 (j, v2))
+  = Sub.v_sub (Sub.v_sub v (i, v1)) (j, v2)
+
+with c_sub_sub c v1 v2 i j :
   c_no_var c j ->
-  Sub.c_sub c (i, Sub.v_sub v' (j, v''))
-  = Sub.c_sub (Sub.c_sub c (i, v')) (j, v'')
-with h_sub_sub h v' v'' i j :
+    Sub.c_sub c (i, Sub.v_sub v1 (j, v2))
+  = Sub.c_sub (Sub.c_sub c (i, v1)) (j, v2)
+
+with h_sub_sub h v1 v2 i j :
   h_no_var h j ->
-  Sub.h_sub h (i, Sub.v_sub v' (j, v''))
-  = Sub.h_sub (Sub.h_sub h (i, v')) (j, v'').
+    Sub.h_sub h (i, Sub.v_sub v1 (j, v2))
+  = Sub.h_sub (Sub.h_sub h (i, v1)) (j, v2).
 Proof.
 {
 revert i j; induction v; intros i j novar; simpl.
-{ 
-destruct v as (x, d). simpl.
-destruct (d=?i) eqn:cd. reflexivity.
-simpl. simpl in novar. assert (d=?j=false) by (apply Nat.eqb_neq; omega).
-rewrite H. reflexivity.
-}
-all : f_equal; try reflexivity || apply IHv || apply IHv1 || apply IHv2; auto.
-all : simpl in novar; try destruct novar; auto.
+{ destruct v as (x, d). simpl.
+  destruct (d=?i) eqn:cd. reflexivity.
+  simpl in *. assert (d=?j=false) by (apply Nat.eqb_neq; omega).
+  rewrite H. reflexivity. }
+all : simpl in novar; try destruct novar; f_equal; auto.
 all : rewrite v_shift_sub, c_sub_sub; omega || auto.
 }{
 clear h_sub_sub.
@@ -558,127 +570,7 @@ rewrite v_shift_sub, c_sub_sub; omega || auto.
 }
 Qed.
 
-
-
-Fixpoint v_under_var_shift v j n cut:
-  v_under_var v j -> cut <= j -> v_under_var (Sub.v_shift v n cut) (n+j)
-
-with c_under_var_shift c j n cut:
-  c_under_var c j -> cut <= j -> c_under_var (Sub.c_shift c n cut) (n+j)
-
-with h_under_var_shift h j n cut:
-  h_under_var h j -> cut <= j -> h_under_var (Sub.h_shift h n cut) (n+j).
-Proof.
-{
-intros under cmp. destruct v; simpl; simpl in under; auto.
-{ destruct v. destruct (cut <=? v0) eqn:ccmp; simpl; omega. }
-all: try (destruct under; constructor; auto).
-all: assert (S(n+j)=n+S j) as Snj by omega; rewrite Snj.
-all: eapply c_under_var_shift; eauto; omega.
-}{
-intros under cmp. destruct c; simpl; simpl in under; auto.
-all: try (destruct under; constructor; auto).
-all: assert (S(S(n+j))=n+S(S j)) as SSnj by omega; try rewrite SSnj.
-all: assert (S(n+j)=n+S j) as Snj by omega; try rewrite Snj.
-2: destruct H0; constructor.
-all: eapply c_under_var_shift; eauto; omega.
-}{
-intros under cmp. destruct h; simpl; simpl in under. auto.
-destruct under. constructor. auto.
-assert (S(S(n+j))=n+S(S j)) as SSnj by omega; try rewrite SSnj.
-eapply c_under_var_shift; eauto; omega.
-}
-Qed.
-
-Fixpoint v_shift_too_high v n cut :
-  v_under_var v cut -> Sub.v_shift v n cut = v
-with c_shift_too_high c n cut :
-  c_under_var c cut -> Sub.c_shift c n cut = c
-with h_shift_too_high h n cut :
-  h_under_var h cut -> Sub.h_shift h n cut = h.
-Proof.
-{
-intros under. destruct v; simpl; simpl in under.
-{ destruct v.
-  assert (cut <=? v0 = false) by (apply leb_correct_conv; omega).
-  rewrite H. reflexivity. }
-all: try (destruct under; f_equal; auto) || (f_equal; auto).
-}{
-intros under. destruct c; simpl; simpl in under.
-all: try (destruct under; f_equal; auto) || (f_equal; auto).
-all: destruct H0; auto.
-}{
-intros under. destruct h; simpl; simpl in under.
-all: try (destruct under; f_equal; auto) || (f_equal; auto).
-}
-Qed.
-
-Fixpoint v_negshift_too_high v n cut :
-  v_under_var v cut -> Sub.v_negshift v n cut = v
-with c_negshift_too_high c n cut :
-  c_under_var c cut -> Sub.c_negshift c n cut = c
-with h_negshift_too_high h n cut :
-  h_under_var h cut -> Sub.h_negshift h n cut = h.
-Proof.
-{
-intros under. destruct v; simpl; simpl in under.
-{ destruct v.
-  assert (cut <=? v0 = false) by (apply leb_correct_conv; omega).
-  rewrite H. reflexivity. }
-all: try (destruct under; f_equal; auto) || (f_equal; auto).
-}{
-intros under. destruct c; simpl; simpl in under.
-all: try (destruct under; f_equal; auto) || (f_equal; auto).
-all: destruct H0; auto.
-}{
-intros under. destruct h; simpl; simpl in under.
-all: try (destruct under; f_equal; auto) || (f_equal; auto).
-}
-Qed.
-
-Fixpoint v_sub_too_high v i v_s:
-  v_under_var v i -> Sub.v_sub v (i, v_s) = v
-with c_sub_too_high c i v_s:
-  c_under_var c i -> Sub.c_sub c (i, v_s) = c
-with h_sub_too_high h i v_s:
-  h_under_var h i -> Sub.h_sub h (i, v_s) = h.
-Proof.
-{
-intros under. destruct v; simpl; simpl in under.
-{ destruct v.
-  assert (v0 =? i = false) by (apply Nat.eqb_neq; omega).
-  rewrite H. reflexivity. }
-all: try (destruct under; f_equal; auto) || (f_equal; auto).
-}{
-intros under. destruct c; simpl; simpl in under.
-all: try (destruct under; f_equal; auto) || (f_equal; auto).
-all: destruct H0; auto.
-}{
-intros under. destruct h; simpl; simpl in under.
-all: try (destruct under; f_equal; auto) || (f_equal; auto).
-}
-Qed.
-
-Fixpoint v_sub_no_var v v' i {struct v}:
-  v_no_var v i -> Sub.v_sub v (i, v') = v
-with c_sub_no_var c v' i {struct c}:
-  c_no_var c i -> Sub.c_sub c (i, v') = c
-with h_sub_no_var h v' i {struct h}:
-  h_no_var h i -> Sub.h_sub h (i, v') = h.
-Proof.
-all: revert i.
-+ intros i novar. destruct v; simpl in novar; try destruct novar. 
-  { destruct v as (x,d). simpl.
-    assert (d=?i=false) by (apply Nat.eqb_neq; omega).
-    rewrite H. reflexivity.
-  }
-  all: simpl in *; f_equal; auto.
-+ intros i novar. induction c; simpl in *; try destruct novar.
-  all: f_equal; auto. all: destruct H0; auto.
-+ intros i novar. induction h; simpl in *; try destruct novar.
-  all: f_equal; auto.
-Qed.
-
+(* ==================== Full Subs Properties ==================== *)
 
 Fixpoint v_under_var_subs v v' i j {struct v}:
   v_under_var v i -> v_under_var v' i -> v_under_var (v_subs v v' j) i
@@ -692,89 +584,75 @@ all: revert i j.
   { destruct v as (x,d). unfold v_subs. simpl. simpl in H.
     destruct (d=?j).
     + rewrite v_negshift_shift, v_shift_0. auto. omega.
-    + simpl. destruct (j<=?d); simpl; omega.
-  }
-  all: simpl in *; auto.
-  - apply v_under_var_subs; auto.
-  - apply v_under_var_subs; auto.
-  - constructor; inv H; apply v_under_var_subs; auto.
-  - rewrite v_shift_comm_aux. apply c_under_var_subs. auto.
-    apply v_under_var_shift. auto. omega. omega.
-  - constructor; inv H.
-    * rewrite v_shift_comm_aux. apply c_under_var_subs. auto.
-      apply v_under_var_shift. auto. omega. omega.
-    * apply h_under_var_subs; auto.
+    + simpl. destruct (j<=?d); simpl; omega. }
+  all: simpl in *; try inv H; try constructor.
+  all: try apply v_under_var_subs || apply h_under_var_subs; auto.
+  all: rewrite v_shift_comm; apply c_under_var_subs || omega; auto.
+  all: apply v_under_var_shift; omega || assumption.
 + intros. induction c; simpl in *; auto.
-  all: try constructor; try inv H; auto.
+  all: try constructor; try constructor; try inv H; auto.
   all: try apply v_under_var_subs; eauto.
-  2: constructor; inv H2.
-  all: rewrite v_shift_comm_aux; try apply c_under_var_subs; omega || auto.
-  all: try apply v_under_var_shift; omega || auto.
+  all: rewrite v_shift_comm; try apply c_under_var_subs; omega || auto.
+  all: try apply v_under_var_shift; omega || (try destruct H2; auto).
   all: assert (S(S i) = 2+i) by omega; rewrite H; apply v_under_var_shift.
-  all: omega || auto.
+  all: omega || assumption.
 + intros. induction h; simpl in *; auto.
   constructor; inv H; auto.
-  rewrite v_shift_comm_aux; try apply c_under_var_subs; omega || auto.
+  rewrite v_shift_comm; try apply c_under_var_subs; omega || auto.
   assert (S(S i) = 2+i) by omega; rewrite H; apply v_under_var_shift.
-  auto. omega.
+  assumption. omega.
 Qed.
+
 
 Fixpoint v_no_var_subs v v' i j {struct v}:
   v_no_var v (1+i) -> v_no_var v' i -> j<=i ->
   v_no_var (v_subs v v' j) i
+
 with c_no_var_subs c v' i j {struct c}:
   c_no_var c (1+i) -> v_no_var v' i -> j<=i ->
   c_no_var (c_subs c v' j) i
+
 with h_no_var_subs h v' i j {struct h}:
   h_no_var h (1+i) -> v_no_var v' i -> j<=i ->
   h_no_var (h_subs h v' j) i.
 Proof.
 all: revert i j.
 + intros. destruct v.
-  { 
-    destruct v as (x,d). unfold v_subs. simpl. simpl in H.
+  { destruct v as (x,d). unfold v_subs. simpl. simpl in H.
     destruct (d=?j) eqn:dj.
     + rewrite v_negshift_shift, v_shift_0. auto. omega.
     + simpl. destruct (j<=?d) eqn:jld; simpl; apply Nat.eqb_neq in dj.
       - apply leb_complete in jld. omega.
-      - apply leb_complete_conv in jld. omega.
-  }
-  all: simpl in *; auto.
-  - apply v_no_var_subs; auto.
-  - apply v_no_var_subs; auto.
-  - constructor; inv H; apply v_no_var_subs; auto.
-  - rewrite v_shift_comm_aux. apply c_no_var_subs. auto.
-    apply v_no_var_shift. auto. all: omega.
-  - constructor; inv H.
-    * rewrite v_shift_comm_aux. apply c_no_var_subs. auto.
-      apply v_no_var_shift. auto. all: omega.
-    * apply h_no_var_subs; auto.
-+ intros. induction c; simpl in *; auto.
-  all: try constructor; try inv H; auto.
+      - apply leb_complete_conv in jld. omega. }
+  all: simpl in *; try inv H; try constructor.
+  all: try apply v_no_var_subs || apply h_no_var_subs; auto.
+  all: rewrite v_shift_comm; apply c_no_var_subs || omega; omega || auto.
+  all: apply v_no_var_shift; omega || assumption.
++ intros. induction c; simpl in *; try constructor; try constructor.
+  all: try inv H; try inv H3; auto.
   all: try apply v_no_var_subs; eauto.
-  2: constructor; inv H3.
-  all: rewrite v_shift_comm_aux; try apply c_no_var_subs; omega || auto.
+  all: rewrite v_shift_comm; try apply c_no_var_subs; omega || auto.
   all: try apply v_no_var_shift; omega || auto.
   all: assert (S(S i) = 2+i) by omega; rewrite H; apply v_no_var_shift.
-  all: omega || auto.
-+ intros. induction h; simpl in *; auto.
-  constructor; inv H; auto.
-  rewrite v_shift_comm_aux; try apply c_no_var_subs; omega || auto.
+  all: omega || assumption.
++ intros. induction h; simpl in *; auto. inv H; constructor; auto.
+  rewrite v_shift_comm; try apply c_no_var_subs; omega || auto.
   assert (S(S i) = 2+i) by omega; rewrite H; apply v_no_var_shift.
-  auto. omega.
+  assumption. omega.
 Qed.
 
 
-
 Lemma v_shift_subs v v' i j (safe: j <= i): 
-  Sub.v_shift (v_subs v v' j) 1 i = 
-  (v_subs (Sub.v_shift v 1 (1+i)) (Sub.v_shift v' 1 i) j)
+    Sub.v_shift (v_subs v v' j) 1 i
+  = (v_subs (Sub.v_shift v 1 (1+i)) (Sub.v_shift v' 1 i) j)
+
 with c_shift_subs c v' i j (safe: j <= i): 
-  Sub.c_shift (c_subs c v' j) 1 i = 
-  (c_subs (Sub.c_shift c 1 (1+i)) (Sub.v_shift v' 1 i) j)
+    Sub.c_shift (c_subs c v' j) 1 i
+  = (c_subs (Sub.c_shift c 1 (1+i)) (Sub.v_shift v' 1 i) j)
+
 with h_shift_subs h v' i j (safe: j <= i): 
-  Sub.h_shift (h_subs h v' j) 1 i = 
-  (h_subs (Sub.h_shift h 1 (1+i)) (Sub.v_shift v' 1 i) j).
+    Sub.h_shift (h_subs h v' j) 1 i
+  = (h_subs (Sub.h_shift h 1 (1+i)) (Sub.v_shift v' 1 i) j).
 Proof.
 {
 induction v; unfold v_subs; simpl.
@@ -789,135 +667,113 @@ apply Nat.eqb_eq in ni. subst.
     simpl in H. rewrite H. simpl.
     assert (j=?j=true) by (apply Nat.eqb_eq; reflexivity).
     rewrite H0. simpl. 
-    rewrite v_negshift_shift. rewrite v_negshift_shift.
-    rewrite v_shift_shift. rewrite v_shift_shift. f_equal.
-    omega. omega.
+    rewrite v_negshift_shift, v_negshift_shift, v_shift_shift, v_shift_shift. f_equal. omega. omega.
   - assert (1+i<=?i=false) by (apply leb_correct_conv; omega).
-    simpl in H. rewrite H. simpl.
-    assert (j<=?i=true) by (apply leb_correct;omega).
-    rewrite H0. rewrite eqij. simpl. rewrite H0.
-    assert (i<=?i-1=false).
-    { apply leb_correct_conv. apply Nat.eqb_neq in eqij. 
-      apply leb_complete in H0. omega. }
-    rewrite H1. reflexivity.
+    simpl in H. rewrite H. simpl. apply leb_correct in safe as s.
+    rewrite s, eqij. simpl. rewrite s. assert (i<=?i-1=false).
+    { apply leb_correct_conv. apply Nat.eqb_neq in eqij. omega. } 
+    rewrite H0. reflexivity.
 + destruct (n=?j) eqn:nj.
-  ++apply Nat.eqb_eq in nj. subst.
+  * apply Nat.eqb_eq in nj. subst.
     assert (1+i<=?j=false) by (apply leb_correct_conv; omega).
-    simpl in H. rewrite H.
-    simpl. assert (j=?j=true) by (apply Nat.eqb_eq; omega).
-    rewrite H0. rewrite v_negshift_shift. rewrite v_negshift_shift. simpl.
-    rewrite v_shift_0. rewrite v_shift_0.
+    simpl in H. rewrite H. simpl.
+    assert (j=?j=true) by (apply Nat.eqb_eq; omega).
+    rewrite H0, v_negshift_shift, v_negshift_shift, v_shift_0, v_shift_0.
     reflexivity. omega. omega.
-  ++destruct (i<=?n) eqn:iln; simpl.
-    - destruct (j<=?n) eqn:jln; simpl.
-      * apply leb_complete in jln. apply leb_complete in iln.
-        assert (i<=?n-1=true).
-        { apply leb_correct. apply Nat.eqb_neq in ni. omega. }
-        rewrite H. simpl. assert (1+i<=?n=true).
-        { apply leb_correct. apply leb_complete in H.
-          apply Nat.eqb_neq in ni. omega. }
-        simpl in H0. rewrite H0. simpl. 
-        assert (1+n=?j=false).
-        { apply Nat.eqb_neq. omega. }
-        simpl in H1. rewrite H1. simpl. assert (j<=? S n=true).
-        { apply leb_correct. omega. }
-        rewrite H2. simpl.
-        f_equal. f_equal. assert (n>0) by (apply Nat.eqb_neq in ni; omega).
-        omega.
-      * apply leb_complete in iln. apply leb_complete_conv in jln. omega.
+  * destruct (i<=?n) eqn:iln; simpl.
+    - apply leb_complete in iln.
+      assert (j<=?n=true) by (apply leb_correct; omega). rewrite H. simpl.
+      assert (i<=?n-1=true).
+      { apply leb_correct. apply Nat.eqb_neq in ni. omega. }
+      rewrite H0. simpl. assert (1+i<=?n=true).
+      { apply leb_correct. apply Nat.eqb_neq in ni. omega. }
+      simpl in H1. rewrite H1. simpl. 
+      assert (1+n=?j=false) by (apply Nat.eqb_neq; omega).
+      simpl in H2. rewrite H2. simpl. assert (j<=? S n=true).
+      { apply leb_correct. omega. }
+      rewrite H3. do 2 f_equal. apply Nat.eqb_neq in ni. omega.
     - apply leb_complete_conv in iln.
       assert (1+i<=?n=false) by (apply leb_correct_conv; omega).
       simpl in H. rewrite H. simpl. rewrite nj. simpl.
       destruct (j<=?n) eqn:jln.
-      * simpl. assert (i<=?n-1=false).
-        { apply leb_correct_conv. omega. }
-        rewrite H0. reflexivity.
-      * simpl. assert (i<=?n=false) by (apply leb_correct_conv; omega).
-        rewrite H0. reflexivity.
-}     
+      simpl. assert (i<=?n-1=false) by (apply leb_correct_conv; omega).
+      rewrite H0. reflexivity.
+      simpl. assert (i<=?n=false) by (apply leb_correct_conv; omega).
+      rewrite H0. reflexivity.
+}
 all: f_equal; auto.
 3: apply h_shift_subs; auto.
 all: clear v_shift_subs h_shift_subs; unfold c_subs in c_shift_subs.
-all: rewrite v_shift_comm_aux; try omega.
+all: rewrite v_shift_comm; try omega.
 all: rewrite c_shift_subs; clear c_shift_subs; try omega.
-all: do 3 f_equal; rewrite (v_shift_comm_aux 1 j); f_equal; try omega.
-all: rewrite (v_shift_comm_aux 1 i); f_equal; omega.
+all: do 3 f_equal; rewrite (v_shift_comm 1 j); f_equal; try omega.
+all: rewrite (v_shift_comm 1 i); f_equal; omega.
 }{
 destruct c; unfold c_subs; simpl; f_equal;
 try apply v_shift_subs; try assumption.
 all: clear v_shift_subs h_shift_subs; unfold c_subs in c_shift_subs.
-+ rewrite <-(v_shift_shift 1), (v_shift_comm_aux 1 j).
-  rewrite (v_shift_comm_aux 1 (1+j)), c_shift_subs. clear c_shift_subs. simpl.
-  do 2 f_equal. all: try omega.
-  rewrite <-(v_shift_shift 1 1 0), (v_shift_comm_aux 1 j).
-  rewrite (v_shift_comm_aux 1 (1+j)). f_equal. 
-  rewrite (v_shift_comm_aux 1 i), (v_shift_comm_aux 1 (1+i)). 
-  do 2 f_equal. all: omega.
-+ rewrite v_shift_comm_aux. rewrite c_shift_subs. clear c_shift_subs.
-  do 3 f_equal. rewrite (v_shift_comm_aux 1 j). f_equal.
-  rewrite (v_shift_comm_aux 1 i). f_equal. all: omega.
-+ rewrite v_shift_comm_aux. rewrite c_shift_subs. clear c_shift_subs.
-  do 3 f_equal. rewrite (v_shift_comm_aux 1 j). f_equal.
-  rewrite (v_shift_comm_aux 1 i). f_equal. all: omega.
-+ rewrite v_shift_comm_aux. rewrite c_shift_subs. clear c_shift_subs.
-  do 3 f_equal. rewrite (v_shift_comm_aux 1 j). f_equal.
-  rewrite (v_shift_comm_aux 1 i). f_equal. all: omega.
-+ rewrite <-(v_shift_shift 1), (v_shift_comm_aux 1 j).
-  rewrite (v_shift_comm_aux 1 (1+j)), c_shift_subs. clear c_shift_subs. simpl.
-  do 2 f_equal. all: try omega.
-  rewrite <-(v_shift_shift 1 1 0), (v_shift_comm_aux 1 j).
-  rewrite (v_shift_comm_aux 1 (1+j)). f_equal. 
-  rewrite (v_shift_comm_aux 1 i), (v_shift_comm_aux 1 (1+i)). 
-  do 2 f_equal. all: omega.
-+ rewrite v_shift_comm_aux. rewrite c_shift_subs. clear c_shift_subs.
-  do 3 f_equal. rewrite (v_shift_comm_aux 1 j). f_equal.
-  rewrite (v_shift_comm_aux 1 i). f_equal. all: omega.
-+ rewrite v_shift_comm_aux. rewrite c_shift_subs. clear c_shift_subs.
-  do 2 f_equal. rewrite (v_shift_comm_aux). reflexivity. all: omega.
-+ rewrite v_shift_comm_aux. rewrite c_shift_subs. clear c_shift_subs.
-  do 3 f_equal. rewrite (v_shift_comm_aux 1 j). f_equal.
-  rewrite (v_shift_comm_aux 1 i). f_equal. all: omega.
-+ rewrite v_shift_comm_aux. rewrite c_shift_subs. clear c_shift_subs.
-  do 2 f_equal. rewrite (v_shift_comm_aux). reflexivity. all: omega.
++ rewrite <-(v_shift_shift 1), (v_shift_comm 1 j).
+  rewrite (v_shift_comm 1 (1+j)), c_shift_subs. clear c_shift_subs. simpl.
+  do 2 f_equal. all: try omega. 
+  rewrite <-(v_shift_shift 1 1 0), (v_shift_comm 1 j), (v_shift_comm 1 (1+j)).
+  all: f_equal||omega||auto. 
+  rewrite (v_shift_comm 1 i), (v_shift_comm 1 (1+i)). do 2 f_equal. all: omega.
++ rewrite v_shift_comm, c_shift_subs. clear c_shift_subs. do 3 f_equal.
+  rewrite (v_shift_comm 1 j), (v_shift_comm 1 i). do 2 f_equal. all: omega.
++ rewrite v_shift_comm, c_shift_subs. clear c_shift_subs. do 3 f_equal.
+  rewrite (v_shift_comm 1 j), (v_shift_comm 1 i). do 2 f_equal. all: omega.
++ rewrite v_shift_comm, c_shift_subs. clear c_shift_subs. do 3 f_equal.
+  rewrite (v_shift_comm 1 j), (v_shift_comm 1 i). do 2 f_equal. all: omega.
++ rewrite <-(v_shift_shift 1), (v_shift_comm 1 j).
+  rewrite (v_shift_comm 1 (1+j)), c_shift_subs. clear c_shift_subs. simpl.
+  do 2 f_equal. all: try omega. 
+  rewrite <-(v_shift_shift 1 1 0), (v_shift_comm 1 j), (v_shift_comm 1 (1+j)).
+  all: f_equal||omega||auto. 
+  rewrite (v_shift_comm 1 i), (v_shift_comm 1 (1+i)). do 2 f_equal. all: omega.
++ rewrite v_shift_comm, c_shift_subs. clear c_shift_subs. do 3 f_equal.
+  rewrite (v_shift_comm 1 j), (v_shift_comm 1 i). do 2 f_equal. all: omega.
++ rewrite v_shift_comm. rewrite c_shift_subs. clear c_shift_subs.
+  do 2 f_equal. rewrite (v_shift_comm). reflexivity. all: omega.
++ rewrite v_shift_comm, c_shift_subs. clear c_shift_subs. do 3 f_equal.
+  rewrite (v_shift_comm 1 j), (v_shift_comm 1 i). do 2 f_equal. all: omega.
++ rewrite v_shift_comm. rewrite c_shift_subs. clear c_shift_subs.
+  do 2 f_equal. rewrite (v_shift_comm). reflexivity. all: omega.
 }{
 destruct h; unfold h_subs; simpl. auto. f_equal.
 + apply h_shift_subs. assumption.
-+ clear v_shift_subs h_shift_subs.
-  unfold c_subs in c_shift_subs.
-  rewrite <-(v_shift_shift 1), (v_shift_comm_aux 1 j).
-  rewrite (v_shift_comm_aux 1 (1+j)), c_shift_subs. clear c_shift_subs. simpl.
-  do 2 f_equal. all: try omega.
-  rewrite <-(v_shift_shift 1 1 0), (v_shift_comm_aux 1 j).
-  rewrite (v_shift_comm_aux 1 (1+j)). f_equal. 
-  rewrite (v_shift_comm_aux 1 i), (v_shift_comm_aux 1 (1+i)). 
-  do 2 f_equal. all: omega.
++ clear v_shift_subs h_shift_subs. unfold c_subs in c_shift_subs.
+  rewrite <-(v_shift_shift 1), (v_shift_comm 1 j).
+  rewrite (v_shift_comm 1 (1+j)), c_shift_subs. clear c_shift_subs. simpl.
+  do 2 f_equal. all: try omega. 
+  rewrite <-(v_shift_shift 1 1 0), (v_shift_comm 1 j), (v_shift_comm 1 (1+j)).
+  all: f_equal||omega||auto. 
+  rewrite (v_shift_comm 1 i), (v_shift_comm 1 (1+i)). do 2 f_equal. all: omega.
 }
 Qed.
 
 
 Lemma v_negshift_subs v v' i j (safe: j <= i): 
   v_no_var v (1+i) -> v_no_var v' (i) ->
-  Sub.v_negshift (v_subs v v' j) 1 i = 
-  (v_subs (Sub.v_negshift v 1 (1+i)) (Sub.v_negshift v' 1 i) j)
+    Sub.v_negshift (v_subs v v' j) 1 i
+  = (v_subs (Sub.v_negshift v 1 (1+i)) (Sub.v_negshift v' 1 i) j)
+  
 with c_negshift_subs c v' i j (safe: j <= i): 
   c_no_var c (1+i) -> v_no_var v' (i) ->
-  Sub.c_negshift (c_subs c v' j) 1 i = 
-  (c_subs (Sub.c_negshift c 1 (1+i)) (Sub.v_negshift v' 1 i) j)
+    Sub.c_negshift (c_subs c v' j) 1 i
+  = (c_subs (Sub.c_negshift c 1 (1+i)) (Sub.v_negshift v' 1 i) j)
+  
 with h_negshift_subs h v' i j (safe: j <= i): 
   h_no_var h (1+i) -> v_no_var v' (i) ->
-  Sub.h_negshift (h_subs h v' j) 1 i = 
-  (h_subs (Sub.h_negshift h 1 (1+i)) (Sub.v_negshift v' 1 i) j).
+    Sub.h_negshift (h_subs h v' j) 1 i
+  = (h_subs (Sub.h_negshift h 1 (1+i)) (Sub.v_negshift v' 1 i) j).
 Proof.
 {
 intros nov nov'. destruct v; unfold v_subs; simpl.
-{
-  clear v_negshift_subs c_negshift_subs h_negshift_subs.
-  destruct v as (x, n).
-  destruct (n=?j) eqn:nj.
+{ clear v_negshift_subs c_negshift_subs h_negshift_subs.
+  destruct v as (x, n). destruct (n=?j) eqn:nj.
   apply Nat.eqb_eq in nj. subst.
   destruct (1+i <=? j) eqn:cmpij.
-  3 : destruct (1+i <=? n) eqn:Sin.
-  all: simpl.
+  3 : destruct (1+i <=? n) eqn:Sin. all: simpl.
   + apply leb_complete in cmpij.
     assert (j=S i) by omega. subst. omega.
   + simpl in cmpij. rewrite cmpij. simpl.
@@ -945,92 +801,65 @@ intros nov nov'. destruct v; unfold v_subs; simpl.
 }
 all: f_equal; simpl in nov.
 all: try apply v_negshift_subs; try omega || auto.
-5: apply h_negshift_subs; auto; destruct nov; auto.
-+ destruct nov. auto.
-+ destruct nov. auto.
-+ unfold c_subs in c_negshift_subs. rewrite v_shift_comm_aux.
-  rewrite (c_negshift_subs c _ (S i) (S j)). clear c_negshift_subs.
-  do 3 f_equal. rewrite v_shift_comm_aux. f_equal.
-  rewrite v_shift_negshift_1j. all: omega || auto.
-  apply v_no_var_shift. auto. omega.
-+ unfold c_subs in c_negshift_subs. rewrite v_shift_comm_aux. destruct nov.
-  rewrite (c_negshift_subs c _ (S i) (S j)). clear c_negshift_subs.
-  do 3 f_equal. rewrite v_shift_comm_aux. f_equal.
-  rewrite v_shift_negshift_1j. all: omega || auto.
-  apply v_no_var_shift. auto. omega.
+all: try destruct nov; apply h_negshift_subs || auto; auto.
+all: unfold c_subs in c_negshift_subs; rewrite v_shift_comm; try omega.
+all: rewrite (c_negshift_subs c _ (S i) (S j)); clear c_negshift_subs.
+all: omega || (apply v_no_var_shift; omega || auto) || auto.
+all: rewrite v_shift_comm; do 4 f_equal; try rewrite v_shift_negshift_comm.
+all: omega || auto.
 }{
 induction c; intros nov nov'; unfold c_subs; simpl in nov |-*; f_equal;
 try apply v_negshift_subs; try assumption.
 all: clear v_negshift_subs h_negshift_subs.
 all: try (destruct nov; assumption).
 all: unfold c_subs in c_negshift_subs; inv nov.
-+ rewrite <-(v_shift_shift 1), (v_shift_comm_aux 1 j).
-  rewrite (v_shift_comm_aux 1 (1+j)), c_negshift_subs. clear c_negshift_subs. simpl. do 3 f_equal. rewrite <-(v_shift_shift 1 1 0), (v_shift_comm_aux 1 j).
-  rewrite (v_shift_comm_aux 1 (1+j)). f_equal. 
-  rewrite v_shift_shift, v_shift_shift, v_shift_negshift_1j. reflexivity. 
-  all: omega || auto. apply v_no_var_shift. apply v_no_var_shift.
-  auto. omega. omega.
-+ rewrite v_shift_comm_aux. inv H0.
-  rewrite (c_negshift_subs _ _ (S i) (S j)). clear c_negshift_subs.
-  do 3 f_equal. rewrite v_shift_comm_aux. f_equal.
-  rewrite v_shift_negshift_1j. all: omega || auto.
-  apply v_no_var_shift. auto. omega.
-+ rewrite v_shift_comm_aux. inv H0.
-  rewrite (c_negshift_subs _ _ (S i) (S j)). clear c_negshift_subs.
-  do 3 f_equal. rewrite v_shift_comm_aux. f_equal.
-  rewrite v_shift_negshift_1j. all: omega || auto.
-  apply v_no_var_shift. auto. omega.
-+ rewrite v_shift_comm_aux.
-  rewrite (c_negshift_subs _ _ (S i) (S j)). clear c_negshift_subs.
-  do 3 f_equal. rewrite v_shift_comm_aux. f_equal.
-  rewrite v_shift_negshift_1j. all: omega || auto.
-  apply v_no_var_shift. auto. omega.
-+ rewrite <-(v_shift_shift 1), (v_shift_comm_aux 1 j).
-  rewrite (v_shift_comm_aux 1 (1+j)), c_negshift_subs. clear c_negshift_subs. simpl. do 3 f_equal. rewrite <-(v_shift_shift 1 1 0), (v_shift_comm_aux 1 j).
-  rewrite (v_shift_comm_aux 1 (1+j)). f_equal. 
-  rewrite v_shift_shift, v_shift_shift, v_shift_negshift_1j. reflexivity. 
-  all: omega || auto. apply v_no_var_shift. apply v_no_var_shift.
-  auto. omega. omega.
-+ rewrite v_shift_comm_aux.
-  rewrite (c_negshift_subs _ _ (S i) (S j)). clear c_negshift_subs.
-  do 3 f_equal. rewrite v_shift_comm_aux. f_equal.
-  rewrite v_shift_negshift_1j. all: omega || auto.
-  apply v_no_var_shift. auto. omega.
-+ rewrite c_negshift_subs. clear c_negshift_subs.
-  do 3 f_equal. all: omega || auto.
-+ rewrite v_shift_comm_aux.
-  rewrite (c_negshift_subs _ _ (S i) (S j)). clear c_negshift_subs.
-  do 3 f_equal. rewrite v_shift_comm_aux. f_equal.
-  rewrite v_shift_negshift_1j. all: omega || auto.
-  apply v_no_var_shift. auto. omega.
-+ rewrite c_negshift_subs. clear c_negshift_subs.
-  do 3 f_equal. all: omega || auto.
+1:rewrite <-(v_shift_shift 1), (v_shift_comm 1 j); try omega.
+1:rewrite (v_shift_comm 1 (1+j)), c_negshift_subs; omega || auto.
+2:apply v_no_var_shift; omega||apply v_no_var_shift; omega || auto.
+1:clear c_negshift_subs; do 3 f_equal.
+1:rewrite <-(v_shift_shift 1 1 0), (v_shift_comm 1 j), (v_shift_comm 1 (1+j));
+  try omega || f_equal; rewrite v_shift_shift, v_shift_shift.
+1:rewrite v_shift_negshift_comm; omega || auto.
+4:rewrite <-(v_shift_shift 1), (v_shift_comm 1 j); try omega.
+4:rewrite (v_shift_comm 1 (1+j)), c_negshift_subs; omega || auto.
+5:apply v_no_var_shift; omega||apply v_no_var_shift; omega || auto.
+4:clear c_negshift_subs; do 3 f_equal.
+4:rewrite <-(v_shift_shift 1 1 0), (v_shift_comm 1 j), (v_shift_comm 1 (1+j));
+  try omega || f_equal; rewrite v_shift_shift, v_shift_shift.
+4:rewrite v_shift_negshift_comm; omega || auto.
+5:rewrite c_negshift_subs; do 3 f_equal; omega || auto.
+6:rewrite c_negshift_subs; do 3 f_equal; omega || auto.
+all: rewrite v_shift_comm; omega || (try inv H0).
+all: rewrite (c_negshift_subs _ _ (S i) (S j)); clear c_negshift_subs;
+     omega || apply v_no_var_shift || auto; omega || auto.
+all: do 3 f_equal; (rewrite v_shift_comm; try omega) || omega || auto. 
+all: f_equal; try rewrite v_shift_negshift_comm.
+all: omega || auto.
 }{
 destruct h; unfold h_subs; intros nov nov'; simpl. auto. inv nov. f_equal.
 + apply h_negshift_subs; auto.
 + unfold c_subs in c_negshift_subs. clear v_negshift_subs h_negshift_subs.
-  rewrite <-(v_shift_shift 1), (v_shift_comm_aux 1 j). simpl.
-  rewrite (v_shift_comm_aux 1 (1+j)), c_negshift_subs. clear c_negshift_subs. simpl. do 3 f_equal. rewrite <-(v_shift_shift 1 1 0), (v_shift_comm_aux 1 j).
-  rewrite (v_shift_comm_aux 1 (1+j)). f_equal. 
-  rewrite v_shift_shift, v_shift_shift, v_shift_negshift_1j. reflexivity. 
-  all: omega || auto. apply v_no_var_shift. apply v_no_var_shift.
-  auto. omega. omega.
+  rewrite <-(v_shift_shift 1), (v_shift_comm 1 j).
+  rewrite (v_shift_comm 1 (1+j)), c_negshift_subs. clear c_negshift_subs. rewrite <-(v_shift_shift 1 1 0), (v_shift_comm 1 j), (v_shift_comm 1 (1+j)). do 4 f_equal. rewrite v_shift_shift, v_shift_shift, v_shift_negshift_comm.
+  all: try (apply v_no_var_shift; omega||apply v_no_var_shift); omega||auto.
 }
 Qed.
 
 
 Lemma v_sub_subs v i j vi vj:
   j >= i ->
-  Sub.v_sub (v_subs v vi i) (j, vj) = 
-  (v_subs (Sub.v_sub v (1+j, Sub.v_shift vj 1 i)) (Sub.v_sub vi (j, vj)) i)
+    Sub.v_sub (v_subs v vi i) (j, vj)
+  = (v_subs (Sub.v_sub v (1+j, Sub.v_shift vj 1 i)) (Sub.v_sub vi (j, vj)) i)
+
 with c_sub_subs c i j vi vj: 
   j >= i ->
-  Sub.c_sub (c_subs c vi i) (j, vj) = 
-  (c_subs (Sub.c_sub c (1+j, Sub.v_shift vj 1 i)) (Sub.v_sub vi (j, vj)) i)
+    Sub.c_sub (c_subs c vi i) (j, vj)
+  = (c_subs (Sub.c_sub c (1+j, Sub.v_shift vj 1 i)) (Sub.v_sub vi (j, vj)) i)
+
 with h_sub_subs h i j vi vj: 
   j >= i ->
-  Sub.h_sub (h_subs h vi i) (j, vj) = 
-  (h_subs (Sub.h_sub h (1+j, Sub.v_shift vj 1 i)) (Sub.v_sub vi (j, vj)) i).
+    Sub.h_sub (h_subs h vi i) (j, vj)
+  = (h_subs (Sub.h_sub h (1+j, Sub.v_shift vj 1 i)) (Sub.v_sub vi (j, vj)) i).
 Proof.
 {
 intros cmp. induction v; unfold v_subs; simpl.
@@ -1066,26 +895,25 @@ apply Nat.eqb_eq in ni. subst.
 all: f_equal; auto.
 3: apply h_sub_subs; auto.
 all: clear v_sub_subs h_sub_subs; unfold c_subs in c_sub_subs.
-all: rewrite v_shift_comm_aux, c_sub_subs; clear c_sub_subs; try omega.
+all: rewrite v_shift_comm, c_sub_subs; clear c_sub_subs; try omega.
 all: do 2 f_equal; try rewrite <-v_shift_sub; try omega.
-all: try rewrite <-v_shift_comm_aux; try omega; f_equal.
+all: try rewrite <-v_shift_comm; try omega; f_equal.
 }{
 intros cmp. induction c; unfold c_subs; simpl; f_equal; auto.
 all: try apply v_sub_subs; try assumption.
 all: clear v_sub_subs h_sub_subs; unfold c_subs in c_sub_subs.
-all: try rewrite v_shift_comm_aux, c_sub_subs; try omega.
+all: try rewrite v_shift_comm, c_sub_subs; try omega.
 all: do 2 f_equal; try rewrite <-v_shift_sub; try omega.
-all: try rewrite <-v_shift_comm_aux; try omega; f_equal.
-all: rewrite (v_shift_comm_aux _ i); f_equal; try omega.
+all: try rewrite <-v_shift_comm; try omega; f_equal.
+all: rewrite (v_shift_comm _ i); f_equal; try omega.
 all: rewrite v_shift_sub; f_equal; omega.
 }{
 intros cmp. induction h; unfold h_subs; simpl; f_equal; auto.
-unfold c_subs in c_sub_subs. rewrite v_shift_comm_aux, c_sub_subs; try omega.
+unfold c_subs in c_sub_subs. rewrite v_shift_comm, c_sub_subs; try omega.
 do 2 f_equal; try rewrite <-v_shift_sub; try omega.
-all: try rewrite <-v_shift_comm_aux; try omega; f_equal.
-rewrite (v_shift_comm_aux _ i); f_equal; try omega.
-rewrite v_shift_comm_aux. f_equal. rewrite v_shift_sub. f_equal.
+all: try rewrite <-v_shift_comm; try omega; f_equal.
+rewrite (v_shift_comm _ i); f_equal; try omega.
+rewrite v_shift_comm. f_equal. rewrite v_shift_sub. f_equal.
 all: omega.
 }
 Qed.
-
