language_formalisation/syntax/syntax_lemmas.v
@@ -1,13 +1,14 @@
-(* Add LoadPath "C:\Users\Ziga\Documents\Ziga_podatki\PHD\language_formalisation\syntax". *)
-Add LoadPath "E:\Ziga_Podatki\faks\PHD\language_formalisation\syntax".
-Require Export Arith syntax.
+Add LoadPath "C:\Users\Ziga\Documents\Ziga_podatki\PHD\language_formalisation\syntax".
+(* Add LoadPath "E:\Ziga_Podatki\faks\PHD\language_formalisation\syntax". *)
+Require Export syntax.
 Require Import Le Compare_dec.
 
 Ltac inv H := inversion H; clear H; subst.
 
+(* ==================== Ctx Modification ==================== *)
 
 Lemma get_ctx_remove_unchanged Γ i j :
-  i > j -> get_vtype Γ j = get_vtype (ctx_remove_var Γ i) j.
+  i > j -> get_vtype Γ j = get_vtype (ctx_remove Γ i) j.
 Proof.
 revert i j; induction Γ; intros i j lt; auto.
 destruct i; destruct j; simpl; try omega.
@@ -17,7 +18,7 @@ Qed.
 
 
 Lemma get_ctx_remove_changed Γ i j :
-  i <= j -> get_vtype Γ (S j) = get_vtype (ctx_remove_var Γ i) j.
+  i <= j -> get_vtype Γ (S j) = get_vtype (ctx_remove Γ i) j.
 Proof.
 revert i j; induction Γ; intros i j lt; auto.
 destruct i; destruct j; simpl; auto.
@@ -27,14 +28,14 @@ Qed.
 
 
 Lemma ctx_remove_extend Γ i A :
-  CtxU (ctx_remove_var Γ i) A = ctx_remove_var (CtxU Γ A) (1+i).
+  CtxU (ctx_remove Γ i) A = ctx_remove (CtxU Γ A) (1+i).
 Proof.
 revert i; induction Γ; intros i; auto.
 Qed.
 
 
 Lemma get_ctx_insert_unchanged Γ A i j:
-  i < j -> get_vtype Γ i = get_vtype (ctx_insert_var Γ A j) i.
+  i < j -> get_vtype Γ i = get_vtype (ctx_insert Γ A j) i.
 Proof.
 revert i j. induction Γ; intros i j cmp; simpl.
 destruct i; destruct j; simpl; try reflexivity.
@@ -46,15 +47,20 @@ Qed.
 
 
 Lemma get_ctx_insert_changed Γ A i j:
-  i >= j -> get_vtype Γ i = get_vtype (ctx_insert_var Γ A j) (1+i).
+  i >= j -> get_vtype Γ i = get_vtype (ctx_insert Γ A j) (1+i).
 Proof.
 revert i j. induction Γ; intros i j cmp; simpl.
 destruct i; destruct j; simpl; try reflexivity.
-destruct j; destruct i.
-+ auto.
-+ auto.
+destruct j; destruct i; auto.
 + omega.
 + simpl. apply IHΓ. omega.
+Qed.
+
+
+Lemma ctx_insert_extend Γ i A_ins A :
+  CtxU (ctx_insert Γ A_ins i) A = ctx_insert (CtxU Γ A) A_ins (1+i).
+Proof.
+revert i; induction Γ; intros i; auto.
 Qed.
 
 
@@ -62,68 +68,59 @@ Lemma get_join_ctx_tctx Γ Z D i:
   get_vtype Γ i = get_vtype (join_ctx_tctx Γ Z D) (i+tctx_len Z).
 Proof.
 induction Z; simpl. f_equal. omega.
-assert (i + S (tctx_len Z)=S(i+tctx_len Z)) by omega. rewrite H. auto.
+assert (i+S(tctx_len Z)=S(i+tctx_len Z)) by omega. rewrite H. auto.
 Qed.
+
 
 Lemma get_join_ctxs Γ Γ' i:
   get_vtype Γ' i = get_vtype (join_ctxs Γ' Γ) (i+ctx_len Γ).
 Proof.
 induction Γ; simpl. f_equal. omega.
-assert (i + S (ctx_len Γ)=S(i+ctx_len Γ)) by omega. rewrite H. auto.
-Qed.
-
-Lemma ctx_insert_extend Γ i A_ins A :
-  CtxU (ctx_insert_var Γ A_ins i) A = ctx_insert_var (CtxU Γ A) A_ins (1+i).
-Proof.
-revert i; induction Γ; intros i; auto.
+assert (i+S(ctx_len Γ)=S(i+ctx_len Γ)) by omega. rewrite H. auto.
 Qed.
 
 
-Lemma join_ctxs_insert_var Γ1 Γ2 i A :
-  join_ctxs (ctx_insert_var Γ1 A i) Γ2= 
-    ctx_insert_var (join_ctxs Γ1 Γ2) A (ctx_len Γ2 + i). 
+Lemma join_ctxs_insert Γ1 Γ2 i A :
+  join_ctxs (ctx_insert Γ1 A i) Γ2 
+  = ctx_insert (join_ctxs Γ1 Γ2) A (ctx_len Γ2+i). 
 Proof.
 induction Γ2; simpl. auto. f_equal. auto.
 Qed.
 
 
-Lemma join_ctx_tctx_insert_var  Γ Z D i A :
-  join_ctx_tctx (ctx_insert_var Γ A i) Z D = 
-    ctx_insert_var (join_ctx_tctx Γ Z D) A (tctx_len Z + i). 
+Lemma join_ctx_tctx_insert  Γ Z D i A :
+    join_ctx_tctx (ctx_insert Γ A i) Z D 
+  = ctx_insert (join_ctx_tctx Γ Z D) A (tctx_len Z+i). 
 Proof.
 induction Z; simpl. auto. f_equal. auto.
 Qed.
 
-Lemma join_ctxs_remove_var Γ1 Γ2 i:
-  join_ctxs (ctx_remove_var Γ1 i) Γ2= 
-    ctx_remove_var (join_ctxs Γ1 Γ2) (ctx_len Γ2 + i). 
+
+Lemma join_ctxs_remove Γ1 Γ2 i:
+    join_ctxs (ctx_remove Γ1 i) Γ2
+  = ctx_remove (join_ctxs Γ1 Γ2) (ctx_len Γ2 + i). 
 Proof.
 induction Γ2; simpl. auto. f_equal. auto.
 Qed.
 
 
-Lemma join_ctx_tctx_remove_var  Γ Z D i :
-  join_ctx_tctx (ctx_remove_var Γ i) Z D = 
-    ctx_remove_var (join_ctx_tctx Γ Z D) (tctx_len Z + i). 
+Lemma join_ctx_tctx_remove  Γ Z D i :
+    join_ctx_tctx (ctx_remove Γ i) Z D 
+  = ctx_remove (join_ctx_tctx Γ Z D) (tctx_len Z + i). 
 Proof.
 induction Z; simpl. auto. f_equal. auto.
 Qed.
 
+(* ==================== Ctx Guarantees ==================== *)
 
 Lemma ctx_len_get_vtype Γ n :
   (exists A, get_vtype Γ n = Some A) <-> ctx_len Γ > n.
 Proof.
-constructor.
-+ revert n. induction Γ; intros n gets.
-  - simpl in gets. destruct gets. discriminate.
-  - simpl in *. destruct n.
-    * omega.
-    * apply IHΓ in gets. omega.
-+ revert n. induction Γ; intros n gets.
-  - simpl in gets. omega.
-  - simpl in *. destruct n.
-    * eauto.
-    * apply IHΓ. omega.
+constructor; revert n; induction Γ; intros n gets; simpl in *.
+- destruct gets. discriminate.
+- destruct n. omega. apply IHΓ in gets. omega.
+- omega.
+- destruct n. eauto. apply IHΓ. omega.
 Qed.
 
 
@@ -137,17 +134,11 @@ Qed.
 Lemma tctx_len_get_ttype Z n :
   (exists A, get_ttype Z n = Some A) <-> tctx_len Z > n.
 Proof.
-constructor.
-+ revert n. induction Z; intros n gets.
-  - simpl in gets. destruct gets. discriminate.
-  - simpl in *. destruct n.
-    * omega.
-    * apply IHZ in gets. omega.
-+ revert n. induction Z; intros n gets.
-  - simpl in gets. omega.
-  - simpl in *. destruct n.
-    * eauto.
-    * apply IHZ. omega.
+constructor; revert n; induction Z; intros n gets; simpl in *.
+- destruct gets. discriminate.
+- destruct n. omega. apply IHZ in gets. omega.
+- omega.
+- destruct n. eauto. apply IHZ. omega.
 Qed.
 
 
@@ -157,13 +148,12 @@ Proof.
 intro. apply tctx_len_get_ttype. eauto.
 Qed.
 
+(* ==================== Term Properties ==================== *)
 
 Fixpoint v_under_var_weaken v i j:
   v_under_var v j -> j <= i -> v_under_var v i
-
 with c_under_var_weaken c i j:
   c_under_var c j -> j <= i -> c_under_var c i
-
 with h_under_var_weaken h i j:
   h_under_var h j -> j <= i -> h_under_var h i.
 Proof.
@@ -174,7 +164,7 @@ induction v; simpl in orig; simpl; auto.
 + destruct orig. auto.
 + eapply c_under_var_weaken. eauto. omega.
 + destruct orig. constructor. 2: eauto.
-  - eapply c_under_var_weaken. eauto. omega.
+  eapply c_under_var_weaken. eauto. omega.
 }{
 induction c; simpl in orig; simpl; eauto.
 all: destruct orig; constructor; eauto. 2: (destruct H0; constructor).
@@ -194,11 +184,11 @@ with h_under_var_no_var h i j:
   h_under_var h i -> i<=j -> h_no_var h j.
 Proof.
 {
-induction v; intros under cmp; simpl; auto.
-+ destruct v. simpl in under. omega.
-+ simpl in under. inv under. constructor; auto.
-+ simpl in under. eapply c_under_var_no_var. eauto. omega.
-+ simpl in under. inv under. constructor. eapply c_under_var_no_var. eauto.     
+induction v; intros under cmp; simpl; auto; simpl in under.
++ destruct v. omega.
++ inv under. constructor; auto.
++ eapply c_under_var_no_var. eauto. omega.
++ inv under. constructor. eapply c_under_var_no_var. eauto.     
   omega. eapply h_under_var_no_var. eauto. omega.
 }{
 induction c; intros under cmp; simpl; auto.
@@ -212,11 +202,9 @@ inv under. constructor. auto. eapply c_under_var_no_var; eauto; omega.
 }
 Qed.
 
-Lemma find_op_case_no_var h i op x k cop:
-  h_no_var h i -> find_op_case h op = Some (x, k, cop) ->
-  c_no_var cop (2+i).
+Lemma find_case_no_var h i op x k c:
+  h_no_var h i -> find_case h op = Some (x, k, c) -> c_no_var c (2+i).
 Proof.
-intros.
-induction h. simpl in H0. discriminate.
+intros. induction h. simpl in H0. discriminate.
 inv H. simpl in H0. destruct (op==o); try inv H0; auto.
 Qed.
