language_formalisation/type_system/subtyping_lemmas.v
@@ -1,21 +1,20 @@
-(* Add LoadPath "C:\Users\Ziga\Documents\Ziga_podatki\PHD\language_formalisation\syntax". *)
-(* Add LoadPath "C:\Users\Ziga\Documents\Ziga_podatki\PHD\language_formalisation\type_system". *)
-(* Add LoadPath "C:\Users\Ziga\Documents\Ziga_podatki\PHD\language_formalisation\substitution". *)
-Add LoadPath "E:\Ziga_Podatki\faks\PHD\language_formalisation\syntax".
-Add LoadPath "E:\Ziga_Podatki\faks\PHD\language_formalisation\type_system".
-Add LoadPath "E:\Ziga_Podatki\faks\PHD\language_formalisation\substitution".
+Add LoadPath "C:\Users\Ziga\Documents\Ziga_podatki\PHD\language_formalisation\syntax".
+Add LoadPath "C:\Users\Ziga\Documents\Ziga_podatki\PHD\language_formalisation\type_system".
+Add LoadPath "C:\Users\Ziga\Documents\Ziga_podatki\PHD\language_formalisation\substitution".
+(* Add LoadPath "E:\Ziga_Podatki\faks\PHD\language_formalisation\syntax". *)
+(* Add LoadPath "E:\Ziga_Podatki\faks\PHD\language_formalisation\type_system". *)
+(* Add LoadPath "E:\Ziga_Podatki\faks\PHD\language_formalisation\substitution". *)
 
-Require Import declarational wf_lemmas.
+Require Export declarational wf_lemmas.
 
 
 Ltac inv H := inversion H; clear H; subst.
 Ltac aconstructor := constructor; auto.
 
 
-(* ========================== Auxiliary Lemmas ========================== *)
+(* ==================== Sig and Eqs Properties ==================== *)
 
-
-Lemma sig_subtype_gets_Some Σ Σ' op A B :
+Lemma sig_subtype_get_Some Σ Σ' op A B :
   sig_subtype Σ Σ' -> get_op_type Σ op = Some (A, B) -> exists A' B', 
   get_op_type Σ' op = Some (A', B') /\ vsubtype A A' /\ vsubtype B' B.
 Proof.
@@ -31,14 +30,13 @@ Lemma sig_subtype_extend Σ Σ' op A B :
 Proof.
 intros. induction H.
 + apply SubtypeSigØ.
-+ eapply SubtypeSigU; eauto.
-  inv H0. simpl. destruct (op0 == op). 
-  * rewrite e in *. rewrite H1 in H9. discriminate.
-  * assumption.
++ eapply SubtypeSigU; eauto. inv H0. simpl.
+  destruct (op0 == op); auto. rewrite e in *. rewrite H1 in H9. discriminate.
 Qed.
 
 
-Lemma sig_subtype_empty Σ : sig_subtype Σ SigØ -> Σ = SigØ.
+Lemma sig_subtype_empty Σ : 
+  sig_subtype Σ SigØ -> Σ = SigØ.
 Proof.
 intro subty. inv subty. reflexivity. simpl in *. discriminate.
 Qed.
@@ -55,22 +53,20 @@ Qed.
 
 
 Lemma eqs_subtype_contains E E' Γ Z T1 T2 :
-  eqs_subtype E E' -> eqs_contain_eq E Γ Z T1 T2 -> 
-  eqs_contain_eq E' Γ Z T1 T2.
+  eqs_subtype E E' -> has_eq E Γ Z T1 T2 -> 
+  has_eq E' Γ Z T1 T2.
 Proof.
-intros sty gets. induction sty; simpl in gets; destruct gets.
-+ destruct H0 as [a [b [c ]]]. subst. assumption.
-+ auto.
+intros sty gets. induction sty; simpl in gets; destruct gets; auto.
+destruct H0 as [a [b [c ]]]. subst. assumption.
 Qed.
 
 Lemma eqs_subtype_empty E E': 
   eqs_subtype E E' -> E' = EqsØ -> E = EqsØ.
 Proof.
-intros subty eq. induction subty. reflexivity.
-subst. simpl in H. destruct H.
+intros subty eq. induction subty. auto. subst. simpl in H. destruct H.
 Qed.
 
-(* ========================== Basic Properties ========================== *)
+(* ==================== Reflexivity and Transitivity ==================== *)
 
 Lemma vsubtype_refl v : wf_vtype v -> vsubtype v v
 with csubtype_refl c : wf_ctype c -> csubtype c c
@@ -78,52 +74,42 @@ with sig_subtype_refl Σ : wf_sig Σ -> sig_subtype Σ Σ
 with eqs_subtype_refl E Σ : wf_eqs E Σ -> eqs_subtype E E
 with ctx_subtype_refl Γ : wf_ctx Γ -> ctx_subtype Γ Γ.
 Proof.
-{intros; induction v; inv H.
+{intros; destruct v; inv H.
 + apply SubtypeUnit.
 + apply SubtypeInt.
 + apply SubtypeTyØ.
 + apply SubtypeTyΣ; auto.
 + apply SubtypeTyΠ; auto.
-+ apply SubtypeTyFun. apply IHv. assumption. apply csubtype_refl. assumption.
-+ apply SubtypeTyHandler; apply csubtype_refl; assumption.
-}{ destruct c. intros. inv H. apply SubtypeCTy.
-apply vsubtype_refl. assumption. 
-apply sig_subtype_refl. assumption.
-eapply eqs_subtype_refl. eauto.
-}{ 
++ apply SubtypeTyFun; auto.
++ apply SubtypeTyHandler; auto. }
+{
+ destruct c. intros. inv H. apply SubtypeCTy; eauto. }
+{ 
 intros; induction Σ.
 + apply SubtypeSigØ.
-+ eapply SubtypeSigU.
-  - apply sig_subtype_extend. apply IHΣ. inv H. assumption. assumption.
-  - simpl. destruct (o==o). reflexivity. destruct n. reflexivity.
-  - apply vsubtype_refl. inv H. assumption.
-  - apply vsubtype_refl. inv H. assumption.
++ eapply SubtypeSigU; inv H; eauto.
+  - apply sig_subtype_extend. auto. apply WfSigU; auto.
+  - simpl. destruct (o==o); try destruct n; auto.
 }{induction E; intros.
 + apply SubtypeEqsØ.
-+ apply SubtypeEqsU. inv H. eapply eqs_subtype_extend. 
-  - apply IHE. assumption.
++ apply SubtypeEqsU. inv H. eapply eqs_subtype_extend; auto. 
   - apply WfEqsU; eauto.
   - simpl. left. auto.
 }
 {clear csubtype_refl sig_subtype_refl eqs_subtype_refl ctx_subtype_refl.
 induction Γ; intros.
 apply SubtypeCtxØ.
-apply SubtypeCtxU; inv H. apply IHΓ. assumption. 
-apply vsubtype_refl. assumption.
+apply SubtypeCtxU; inv H; auto.
 }
 Qed.
 
 
-
-Fixpoint eqs_subtype_trans E1 E2 E3  
-  (E12 : eqs_subtype E1 E2) {struct E12} : 
+Fixpoint eqs_subtype_trans E1 E2 E3 (E12 : eqs_subtype E1 E2) {struct E12} : 
   eqs_subtype E2 E3 -> eqs_subtype E1 E3.
 Proof.
 intros E23. destruct E12.
 apply SubtypeEqsØ.
-eapply SubtypeEqsU.
-+ eapply eqs_subtype_trans; eauto.
-+ eapply eqs_subtype_contains; eauto.
+eapply SubtypeEqsU; eauto; eapply eqs_subtype_contains; eauto.
 Qed.
 
 
@@ -154,8 +140,8 @@ Proof.
 {
 clear sig_subtype_trans sig_subtype_trans_rev get_op_trans.
 intros A23; destruct A12; try assumption; inv A23. 
-+ apply SubtypeTyΣ; eapply vsubtype_trans; eauto.
-+ apply SubtypeTyΠ; eapply vsubtype_trans; eauto.
++ apply SubtypeTyΣ; eauto.
++ apply SubtypeTyΠ; eauto.
 + apply SubtypeTyFun.
   - eapply vsubtype_trans_rev; eauto. 
   - eapply csubtype_trans; eauto.
@@ -191,7 +177,7 @@ intros C32; destruct C21. inv C32. apply SubtypeCTy.
 clear csubtype_trans csubtype_trans_rev sig_subtype_trans_rev.
 intros S23. destruct S12.
 { apply SubtypeSigØ. }
-apply (sig_subtype_gets_Some Σ' Σ3) in H as H'.
+apply (sig_subtype_get_Some Σ' Σ3) in H as H'.
 destruct H' as [A'' [B'' [g]]]. eapply SubtypeSigU.
 2 : exact g. all: try assumption.
 + eapply sig_subtype_trans; eauto.
@@ -216,15 +202,15 @@ inv S32. simpl in *. destruct (o==op).
 }{
 clear csubtype_trans csubtype_trans_rev.
 clear sig_subtype_trans sig_subtype_trans_rev get_op_trans.
-intros. revert H. induction S12; intros gets.
-simpl in gets. discriminate.
-simpl in *. destruct (op==op0). 2: auto. inv gets.
+intros. revert H. induction S12; intros gets; simpl in *. discriminate.
+destruct (op==op0). 2: auto. inv gets.
 exists A'0. exists B'0. aconstructor. constructor.
 - eapply vsubtype_trans_rev; eauto.
 - eapply vsubtype_trans; eauto.
 }
 Qed.
 
+(* ==================== Context Properties ==================== *)
 
 Fixpoint ctx_subtype_get Γ Γ' A num (csty : ctx_subtype Γ Γ') {struct csty}:
   get_vtype Γ num = Some A -> 
@@ -232,9 +218,8 @@ Fixpoint ctx_subtype_get Γ Γ' A num (csty : ctx_subtype Γ Γ') {struct csty}:
 Proof.
 revert num. induction csty. clear ctx_subtype_get.
 + intros num H. simpl in H. discriminate.
-+ intros num get. destruct num.
-  - clear IHcsty. simpl in *. inv get. exists A'. auto.
-  - simpl in *. eapply IHcsty. assumption.
++ intros num get. destruct num; eauto.
+  clear IHcsty. simpl in *. inv get. exists A'. auto.
 Qed.
 
 
@@ -244,18 +229,16 @@ Fixpoint ctx_subtype_get_rev Γ Γ' A num (csty : ctx_subtype Γ' Γ) {struct cs
 Proof.
 revert num. induction csty. clear ctx_subtype_get_rev.
 + intros num H. simpl in H. discriminate.
-+ intros num get. destruct num.
-  - clear IHcsty. simpl in *. inv get. exists A0. auto.
-  - simpl in *. eapply IHcsty. exact get.
++ intros num get. destruct num; eauto.
+  clear IHcsty. simpl in *. inv get. exists A0. auto.
 Qed.
+
 
 Lemma ctx_subtype_join_ctxs Γ1 Γ1' Γ2 Γ2':
   ctx_subtype Γ1 Γ1' -> ctx_subtype Γ2 Γ2' ->
   ctx_subtype (join_ctxs Γ1 Γ2) (join_ctxs Γ1' Γ2').
 Proof.
-intros sty1 sty2.
-induction sty2; simpl. assumption.
-apply SubtypeCtxU; assumption. 
+intros sty1 sty2. induction sty2; auto. apply SubtypeCtxU; assumption. 
 Qed.
 
 
@@ -263,16 +246,16 @@ Lemma ctx_subtype_join_ctx_tctx Γ Γ' Z D:
   ctx_subtype Γ Γ' -> wf_tctx Z -> wf_ctype D ->
   ctx_subtype (join_ctx_tctx Γ Z D) (join_ctx_tctx Γ' Z D).
 Proof.
-intros sty wfZ wfD.
-induction Z; simpl. assumption.
-inv wfZ. apply SubtypeCtxU. auto.  apply vsubtype_refl.
-apply WfTyFun; assumption. 
+intros sty wfZ wfD. induction Z; auto.
+inv wfZ. apply SubtypeCtxU. auto. apply vsubtype_refl. apply WfTyFun; auto. 
 Qed.
 
 
 Lemma ctx_subtype_len Γ Γ':
   ctx_subtype Γ Γ' -> ctx_len Γ = ctx_len Γ'.
-Proof. intro sty. induction sty; simpl; auto. Qed. 
+Proof. 
+intro sty. induction sty; simpl; auto. 
+Qed. 
 
 
 Fixpoint ctx_subtype_vtype Γ Γ' v A (types : has_vtype Γ v A) {struct types}:
@@ -284,8 +267,7 @@ with ctx_subtype_ctype Γ Γ' c C (types : has_ctype Γ c C ) {struct types}:
 with ctx_subtype_htype Γ Γ' h Σ D (types : has_htype Γ h Σ D) {struct types}:
   wf_ctx Γ' -> ctx_subtype Γ' Γ -> has_htype Γ' h Σ D
 
-with ctx_subtype_respects Γ Γ' h Σ D E 
-  (types : respects Γ h Σ D E) {struct types}:
+with ctx_subtype_respects Γ Γ' h Σ D E (r : respects Γ h Σ D E) {struct r}:
   wf_ctx Γ' -> ctx_subtype Γ' Γ -> respects Γ' h Σ D E
 
 with ctx_subtype_veq Γ Γ' A v1 v2 (equals : veq A Γ v1 v2) {struct equals}:
@@ -303,17 +285,15 @@ destruct types. induction H1; apply TypeV; try assumption.
 + apply (ctx_subtype_get_rev _ _ A n) in ctxsty.
   destruct ctxsty as [A' [gets]]. 2: assumption. 
   eapply TypeVSubtype. 2: eauto.
-  apply TypeV. assumption. apply ctx_gets_wf in gets as wfA'; eauto.
+  apply TypeV. assumption. apply get_vtype_wf in gets as wfA'; eauto.
   apply TypeVar. assumption.
 + apply TypePair; apply (ctx_subtype_vtype Γ Γ'); assumption.
 + apply TypeInl. apply (ctx_subtype_vtype Γ Γ'); assumption.
 + apply TypeInr. apply (ctx_subtype_vtype Γ Γ'); assumption.
-+ apply TypeFun. eapply ctx_subtype_ctype; inv H0.
-  - exact H1.
++ apply TypeFun. eapply ctx_subtype_ctype; inv H0. eauto.
   - apply WfCtxU; assumption.
   - apply SubtypeCtxU. assumption. apply vsubtype_refl. assumption.
-+ apply TypeHandler. eapply ctx_subtype_ctype; inv H0; inv H6.
-  - exact H1.
++ apply TypeHandler. eapply ctx_subtype_ctype; inv H0; inv H6. eauto.
   - apply WfCtxU; assumption.
   - apply SubtypeCtxU. assumption. apply vsubtype_refl. assumption.
   - eapply (ctx_subtype_htype Γ Γ'); assumption.
@@ -324,16 +304,15 @@ destruct types. induction H1; apply TypeV; try assumption.
 clear ctx_subtype_respects ctx_subtype_veq ctx_subtype_ceq.
 intros wf ctxsty.
 destruct types. induction H1; apply TypeC; try assumption.
-+ apply TypeRet. eapply (ctx_subtype_vtype Γ Γ'); assumption.
-+ apply TypeAbsurd. eapply (ctx_subtype_vtype Γ Γ'); assumption.
++ apply TypeRet. eauto.
++ apply TypeAbsurd. eauto.
 + eapply TypeΠMatch.
   - eapply (ctx_subtype_vtype Γ Γ'); eauto.
   - eapply ctx_subtype_ctype. exact H2. all: inv H2; inv H3; inv H7.
     * apply WfCtxU. apply WfCtxU. all: assumption.
     * apply SubtypeCtxU. apply SubtypeCtxU. assumption.
       all: apply vsubtype_refl; assumption.
-+ eapply TypeΣMatch.
-  - eauto.
++ eapply TypeΣMatch. eauto.
   - eapply ctx_subtype_ctype. exact H2. all: inv H2; inv H4. 
     * apply WfCtxU; assumption.
     * apply SubtypeCtxU. exact ctxsty. apply vsubtype_refl. assumption.
@@ -342,22 +321,20 @@ destruct types. induction H1; apply TypeC; try assumption.
     * apply SubtypeCtxU. exact ctxsty. apply vsubtype_refl. assumption.
 + eapply TypeDoBind.
   - eapply ctx_subtype_ctype; eauto.
-  - inv H1. inv H4. eapply ctx_subtype_ctype.
-    * eauto.
+  - inv H1. inv H4. eapply ctx_subtype_ctype. eauto.
     * apply WfCtxU; assumption.
     * apply SubtypeCtxU. exact ctxsty. apply vsubtype_refl. assumption.
 + eapply TypeApp; eauto.
 + eapply TypeHandle; eauto.
 + eapply TypeLetRec.
-  - eapply ctx_subtype_ctype. exact H1. all: inv H2; inv H3.
+  - eapply ctx_subtype_ctype. eauto. all: inv H2; inv H3.
     * apply WfCtxU. apply WfCtxU. eauto. inv H8. all: eauto.
     * apply SubtypeCtxU. apply SubtypeCtxU. exact ctxsty.
       apply vsubtype_refl. inv H8. assumption. apply vsubtype_refl. assumption.
-  - eapply ctx_subtype_ctype. exact H2. all: inv H2; inv H3.
+  - eapply ctx_subtype_ctype. eauto. all: inv H2; inv H3.
     * apply WfCtxU; assumption.
     * apply SubtypeCtxU. exact ctxsty. apply vsubtype_refl. assumption.
-+ eapply TypeOp.
-  exact H1. eapply ctx_subtype_vtype. exact H2. assumption. assumption.
++ eapply TypeOp. eauto. eapply ctx_subtype_vtype; eauto.
   eapply ctx_subtype_ctype. exact H3. all: inv H3; inv H4.
   - apply WfCtxU; assumption.
   - apply SubtypeCtxU. assumption. apply vsubtype_refl. assumption.
@@ -378,15 +355,13 @@ destruct types. induction H2; apply TypeH; try assumption.
 }{
 clear ctx_subtype_vtype ctx_subtype_ctype ctx_subtype_htype ctx_subtype_veq.
 intros wf ctxsty.
-inv types. eapply Respects; auto. destruct H3.
+inv r. eapply Respects; auto. destruct H3.
 + eapply RespectEqsØ.
-+ eapply RespectEqsU.
-  - eapply ctx_subtype_respects; eauto.
-  - clear ctx_subtype_respects.
-    eapply ctx_subtype_ceq. eauto.
-    apply join_ctx_tctx_wf. apply join_ctxs_wf. all: inv H2; auto. 
-    apply ctx_subtype_join_ctx_tctx. apply ctx_subtype_join_ctxs.
-    all: try assumption. all: apply ctx_subtype_refl; assumption.
++ eapply RespectEqsU; eauto.
+  eapply ctx_subtype_ceq. eauto.
+  apply join_ctx_tctx_wf. apply join_ctxs_wf. all: inv H2; auto. 
+  apply ctx_subtype_join_ctx_tctx. apply ctx_subtype_join_ctxs. 
+  all: assumption || apply ctx_subtype_refl; assumption.
 }{
 inv equals. inv H1.
 }{
@@ -395,7 +370,7 @@ inv equals. inv H1.
 Qed.
 
 
-(* ========================== Subtype Shapes ========================== *)
+(* ==================== Subtype Shapes ==================== *)
 
 Lemma subtype_shape_empty A : vsubtype A TyØ -> A = TyØ.
 Proof.
@@ -451,40 +426,38 @@ intro orig. inv orig. exists C'. exists D'. auto.
 Qed.
 
 Lemma subtype_shape_cty A Σ E C : csubtype C (CTy A Σ E) ->
-  exists A' Σ' E', C = CTy A' Σ' E' /\ vsubtype A' A 
-    /\ sig_subtype Σ' Σ /\ eqs_subtype E' E.
+  exists A' Σ' E', 
+    C = CTy A' Σ' E' /\ vsubtype A' A /\ sig_subtype Σ' Σ /\ eqs_subtype E' E.
 Proof.
 intro orig. inv orig. exists A0. exists Σ0. exists E0. auto.
 Qed.
   
 Lemma subtype_shape_cty_rev A Σ E C : csubtype (CTy A Σ E) C ->
-  exists A' Σ' E', C = CTy A' Σ' E' /\ vsubtype A A' 
-    /\ sig_subtype Σ Σ' /\ eqs_subtype E E'.
+  exists A' Σ' E', C = 
+    CTy A' Σ' E' /\ vsubtype A A' /\ sig_subtype Σ Σ' /\ eqs_subtype E E'.
 Proof.
 intro orig. inv orig. exists A'. exists Σ'. exists E'. auto.
 Qed.
 
+(* ==================== Template WF Subtyping ==================== *)
 
-(* ========================== WF Subtyping ========================== *)
-
-Lemma tmpl_wf_subtype_sig Γ Γ' Z T Σ Σ':
-  wf_tmpl Γ Z T Σ -> sig_subtype Σ Σ' -> ctx_subtype Γ' Γ 
-  -> wf_sig Σ' -> wf_ctx Γ'
-  -> wf_tmpl Γ' Z T Σ'.
+Lemma wf_t_subtype_sig Γ Γ' Z T Σ Σ':
+  wf_t Γ Z T Σ -> sig_subtype Σ Σ' -> 
+  ctx_subtype Γ' Γ -> wf_sig Σ' -> wf_ctx Γ' ->
+  wf_t Γ' Z T Σ'.
 Proof.
 intros orig. revert Γ'. induction orig; intros Γ' sty cty wfs wfc.
 + eapply WfTApp. eapply ctx_subtype_vtype; eauto. assumption.
 + eapply WfTAbsurd. eapply ctx_subtype_vtype; eauto.
 + eapply WfTΠMatch. eapply ctx_subtype_vtype; eauto. inv H. inv H1.
   apply IHorig; auto. apply SubtypeCtxU. 
-  apply SubtypeCtxU. 4: apply WfCtxU. 4: apply WfCtxU. all: auto.
-  all: apply vsubtype_refl; auto.
+  apply SubtypeCtxU. 4: apply WfCtxU. 4: apply WfCtxU.
+  all: assumption || apply vsubtype_refl; auto.
 + eapply WfTΣMatch. eapply ctx_subtype_vtype; eauto.  all: inv H; inv H1.
   apply IHorig1; auto. 3: apply IHorig2; auto.
-  1: apply SubtypeCtxU. 4: apply SubtypeCtxU.
-  3: apply WfCtxU. 7: apply WfCtxU. all: auto.
-  all: apply vsubtype_refl; auto.
-+ eapply sig_subtype_gets_Some in H. 2: exact sty.
+  1: apply SubtypeCtxU. 4: apply SubtypeCtxU. 3: apply WfCtxU. 7: apply WfCtxU.
+  all: assumption || apply vsubtype_refl; auto.
++ eapply sig_subtype_get_Some in H. 2: exact sty.
   destruct H as [A'[B'[gets'[Asty]]]].
   eapply WfTOp. eauto.
   - eapply ctx_subtype_vtype; eauto. apply TypeV.
@@ -500,23 +473,21 @@ Lemma wf_eqs_sig_subtype E Σ Σ':
   wf_eqs E Σ -> sig_subtype Σ Σ' -> wf_sig Σ' -> wf_eqs E Σ'.
 Proof.
 intros. induction H. apply WfEqsØ.
-apply WfEqsU; auto. all: eapply tmpl_wf_subtype_sig; eauto.
+apply WfEqsU; auto. all: eapply wf_t_subtype_sig; eauto.
 all: apply ctx_subtype_refl; auto.
 Qed.
 
-(* ========================== Respects Subtypes ========================== *)
+(* ==================== Respects Subtypes ==================== *)
 
-Lemma contains_respects Γ h Σ D E Γ' Z T1 T2:
-  respects Γ h Σ D E -> eqs_contain_eq E Γ' Z T1 T2 ->
+Lemma has_eq_respects Γ h Σ D E Γ' Z T1 T2:
+  respects Γ h Σ D E -> has_eq E Γ' Z T1 T2 ->
   ceq D (join_ctx_tctx (join_ctxs Γ Γ') Z D)
-    (handle_tmpl (ctx_len Γ') (tctx_len Z) h T1)
-    (handle_tmpl (ctx_len Γ') (tctx_len Z) h T2).
+    (handle_t (ctx_len Γ') (tctx_len Z) h T1)
+    (handle_t (ctx_len Γ') (tctx_len Z) h T2).
 Proof.
-intros r c. induction E.
-+ simpl in c. destruct c.
-+ simpl in c. destruct c.
-  - destruct H as [a[b[c]]]. subst. inv r. inv H3. assumption.
-  - apply IHE. inv r. inv H4. all: assumption.
+intros r c. induction E; simpl in c; destruct c.
+- destruct H as [a[b[c]]]. subst. inv r. inv H3. assumption.
+- apply IHE. inv r. inv H4. all: assumption.
 Qed.
 
 
@@ -527,13 +498,10 @@ Proof.
 intros. induction H1.
 + inv H; apply Respects; auto. apply RespectEqsØ.
 + apply Respects; try (inv H; assumption). 
-  apply RespectEqsU. inv H0. apply IHeqs_subtype; auto.
-  eapply contains_respects; eauto.
+  apply RespectEqsU. inv H0. auto. eapply has_eq_respects; eauto.
 Qed.
   
-
-(* ========================== Value Shapes ========================== *)
-
+(* ==================== Value Shapes ==================== *)
 
 (* Var *)
 Fixpoint shape_var_full Γ v x n A (orig : has_vtype Γ v A) {struct orig} :
@@ -543,12 +511,10 @@ Proof.
 intros same.
 destruct orig. destruct H1; try discriminate.
 + clear shape_var_full.
-  exists A. inv same.
-  aconstructor. apply vsubtype_refl. assumption.
+  exists A. inv same. aconstructor. apply vsubtype_refl. assumption.
 + subst. eapply shape_var_full in H1. clear shape_var_full. 2: reflexivity.
   destruct H1 as [A'' [gets]].
-  exists A''. aconstructor.
-  eapply vsubtype_trans. exact H1. assumption.
+  exists A''. aconstructor. eapply vsubtype_trans; eauto.
 Qed.
 
 
@@ -556,13 +522,11 @@ Lemma shape_var Γ x n A:
   has_vtype Γ (Var (x, n)) A -> 
   (exists A', get_vtype Γ n = Some A' /\ vsubtype A' A).
 Proof.
-intro orig.
-apply (shape_var_full _ _ x n A) in orig as shape. 2: reflexivity.
-assumption.
+intro orig. apply (shape_var_full _ _ x n A) in orig as shape; eauto.
 Qed.
 
 
-Lemma shape_var_empty_ctx id A:
+Lemma shape_var_ctx_empty id A:
   has_vtype CtxØ (Var id) A -> False.
 Proof.
 intro orig. destruct id as (x, n).
@@ -576,18 +540,15 @@ Fixpoint shape_empty_full Γ v A (orig : has_vtype Γ v A) {struct orig} :
   A = TyØ -> (exists x n, v = Var (x, n)).
 Proof.
 intros samety.
-destruct orig. destruct H1; try discriminate.
-+ clear shape_empty_full. exists x. exists n. reflexivity.
-+ subst. apply subtype_shape_empty in H2. subst.
-  eapply shape_empty_full in H1; auto.
+destruct orig. destruct H1; try discriminate. eauto.
+subst. apply subtype_shape_empty in H2. subst; eauto.
 Qed.
 
 
 Lemma shape_empty Γ v:
   has_vtype Γ v TyØ -> (exists x num, v = Var (x, num)).
 Proof.
-intro orig.
-apply (shape_empty_full _ _) in orig as shape; auto.
+intro orig. apply (shape_empty_full _ _) in orig as shape; auto.
 Qed.
 
 
@@ -599,19 +560,17 @@ Fixpoint shape_prod_full Γ v A B ty (orig : has_vtype Γ v ty) {struct orig} :
 Proof.
 intros same.
 destruct orig. destruct H1; try discriminate.
-+ clear shape_prod_full. left. exists x. exists n. reflexivity.
-+ clear shape_prod_full. right. inv same.
-  exists v1. exists v2. auto.
++ left. eauto.
++ right. inv same. eauto.
 + rewrite same in H2. apply subtype_shape_prod in H2. 
-  destruct H2 as [A'' [B'' [pity]]]. subst. 
+  destruct H2 as [A'' [B'' [pity]]]. subst.
   apply (shape_prod_full _ _ A'' B'') in H1. clear shape_prod_full. 
   2: reflexivity. destruct H1. auto.
   right. destruct H1 as [v1 [v2]].
   exists v1. exists v2. destruct H1 as [s[vty1]]. destruct H2.
-  aconstructor. inv H0. constructor;
-  apply TypeV; try assumption; eapply TypeVSubtype; eauto.
+  aconstructor. inv H0. constructor; apply TypeV.
+  all: assumption || eapply TypeVSubtype; eauto.
 Qed.
-
 
 
 Fixpoint shape_pair_full Γ v v1 v2 ty (orig : has_vtype Γ v ty) {struct orig} :
@@ -621,12 +580,10 @@ Proof.
 intros same.
 destruct orig. destruct H1; try discriminate.
 + clear shape_pair_full. exists A. exists B. inv same. auto.
-+ subst.
-  apply (shape_pair_full _ _ v1 v2) in H1. clear shape_pair_full. 
++ subst. apply (shape_pair_full _ _ v1 v2) in H1. clear shape_pair_full. 
   2: reflexivity. destruct H1 as [A''[B''[ty[tyv1]]]]. subst.
   apply subtype_shape_prod_rev in H2. destruct H2 as [A'''[B'''[s[sty1]]]].
-  exists A'''. exists B'''. subst. inv H0.
-  aconstructor. constructor;
+  exists A'''. exists B'''. subst. inv H0. aconstructor. constructor;
   apply TypeV; try assumption; eapply TypeVSubtype; eauto.
 Qed.
 
@@ -652,32 +609,29 @@ Fixpoint shape_sum_full Γ v A B ty (orig : has_vtype Γ v ty) {struct orig} :
 Proof.
 intros same.
 destruct orig. destruct H1; try discriminate.
-+ clear shape_sum_full. left. exists x. exists n. reflexivity.
-+ clear shape_sum_full. right. left. exists v. inv same. auto.
-+ clear shape_sum_full. right. right. exists v. inv same. auto.
++ left. eauto.
++ right. left. inv same. eauto.
++ right. right. inv same. eauto.
 + rewrite same in H2. apply subtype_shape_sum in H2. 
-  destruct H2 as [A'' [B'' [sigty]]]. subst.
-  inv H0. destruct H2. 
+  destruct H2 as [A'' [B'' [sigty]]]. subst. inv H0. destruct H2. 
   apply (shape_sum_full _ _ A'' B'') in H1. clear shape_sum_full. 
-  2: reflexivity. destruct H1. auto. right.
-  do 3 destruct H1; subst.
+  2: reflexivity. destruct H1. auto. right. do 3 destruct H1; subst.
   * left. exists x. aconstructor.
     apply TypeV; try assumption. eapply TypeVSubtype; eauto.
   * right. exists x. aconstructor.
     apply TypeV; try assumption. eapply TypeVSubtype; eauto.
 Qed.
 
+
 Fixpoint shape_inl_full Γ v A v' (orig : has_vtype Γ v A) {struct orig} :
   v = Inl v' ->
   (exists A' B', A = TyΣ A' B' /\ has_vtype Γ v' A').
 Proof.
-intros same.
-destruct orig. destruct H1; try discriminate.
-+ exists A. exists B. inv same. auto.
+intros same. destruct orig. destruct H1; try discriminate.
++ inv same. eauto.
 + inv same. eapply shape_inl_full in H1. 2: reflexivity.
-  destruct H1 as [A''[B''[tysum]]]. subst.
-  apply subtype_shape_sum_rev in H2.
-  destruct H2 as [A'''[B'''[tysum]]]. subst.
+  destruct H1 as [A''[B''[tysum]]]. subst. 
+  apply subtype_shape_sum_rev in H2. destruct H2 as [A'''[B'''[tysum]]]. subst.
   exists A'''. exists B'''. aconstructor. inv H0. destruct H2.
   apply TypeV; auto. eapply TypeVSubtype; eauto.
 Qed.
@@ -686,13 +640,11 @@ Fixpoint shape_inr_full Γ v A v' (orig : has_vtype Γ v A) {struct orig} :
   v = Inr v' ->
   (exists A' B', A = TyΣ A' B' /\ has_vtype Γ v' B').
 Proof.
-intros same.
-destruct orig. destruct H1; try discriminate.
-+ exists A. exists B. inv same. auto.
+intros same. destruct orig. destruct H1; try discriminate.
++ inv same. eauto.
 + inv same. eapply shape_inr_full in H1. 2: reflexivity.
   destruct H1 as [A''[B''[tysum]]]. subst.
-  apply subtype_shape_sum_rev in H2.
-  destruct H2 as [A'''[B'''[tysum]]]. subst.
+  apply subtype_shape_sum_rev in H2. destruct H2 as [A'''[B'''[tysum]]]. subst.
   exists A'''. exists B'''. aconstructor. inv H0. destruct H2.
   apply TypeV; auto. eapply TypeVSubtype; eauto.
 Qed.
@@ -701,8 +653,7 @@ Qed.
 Lemma shape_sum_inl Γ v A B :
   has_vtype Γ (Inl v) (TyΣ A B) -> has_vtype Γ v A.
 Proof.
-intro orig.
-apply (shape_sum_full _ _ A B) in orig as shape. 2: reflexivity.
+intro orig. apply (shape_sum_full _ _ A B) in orig as shape. 2: reflexivity.
 destruct shape.
 + destruct H as [x [n]]. discriminate.
 + destruct H; destruct H; destruct H; inv H. auto.
@@ -712,28 +663,26 @@ Qed.
 Lemma shape_sum_inr Γ v A B :
   has_vtype Γ (Inr v) (TyΣ A B) -> has_vtype Γ v B.
 Proof.
-intro orig.
-apply (shape_sum_full _ _ A B) in orig as shape. 2: reflexivity.
+intro orig. apply (shape_sum_full _ _ A B) in orig as shape. 2: reflexivity.
 destruct shape.
 + destruct H as [x [n]]. discriminate.
 + destruct H; destruct H; destruct H; inv H. auto.
 Qed.
+
 
 (* Function *)
 Fixpoint shape_fun_full Γ v x c ty (orig : has_vtype Γ v ty) {struct orig} :
   v = Fun x c ->
   (exists A C, ty = TyFun A C /\ has_ctype (CtxU Γ A) c C).
 Proof.
-intros same.
-destruct orig. destruct H1; try discriminate.
-+ clear shape_fun_full. exists A. exists C. inv same. auto.
+intros same. destruct orig. destruct H1; try discriminate.
++ inv same. eauto.
 + subst. apply (shape_fun_full _ _ x c) in H1. clear shape_fun_full. 
   2: reflexivity. destruct H1 as [A''[C''[s]]]. subst.
   apply subtype_shape_fun_rev in H2. destruct H2 as [A'''[C'''[s[vty1]]]].
   exists A'''. exists C'''. aconstructor. subst. inv H0.
-  apply TypeC.
+  apply TypeC; auto.
   * apply WfCtxU; assumption.
-  * assumption.
   * eapply TypeCSubtype. 2: eauto.
     eapply ctx_subtype_ctype. eauto. apply WfCtxU; assumption.
     apply SubtypeCtxU. apply ctx_subtype_refl. all: assumption.
@@ -744,31 +693,25 @@ Fixpoint shape_tyfun_full Γ v A C ty (orig : has_vtype Γ v ty) {struct orig} :
   (exists x n, v = Var (x, n)) \/
   (exists x c, v = Fun x c /\ has_ctype (CtxU Γ A) c C).
 Proof.
-intros same.
-destruct orig. destruct H1; try discriminate.
-+ clear shape_tyfun_full. left. exists x. exists n. reflexivity.
-+ clear shape_tyfun_full. right. inv same. 
-  exists x. exists c. auto.
+intros same. destruct orig. destruct H1; try discriminate. eauto.
++ inv same. eauto. 
 + rewrite same in H2. apply subtype_shape_fun in H2. 
   destruct H2 as [A'' [C'' [funty]]]. subst. 
   apply (shape_tyfun_full _ _ A'' C'') in H1. clear shape_tyfun_full. 
   2: reflexivity. destruct H1. auto.
   right. destruct H1. destruct H1 as [c']. 
   exists x. exists c'.
-  destruct H1. aconstructor. apply TypeC; inv H0.
+  destruct H1. aconstructor. apply TypeC; inv H0; auto.
   * apply WfCtxU; assumption.
-  * assumption.
   * destruct H2. eapply TypeCSubtype. 2: eauto.
-    eapply ctx_subtype_ctype. eauto.
-    apply WfCtxU; assumption.
+    eapply ctx_subtype_ctype. eauto. apply WfCtxU; assumption.
     apply SubtypeCtxU. apply ctx_subtype_refl. all: assumption.
 Qed.
 
 Lemma shape_fun Γ x c A C :
   has_vtype Γ (Fun x c) (TyFun A C) -> has_ctype (CtxU Γ A) c C.
 Proof.
-intro orig.
-apply (shape_tyfun_full _ _ A C) in orig as shape. 2: reflexivity.
+intro orig. apply (shape_tyfun_full _ _ A C) in orig as shape. 2: reflexivity.
 destruct shape.
 + destruct H as [y [n]]. discriminate.
 + do 3 (destruct H). inv H. inv H0. apply TypeC; assumption.
@@ -783,8 +726,7 @@ Fixpoint shape_handler_full Γ v x c_r h ty
     has_ctype (CtxU Γ A) c_r D /\ has_htype Γ h Σ' D' /\ respects Γ h Σ' D' E
     /\ sig_subtype Σ Σ' /\ csubtype D' D).
 Proof.
-intros same.
-destruct orig. destruct H1; try discriminate.
+intros same. destruct orig. destruct H1; try discriminate.
 + clear shape_handler_full. exists A. exists Σ. exists E. exists D.
   exists Σ. exists D. inv same. do 3 aconstructor.
   inv H0. inv H6. aconstructor. constructor.
@@ -820,9 +762,7 @@ Fixpoint shape_tyhandler_full Γ v A Σ E D ty
     /\ has_htype Γ h Σ' D' /\ respects Γ h Σ' D' E
     /\ sig_subtype Σ Σ' /\ csubtype D' D).
 Proof.
-intros same.
-destruct orig. destruct H1; try discriminate.
-+ clear shape_tyhandler_full. left. exists x. exists n. reflexivity.
+intros same. destruct orig. destruct H1; try discriminate. eauto.
 + clear shape_tyhandler_full. right.
   exists x. exists c_ret. exists h. exists Σ. exists D.
   inv same. do 4 aconstructor. constructor; inv H2.
@@ -837,8 +777,7 @@ destruct orig. destruct H1; try discriminate.
   aconstructor. constructor; destruct H1.
   - eapply ctx_subtype_ctype. eauto.
     inv H0. inv H7. apply WfCtxU; assumption.
-    apply SubtypeCtxU. apply ctx_subtype_refl. assumption.
-    inv H2. assumption.
+    apply SubtypeCtxU. apply ctx_subtype_refl. all: inv H2; assumption.
   - inv H2. aconstructor. constructor.  eapply respects_eqs_subtype; eauto. 
     inv H0. inv H6. eapply wf_eqs_sig_subtype; eauto.
     eapply sig_subtype_trans; eauto. inv hty. assumption. constructor.
@@ -854,7 +793,7 @@ intro orig.
 apply (shape_tyhandler_full _ _ A Σ E D) in orig as shape. 2: reflexivity.
 destruct shape.
 + destruct H as [y [n]]. discriminate.
-+ do 6 (destruct H). exists x3. exists x4. inv H. auto. 
++ do 6 (destruct H). inv H. eauto.
 Qed.
 
 (* ========================= Handler Cases Shapes ========================= *)
@@ -862,46 +801,40 @@ Qed.
 Lemma h_has_case Γ h Σ D op A_op B_op:
   has_htype Γ h Σ D ->
   get_op_type Σ op = Some (A_op, B_op) ->
-  exists x k c_op, find_op_case h op = Some (x, k, c_op).
+  exists x k c_op, find_case h op = Some (x, k, c_op).
 Proof.
 revert Γ Σ. induction h; intros Γ Σ typed gets; inv typed; inv H2.
 + simpl in gets. discriminate.
-+ simpl in *. destruct (op==o).
-  - exists v. exists v0. exists c. reflexivity.
-  - eapply IHh; eauto.
++ simpl in *. destruct (op==o); eauto.
 Qed.
 
 Lemma case_has_type Γ h Σ D op Aop Bop x k c_op:
-  has_htype Γ h Σ D -> get_op_type Σ op = Some (Aop, Bop)
-  -> find_op_case h op = Some (x, k, c_op) ->
+  has_htype Γ h Σ D -> get_op_type Σ op = Some (Aop, Bop) ->
+  find_case h op = Some (x, k, c_op) ->
   has_ctype (CtxU (CtxU Γ (TyFun Bop D)) Aop) c_op D.
 Proof.
 revert Σ. induction h; intros Σ tys gets finds.
 simpl in finds. discriminate.
 simpl in *. destruct (op==o).
 - inv tys. inv H2. simpl in *. destruct (o==o). 2: (destruct n; reflexivity).
-  inv finds. inv gets. intros. subst. assumption.
+  inv finds. inv gets. assumption.
 - inv tys. inv H2. eapply IHh; eauto.
-  clear IHh. simpl in gets. destruct (op==o).
-  * rewrite e in n. destruct n. reflexivity.
-  * assumption.
+  simpl in gets. destruct (op==o); eauto. rewrite e in n. destruct n. auto.
 Qed. 
 
-(* ========================== Computation Shapes ========================== *)
-
+(* ==================== Computation Shapes ==================== *)
 
 (* Return *)
-Fixpoint shape_ret_full Γ c C v A Σ E
-  (orig : has_ctype Γ c C) {struct orig} :
-  c = (Ret v) -> C = (CTy A Σ E) -> has_vtype Γ v A.
+Fixpoint shape_ret_full Γ c C v A Σ E (orig : has_ctype Γ c C) {struct orig} :
+  c = (Ret v) -> C = (CTy A Σ E) -> 
+  has_vtype Γ v A.
 Proof.  
 intros same samety. destruct orig. destruct H1; try discriminate.
 + clear shape_ret_full. inv same. inv samety. assumption.
 + destruct C as (A', Σ', E').
   apply (shape_ret_full _ _ (CTy A' Σ' E') v A' Σ' E') in H1;
   clear shape_ret_full; auto. subst.
-  inv H0. apply TypeV; auto.
-  inv H2. eapply TypeVSubtype; eauto.
+  inv H0. apply TypeV; auto. inv H2. eapply TypeVSubtype; eauto.
 Qed.
 
 
@@ -916,9 +849,8 @@ Qed.
 Fixpoint shape_absurd_full Γ c C v (orig : has_ctype Γ c C) {struct orig} :
   c = (Absurd v) -> has_vtype Γ v TyØ.
 Proof.  
-intros same. destruct orig. destruct H1; try discriminate; inv same.
-+ assumption.
-+ apply (shape_absurd_full _ _ _ v) in H1; auto.
+intros same. destruct orig. destruct H1; try discriminate; inv same; auto.
+apply (shape_absurd_full _ _ _ v) in H1; auto.
 Qed.
 
 
@@ -940,10 +872,7 @@ intros same. destruct orig. destruct H1; try discriminate; inv same.
 + apply (shape_prodmatch_full _ _ v x y c') in H1; clear shape_prodmatch_full. 
   2: reflexivity. destruct H1 as [A' [B' [vty]]].
   exists A'. exists B'. aconstructor.
-  apply TypeC.
-  - inv H1. assumption.
-  - assumption.
-  - eapply TypeCSubtype; eauto.
+  apply TypeC; try (inv H1; assumption). eapply TypeCSubtype; eauto.
 Qed.
 
 
@@ -969,10 +898,7 @@ intros same. destruct orig. destruct H1; try discriminate.
   destruct H1 as [A' [B' [vty]]].
   exists A'. exists B'. aconstructor.
   inv H1. constructor; apply TypeC; auto.
-  - inv H3. assumption.
-  - eapply TypeCSubtype; eauto.
-  - inv H4. assumption.
-  - eapply TypeCSubtype; eauto.
+  all: (eapply TypeCSubtype; eauto) || (inv H3; inv H4; assumption).
 Qed.
 
 
@@ -995,8 +921,7 @@ intros same. destruct orig. destruct H1; try discriminate.
 + apply (shape_app_full _ _ v1 v2) in H1;
   clear shape_app_full. 2: assumption.
   destruct H1 as [A' [fty]].
-  exists A'. aconstructor. apply TypeV. 
-  - assumption.
+  exists A'. aconstructor. apply TypeV. auto.
   - inv fty. inv H4. apply WfTyFun; assumption.
   - eapply TypeVSubtype. exact fty. apply SubtypeTyFun.
     apply vsubtype_refl. inv fty. inv H4. all: assumption.
@@ -1008,8 +933,7 @@ Fixpoint shape_app Γ x c v C :
   (exists A, has_ctype (CtxU Γ A) c C /\ has_vtype Γ v A).
 Proof.
 intro orig. eapply (shape_app_full _ _ (Fun x c) v C) in orig.
-2: reflexivity. destruct orig as [A [fty]]. 
-exists A. constructor. apply shape_fun in fty. all: assumption.
+2: reflexivity. destruct orig as [A [fty]]. apply shape_fun in fty. eauto.
 Qed.
 
 
@@ -1020,14 +944,14 @@ Fixpoint shape_handle_full Γ c v c' C (orig : has_ctype Γ c C) {struct orig} :
 Proof.  
 intros same. destruct orig. destruct H1; try discriminate.
 + clear shape_handle_full. inv same. exists C. auto.
-+ apply (shape_handle_full _ _ v c') in H1;
-  clear shape_handle_full. 2: assumption.
++ apply (shape_handle_full _ _ v c') in H1; auto.
   destruct H1 as [D [vty]].
   exists D. aconstructor. inv H1.
   apply TypeV. assumption. apply WfTyHandler; auto.
   eapply TypeVSubtype. exact vty.
   apply SubtypeTyHandler. apply csubtype_refl. all: assumption.
 Qed.
+
 
 Fixpoint shape_handle Γ v c D :
   has_ctype Γ (Handle v c) D ->
@@ -1042,15 +966,14 @@ Fixpoint shape_letrec_full Γ c f x c1 c2 D
   (orig : has_ctype Γ c D) {struct orig} :
   c = (LetRec f x c1 c2) ->
   (exists A C, has_ctype (CtxU (CtxU Γ A) (TyFun A C)) c1 C /\ 
-  has_ctype (CtxU Γ (TyFun A C)) c2 D).
+    has_ctype (CtxU Γ (TyFun A C)) c2 D).
 Proof.  
 intros same. destruct orig. destruct H1; try discriminate.
 + clear shape_letrec_full. inv same. exists A. exists C. auto.
 + apply (shape_letrec_full _ _ f x c1 c2) in H1;
   clear shape_letrec_full. 2: assumption.
   destruct H1 as [A' [C'' [cty]]]. inv H1.
-  exists A'. exists C''. aconstructor.
-  apply TypeC; auto.
+  exists A'. exists C''. aconstructor. apply TypeC; auto.
   eapply TypeCSubtype. 2: eauto. apply TypeC; assumption.
 Qed.
 
@@ -1078,8 +1001,7 @@ intros same samety. destruct orig. destruct H1; try discriminate; inv same.
   exists A''. constructor.
   - apply TypeC. assumption. inv cty. inv H0. inv H4.
     apply WfCTy; assumption. eapply TypeCSubtype. exact cty.
-    inv H2. inv cty. inv H3. 
-    apply SubtypeCTy. apply vsubtype_refl. all: assumption.
+    inv H2. inv cty. inv H3. apply SubtypeCTy; auto. apply vsubtype_refl; auto.
   - apply TypeC. inv H1. 3: eapply TypeCSubtype. all: eauto.
 Qed.
 
@@ -1098,23 +1020,20 @@ Fixpoint shape_op_full Γ c C op v y c' A Σ E
   (orig : has_ctype Γ c C) {struct orig} :
   c = (Op op v y c') -> C = (CTy A Σ E) ->
   (exists Aop Bop, get_op_type Σ op = Some (Aop, Bop) /\
-  has_vtype Γ v Aop /\  has_ctype (CtxU Γ Bop) c' C).
+    has_vtype Γ v Aop /\  has_ctype (CtxU Γ Bop) c' C).
 Proof.  
 intros same samety. destruct orig. destruct H1; try discriminate; inv same.
-+ inv samety. clear shape_op_full. exists A_op. exists B_op. auto.
++ inv samety. eauto.
 + destruct C as (A', Σ', E').
   apply (shape_op_full _ _ (CTy A' Σ' E') op v y c' A' Σ' E') in H1;
-  clear shape_op_full; try reflexivity.
-  destruct H1 as [A'' [B'' [g [vty]]]]. inv H2.
-  eapply sig_subtype_gets_Some in g. 2: exact H10.
-  destruct g as [A''' [B''' [g' [sty']]]].
-  exists A'''. exists B'''.
-  aconstructor. constructor.
+  clear shape_op_full; eauto. destruct H1 as [A'' [B'' [g [vty]]]]. inv H2.
+  eapply sig_subtype_get_Some in g; eauto. destruct g as [A'''[B'''[g'[s']]]].
+  exists A'''. exists B'''. aconstructor. constructor.
   - apply TypeV. assumption. apply get_op_type_wf in g'. destruct g'.
     assumption. inv H0. assumption. eapply TypeVSubtype; eauto.
   - eapply (ctx_subtype_ctype (CtxU Γ B'') (CtxU Γ B''')).
     * apply TypeC. inv H1. assumption. assumption.
-      eapply TypeCSubtype. exact H1. apply SubtypeCTy; assumption.
+      eapply TypeCSubtype. eauto. apply SubtypeCTy; assumption.
     * apply WfCtxU. assumption. apply get_op_type_wf in g'. destruct g'.
       all: inv H0; assumption.
     * apply SubtypeCtxU. apply ctx_subtype_refl. all: assumption.
@@ -1129,10 +1048,7 @@ Proof.
 intro orig. eapply (shape_op_full _ _ _ op v y c A Σ E) in orig; auto.
 Qed.
 
-
-
-
-(* ========================== Logic Subtyping ========================== *)
+(* ==================== Logic Subtyping ==================== *)
 
 Lemma veq_subtype A A' Γ v1 v2 :
   veq A Γ v1 v2 -> wf_vtype A' -> vsubtype A A' -> veq A' Γ v1 v2.
