language_formalisation/type_system/type_aux_lemmas.v
@@ -1,16 +1,15 @@
-(* Add LoadPath "C:\Users\Ziga\Documents\Ziga_podatki\PHD\language_formalisation\syntax". *)
-(* Add LoadPath "C:\Users\Ziga\Documents\Ziga_podatki\PHD\language_formalisation\type_system". *)
-(* Add LoadPath "C:\Users\Ziga\Documents\Ziga_podatki\PHD\language_formalisation\substitution". *)
-Add LoadPath "E:\Ziga_Podatki\faks\PHD\language_formalisation\syntax".
-Add LoadPath "E:\Ziga_Podatki\faks\PHD\language_formalisation\type_system".
-Add LoadPath "E:\Ziga_Podatki\faks\PHD\language_formalisation\substitution".
+Add LoadPath "C:\Users\Ziga\Documents\Ziga_podatki\PHD\language_formalisation\syntax".
+Add LoadPath "C:\Users\Ziga\Documents\Ziga_podatki\PHD\language_formalisation\type_system".
+Add LoadPath "C:\Users\Ziga\Documents\Ziga_podatki\PHD\language_formalisation\substitution".
+(* Add LoadPath "E:\Ziga_Podatki\faks\PHD\language_formalisation\syntax". *)
+(* Add LoadPath "E:\Ziga_Podatki\faks\PHD\language_formalisation\type_system". *)
+(* Add LoadPath "E:\Ziga_Podatki\faks\PHD\language_formalisation\substitution". *)
 
-Require Export syntax syntax_lemmas declarational substitution Omega Logic.
-Require Export substitution_lemmas subtyping subtyping_lemmas wf_lemmas.
+Require Export syntax_lemmas substitution_lemmas subtyping_lemmas.
 
 Ltac inv H := inversion H; clear H; subst.
 
-
+(* ==================== Typing and No/Under Var ==================== *)
 
 Lemma has_vtype_is_under_ctx Γ v A:
   has_vtype Γ v A -> v_under_var v (ctx_len Γ)
@@ -21,30 +20,25 @@ with has_htype_is_under_ctx Γ h Σ D:
 Proof.
 {
 intro types. destruct types. destruct H1; simpl; auto.
-all: try constructor; eauto.
-+ eapply ctx_len_gets. eauto.
-+ assert (S (ctx_len Γ) = ctx_len (CtxU Γ A)) by (simpl; reflexivity).
-  rewrite H2. eauto.
-+ assert (S (ctx_len Γ) = ctx_len (CtxU Γ A)) by (simpl; reflexivity).
-  rewrite H4. eauto.
+all: try constructor; eauto. eapply ctx_len_gets. eauto.
+all: assert (S (ctx_len Γ) = ctx_len (CtxU Γ A)) as cA by (simpl; reflexivity).
+all: rewrite cA; eauto.
 }{
 intro types. destruct types. destruct H1; simpl.
-all: try constructor. all: try constructor.
-all: try eauto.
+all: try constructor; try constructor; try eauto.
 all: assert (forall A Γ, S(ctx_len Γ) = ctx_len (CtxU Γ A)) as ext by auto.
-all: erewrite ext; eauto.
-all: erewrite ext; eauto.
+all: erewrite ext; eauto; erewrite ext; eauto.
 }{
-intro types. destruct types. destruct H2; simpl. auto.
-constructor; eauto.
-assert (S(S(ctx_len Γ)) = ctx_len(CtxU(CtxU Γ (TyFun B_op D)) A_op)) as ext
-by auto. rewrite ext. eauto.
+intro types. destruct types. destruct H2; simpl. auto. constructor; eauto.
+assert (S(S(ctx_len Γ)) = ctx_len(CtxU(CtxU Γ (TyFun B_op D)) A_op)) by auto.
+rewrite H5. eauto.
 }
 Qed.
 
-Lemma wf_under_ctx_tctx Γ Z T Σ:
-  wf_tmpl Γ Z T Σ -> 
-  tmpl_under_var T (ctx_len Γ) /\ tmpl_under_tvar_j T (tctx_len Z).
+
+Lemma wf_is_under_ctx_tctx Γ Z T Σ:
+  wf_t Γ Z T Σ -> 
+  t_under_var T (ctx_len Γ) /\ t_under_tvar T (tctx_len Z).
 Proof.
 revert Γ. induction T; intros Γ wf.
 + destruct v as (x, i). inv wf. simpl. constructor.
@@ -53,83 +47,71 @@ revert Γ. induction T; intros Γ wf.
 + inv wf. simpl. constructor. 2: auto.
   eapply has_vtype_is_under_ctx. eauto.
 + inv wf. simpl. constructor. constructor.
-  - eapply has_vtype_is_under_ctx. eauto.
-  - apply IHT in H7. destruct H7. simpl in *. assumption.
-  - apply IHT in H7. destruct H7. assumption.
+  eapply has_vtype_is_under_ctx. eauto.
+  all: apply IHT in H7; destruct H7; assumption.
 + inv wf. simpl. constructor. constructor.
-  - eapply has_vtype_is_under_ctx. eauto.
-  - apply IHT1 in H8. apply IHT2 in H9.
-    destruct H8. destruct H9. simpl in *. auto.
-  - apply IHT1 in H8. apply IHT2 in H9.
-    destruct H8. destruct H9. simpl in *. auto.
+  eapply has_vtype_is_under_ctx. eauto.
+  all: apply IHT1 in H8; apply IHT2 in H9; destruct H8; destruct H9; auto.
 + inv wf. simpl. constructor. constructor.
-  - eapply has_vtype_is_under_ctx. eauto.
-  - apply IHT in H8. destruct H8. simpl in *. assumption.
-  - apply IHT in H8. destruct H8. assumption.
+  eapply has_vtype_is_under_ctx. eauto.
+  all: apply IHT in H8; destruct H8; assumption.
 Qed.
 
 
-Lemma handle_tmpl_no_var h i Γ Z T Σ:
-  h_no_var h i -> wf_tmpl Γ Z T Σ ->
-  c_no_var (handle_tmpl (ctx_len Γ) (tctx_len Z) h T) 
+Lemma handle_t_no_var h i Γ Z T Σ:
+  h_no_var h i -> wf_t Γ Z T Σ ->
+  c_no_var (handle_t (ctx_len Γ) (tctx_len Z) h T) 
     (i + ctx_len Γ + tctx_len Z).
 Proof.
 revert h Γ i. induction T; intros; simpl.
 all: assert (i+ctx_len Γ+tctx_len Z=tctx_len Z+(i+ctx_len Γ)) as comm by omega.
-+ destruct v as (x, d). constructor; apply wf_under_ctx_tctx in H0;
-  destruct H0; simpl in *. omega.
-  rewrite comm. apply v_no_var_shift. 2:omega.
-  eapply v_under_var_no_var. eauto. omega.
-+ rewrite comm. apply v_no_var_shift. 2:omega.
-  apply wf_under_ctx_tctx in H0. destruct H0.
-  eapply v_under_var_no_var. eauto. omega.
+all: assert (S(S(i+ctx_len Γ+tctx_len Z))=(i+S(S(ctx_len Γ)))+tctx_len Z) 
+  as ssctx by omega.
+all: assert (S(i+ctx_len Γ+tctx_len Z)=(i+S(ctx_len Γ))+tctx_len Z)
+  as sctx by (simpl; omega).
++ destruct v as (x, d). constructor; apply wf_is_under_ctx_tctx in H0;
+  destruct H0; simpl in *. omega. rewrite comm. apply v_no_var_shift.
+  eapply v_under_var_no_var. all: omega || eauto.
++ rewrite comm. apply v_no_var_shift. apply wf_is_under_ctx_tctx in H0.
+  destruct H0. eapply v_under_var_no_var. all: omega || eauto.
 + constructor; inv H0.
   - rewrite comm. apply v_no_var_shift. eapply v_under_var_no_var.
-    eapply has_vtype_is_under_ctx. eauto. all: omega.
-  - assert (S(S(i+ctx_len Γ+tctx_len Z))=(i+S(S(ctx_len Γ)))+tctx_len Z).
-    omega. assert (S(S(ctx_len Γ))=ctx_len (CtxU (CtxU Γ A) B)).
-    simpl. omega. rewrite H0, H1. apply IHT; auto.
+    eapply has_vtype_is_under_ctx. all: omega || eauto.
+  - assert (S(S(ctx_len Γ))=ctx_len (CtxU (CtxU Γ A) B)) by (simpl; omega).
+    rewrite ssctx, H0. auto.
 + inv H0. constructor. 2: constructor.
   - rewrite comm. apply v_no_var_shift. eapply v_under_var_no_var.
     eapply has_vtype_is_under_ctx. eauto. all: omega.
-  - assert (S(i+ctx_len Γ+tctx_len Z)=(i+S(ctx_len Γ))+tctx_len Z).
-    omega. assert (S(ctx_len Γ)=ctx_len (CtxU Γ A)).
-    simpl. omega. rewrite H0, H1. apply IHT1; auto.
-  - assert (S(i+ctx_len Γ+tctx_len Z)=(i+S(ctx_len Γ))+tctx_len Z).
-    omega. assert (S(ctx_len Γ)=ctx_len (CtxU Γ B)).
-    simpl. omega. rewrite H0, H1. apply IHT2; auto.
-+ destruct (find_op_case h o) eqn:finds; inv H0.
+  - assert (S(ctx_len Γ)=ctx_len (CtxU Γ A)).
+    simpl. omega. rewrite sctx, H0. auto.
+  - assert (S(ctx_len Γ)=ctx_len (CtxU Γ B)).
+    simpl. omega. rewrite sctx, H0. auto.
++ destruct (find_case h o) eqn:finds; inv H0.
   - destruct p as ((x, k), c_op). unfold c_subs2_out. unfold c_subs_out.
-    apply c_no_var_subs. apply c_no_var_subs.
-    * eapply find_op_case_no_var in finds. 2: eauto. simpl.
+    apply c_no_var_subs. apply c_no_var_subs. all: omega || simpl.
+    * eapply find_case_no_var in finds. 2: eauto. simpl.
       assert (S(S(i+ctx_len Γ+tctx_len Z))=ctx_len Γ+tctx_len Z+(2+i)) by omega.
       rewrite H0. apply c_no_var_shift. eauto. omega.
-    * rewrite v_shift_shift. simpl.
-      assert (S(i+ctx_len Γ+tctx_len Z)=tctx_len Z+1+(ctx_len Γ+i)) by omega.
-      rewrite H0. apply v_no_var_shift.
-      eapply v_under_var_no_var. eapply has_vtype_is_under_ctx.
-      eauto. omega. omega.
-    * omega.
+    * assert (S(i+ctx_len Γ+tctx_len Z)=tctx_len Z+1+(ctx_len Γ+i)) by omega.
+      rewrite v_shift_shift, H0. apply v_no_var_shift; try omega.
+      eapply v_under_var_no_var. eapply has_vtype_is_under_ctx. eauto. omega.
     * simpl. assert (S(i+ctx_len Γ+tctx_len Z)=i+(S (ctx_len Γ))+tctx_len Z).
-      omega. rewrite H0. assert (S (ctx_len Γ) = ctx_len (CtxU Γ B_op)).
-      simpl. omega. rewrite H1. apply IHT; auto.
-    * omega.
+      omega. assert (S (ctx_len Γ) = ctx_len (CtxU Γ B_op)). simpl. omega.
+      rewrite H0, H1. auto.
   - simpl. constructor.
     * rewrite comm. eapply v_under_var_no_var.
       eapply has_vtype_is_under_ctx. eauto. all: omega.
-    * simpl. assert (S(i+ctx_len Γ+tctx_len Z)=i+(S (ctx_len Γ))+tctx_len Z).
-      omega. rewrite H0. assert (S (ctx_len Γ) = ctx_len (CtxU Γ B_op)).
-      simpl. omega. rewrite H1. apply IHT; auto.
+    * rewrite sctx. assert (S (ctx_len Γ) = ctx_len (CtxU Γ B_op)).
+      simpl. omega. rewrite H0. auto.
 Qed.
 
-Lemma handle_tmpl_shift Γ' Γ Z h T Σ D i:
-  wf_tmpl Γ Z T Σ -> has_htype Γ' h Σ D 
-  -> 
-  handle_tmpl (ctx_len Γ) (tctx_len Z) (Sub.h_shift h 1 i) T
-  = 
-  Sub.c_shift 
-    (handle_tmpl (ctx_len Γ) (tctx_len Z) h T) 
-    1 (i + ctx_len Γ + tctx_len Z).
+(* ==================== Handling and Shifts. ==================== *)
+
+Lemma handle_t_shift Γ' Γ Z h T Σ D i:
+  wf_t Γ Z T Σ -> has_htype Γ' h Σ D -> 
+    handle_t (ctx_len Γ) (tctx_len Z) (Sub.h_shift h 1 i) T
+  = Sub.c_shift (handle_t (ctx_len Γ) (tctx_len Z) h T) 
+      1 (i + ctx_len Γ + tctx_len Z).
 Proof.
 revert Γ h i. induction T; intros Γ h i wf types; simpl; inv wf.
 all: assert (i+ctx_len Γ+tctx_len Z=tctx_len Z+(i+ctx_len Γ)) as comm by omega.
@@ -137,66 +119,54 @@ all: assert (i+ctx_len Γ+tctx_len Z=tctx_len Z+(i+ctx_len Γ)) as comm by omega
   destruct ((i + ctx_len Γ + tctx_len Z) <=? num) eqn:cmp.
   - apply leb_complete in cmp. omega.
   - f_equal. apply eq_sym. eapply v_shift_too_high.
-    apply has_vtype_is_under_ctx in H3.
-    rewrite comm. apply v_under_var_shift.
+    apply has_vtype_is_under_ctx in H3. rewrite comm. apply v_under_var_shift.
     eapply v_under_var_weaken. eauto. all: omega.
 + f_equal. apply eq_sym. eapply v_shift_too_high.
-    apply has_vtype_is_under_ctx in H2.
-    rewrite comm. apply v_under_var_shift.
+    apply has_vtype_is_under_ctx in H2. rewrite comm. apply v_under_var_shift.
     eapply v_under_var_weaken. eauto. all: omega.
 + f_equal.
   - apply eq_sym. eapply v_shift_too_high. 
-    apply has_vtype_is_under_ctx in H6.
-    rewrite comm. apply v_under_var_shift.
+    apply has_vtype_is_under_ctx in H6. rewrite comm. apply v_under_var_shift.
     eapply v_under_var_weaken. eauto. all: omega.
-  - assert 
-      (S(S(i+ctx_len Γ+tctx_len Z))=i+ctx_len(CtxU(CtxU Γ A) B)+tctx_len Z)
+  - assert (S(S(i+ctx_len Γ+tctx_len Z))=i+ctx_len(CtxU(CtxU Γ A)B)+tctx_len Z)
     as clen by (simpl; omega).
     assert (S(S(ctx_len Γ)) = ctx_len (CtxU(CtxU Γ A) B)) as clen' by omega.
     rewrite clen, clen', IHT; auto.
 + f_equal.
-  - apply eq_sym. eapply v_shift_too_high.
-    apply has_vtype_is_under_ctx in H7.
-    rewrite comm. apply v_under_var_shift.
+  - apply eq_sym. eapply v_shift_too_high. 
+    apply has_vtype_is_under_ctx in H7. rewrite comm. apply v_under_var_shift.
     eapply v_under_var_weaken. eauto. all: omega.
   - eapply (IHT1 _) in H8. simpl in H8.
-    assert (S(i + ctx_len Γ+tctx_len Z)=i+S (ctx_len Γ)+tctx_len Z) by omega.
+    assert (S(i+ctx_len Γ+tctx_len Z)=i+S (ctx_len Γ)+tctx_len Z) by omega.
     rewrite H. eauto. assumption.
   - eapply (IHT2 _) in H9. simpl in H9.
-    assert (S(i + ctx_len Γ+tctx_len Z)=i+S (ctx_len Γ)+tctx_len Z) by omega.
+    assert (S(i+ctx_len Γ+tctx_len Z)=i+S (ctx_len Γ)+tctx_len Z) by omega.
     rewrite H. eauto. assumption.
 + eapply h_has_case in H6 as find. 2: exact types.
   destruct find as [x[k[cop]]]. rename H into find.
-  erewrite h_shift_find_op_Some, find. 2:eauto.
-  unfold c_subs2_out. unfold c_subs_out.
+  erewrite shift_find_Some, find; eauto. unfold c_subs2_out. unfold c_subs_out.
   rewrite c_shift_subs. 2: omega. f_equal.
   * rewrite c_shift_subs. 2: omega. f_equal; simpl.
     assert (S(S(i+ctx_len Γ+tctx_len Z))=(ctx_len Γ+tctx_len Z)+S(S i))
     as cext by omega. rewrite cext.
-    apply (c_shift_comm_aux 1 (S(S i)) _ (ctx_len Γ+tctx_len Z)). omega.
-    rewrite v_shift_shift.
-    rewrite (v_shift_too_high (Sub.v_shift v (tctx_len Z + 1) 0)).
-    reflexivity.
-    assert (S(i+ctx_len Γ+tctx_len Z)=(tctx_len Z+1)+(i+ctx_len Γ))
-    as comm' by omega. rewrite comm'.
-    apply v_under_var_shift. 2: omega.
-    apply has_vtype_is_under_ctx in H7.
-    eapply v_under_var_weaken. eauto. omega.
+    apply (c_shift_comm 1 (S(S i)) _ (ctx_len Γ+tctx_len Z)). omega.
+    rewrite v_shift_shift, (v_shift_too_high (Sub.v_shift v (tctx_len Z+1) 0)).
+    2:assert (S(i+ctx_len Γ+tctx_len Z)=(tctx_len Z+1)+(i+ctx_len Γ)) as comm'.
+    reflexivity. omega. rewrite comm'. apply v_under_var_shift.
+    apply has_vtype_is_under_ctx in H7. eapply v_under_var_weaken.
+    all: omega || eauto.
   * f_equal. simpl. 
     assert (S(ctx_len Γ)=ctx_len (CtxU Γ B_op)) by (simpl;omega).
     assert (S(i+ctx_len Γ+tctx_len Z)=i+ctx_len (CtxU Γ B_op)+tctx_len Z).
-    { simpl. omega. }
-    rewrite H, H0, IHT. f_equal. all: assumption.
+    simpl. omega. rewrite H, H0, IHT. f_equal. all: assumption.
 Qed.
 
-Lemma handle_tmpl_negshift Γ' Γ Z h T Σ D i:
-  h_no_var h i -> wf_tmpl Γ Z T Σ -> has_htype Γ' h Σ D 
-  -> 
-  handle_tmpl (ctx_len Γ) (tctx_len Z) (Sub.h_negshift h 1 i) T
-  = 
-  Sub.c_negshift 
-    (handle_tmpl (ctx_len Γ) (tctx_len Z) h T) 
-    1 (i + ctx_len Γ + tctx_len Z).
+
+Lemma handle_t_negshift Γ' Γ Z h T Σ D i:
+  h_no_var h i -> wf_t Γ Z T Σ -> has_htype Γ' h Σ D -> 
+    handle_t (ctx_len Γ) (tctx_len Z) (Sub.h_negshift h 1 i) T
+  = Sub.c_negshift (handle_t (ctx_len Γ) (tctx_len Z) h T) 
+      1 (i + ctx_len Γ + tctx_len Z).
 Proof.
 revert Γ h i. induction T; intros Γ h i novar wf types; simpl; inv wf.
 all: assert (i+ctx_len Γ+tctx_len Z=tctx_len Z+(i+ctx_len Γ)) as comm by omega.
@@ -204,17 +174,14 @@ all: assert (i+ctx_len Γ+tctx_len Z=tctx_len Z+(i+ctx_len Γ)) as comm by omega
   destruct ((i + ctx_len Γ + tctx_len Z) <=? num) eqn:cmp.
   - apply leb_complete in cmp. omega.
   - f_equal. apply eq_sym. eapply v_negshift_too_high.
-    apply has_vtype_is_under_ctx in H3.
-    rewrite comm. apply v_under_var_shift.
+    apply has_vtype_is_under_ctx in H3. rewrite comm. apply v_under_var_shift.
     eapply v_under_var_weaken. eauto. all: omega.
 + f_equal. apply eq_sym. eapply v_negshift_too_high.
-    apply has_vtype_is_under_ctx in H2.
-    rewrite comm. apply v_under_var_shift.
+    apply has_vtype_is_under_ctx in H2. rewrite comm. apply v_under_var_shift.
     eapply v_under_var_weaken. eauto. all: omega.
 + f_equal.
   - apply eq_sym. eapply v_negshift_too_high. 
-    apply has_vtype_is_under_ctx in H6.
-    rewrite comm. apply v_under_var_shift.
+    apply has_vtype_is_under_ctx in H6. rewrite comm. apply v_under_var_shift.
     eapply v_under_var_weaken. eauto. all: omega.
   - assert 
       (S(S(i+ctx_len Γ+tctx_len Z))=i+ctx_len(CtxU(CtxU Γ A) B)+tctx_len Z)
@@ -224,64 +191,52 @@ all: assert (i+ctx_len Γ+tctx_len Z=tctx_len Z+(i+ctx_len Γ)) as comm by omega
 + f_equal;
   assert (S(i + ctx_len Γ+tctx_len Z)=i+S (ctx_len Γ)+tctx_len Z) by omega.
   - apply eq_sym. eapply v_negshift_too_high.
-    apply has_vtype_is_under_ctx in H7.
-    rewrite comm. apply v_under_var_shift.
+    apply has_vtype_is_under_ctx in H7. rewrite comm. apply v_under_var_shift.
     eapply v_under_var_weaken. eauto. all: omega.
-  - eapply (IHT1 _) in H8. simpl in H8.
-    rewrite H. all: eauto.
-  - eapply (IHT2 _) in H9. simpl in H9.
-    rewrite H. all: eauto.
+  - eapply (IHT1 _) in H8. simpl in H8. rewrite H. all: eauto.
+  - eapply (IHT2 _) in H9. simpl in H9. rewrite H. all: eauto.
 + eapply h_has_case in H6 as find. 2: exact types.
   destruct find as [x[k[cop]]]. rename H into find.
-  erewrite find, h_negshift_find_op_Some. 2: eauto.
-  unfold c_subs2_out. unfold c_subs_out.
-  rewrite c_negshift_subs. 2: omega. f_equal.
+  erewrite find, negshift_find_Some. unfold c_subs2_out. unfold c_subs_out.
+  2: eauto. rewrite c_negshift_subs. 2: omega. f_equal.
   * rewrite c_negshift_subs. 2: omega. f_equal; simpl.
     - assert (S(S(i+ctx_len Γ+tctx_len Z))=(ctx_len Γ+tctx_len Z)+S(S i))
       as cext by omega. rewrite cext.
-      apply c_shift_negshift_1j. eapply find_op_case_no_var; eauto. omega.
-    - rewrite v_shift_shift.
-      rewrite (v_negshift_too_high (Sub.v_shift v (tctx_len Z + 1) 0)).
-      reflexivity.
-      assert (S(i+ctx_len Γ+tctx_len Z)=(tctx_len Z+1)+(i+ctx_len Γ))
-      as comm' by omega. rewrite comm'.
-      apply v_under_var_shift. 2: omega.
-      apply has_vtype_is_under_ctx in H7.
+      apply c_shift_negshift_comm. eapply find_case_no_var; eauto. omega.
+    - rewrite v_shift_shift,(v_negshift_too_high(Sub.v_shift v(tctx_len Z+1)0)).
+      2: assert (S(i+ctx_len Γ+tctx_len Z)=(tctx_len Z+1)+(i+ctx_len Γ))
+      as comm' by omega. reflexivity. rewrite comm'.
+      apply v_under_var_shift. 2: omega. apply has_vtype_is_under_ctx in H7.
       eapply v_under_var_weaken. eauto. omega.
     - assert (S(S(i+ctx_len Γ+tctx_len Z))=(ctx_len Γ+tctx_len Z)+S(S i)).
       omega. simpl. rewrite H. apply c_no_var_shift.
-      eapply find_op_case_no_var; eauto. omega.
+      eapply find_case_no_var; eauto. omega.
     - rewrite v_shift_shift. simpl. 
       assert (S(i+ctx_len Γ+tctx_len Z)=(tctx_len Z+1)+(i+ctx_len Γ)) by omega.
-      rewrite H. apply v_no_var_shift.
-      apply has_vtype_is_under_ctx in H7.
+      rewrite H. apply v_no_var_shift. apply has_vtype_is_under_ctx in H7.
       eapply v_under_var_no_var. eauto. omega. omega.
   * simpl. f_equal. 
     assert (S(ctx_len Γ)=ctx_len (CtxU Γ B_op)) by (simpl;omega).
     assert (S(i+ctx_len Γ+tctx_len Z)=i+ctx_len (CtxU Γ B_op)+tctx_len Z).
-    { simpl. omega. }
-    rewrite H, H0, IHT. f_equal. all: assumption.
-  * clear IHT. eapply c_no_var_subs; simpl.
+    simpl. omega. rewrite H, H0, IHT. f_equal. all: assumption.
+  * clear IHT. eapply c_no_var_subs; simpl. 3: omega.
     - assert (S(S(i+ctx_len Γ+tctx_len Z))=ctx_len Γ + tctx_len Z + (2+i)).
       omega. rewrite H. apply c_no_var_shift.
-      eapply find_op_case_no_var; eauto. omega.
+      eapply find_case_no_var; eauto. omega.
     - eapply v_under_var_no_var. rewrite v_shift_shift.
-      eapply v_under_var_shift. eapply has_vtype_is_under_ctx. eauto.
-      all: omega.
-    - omega.
-  * simpl. clear IHT.
-    assert (S(ctx_len Γ)=ctx_len (CtxU Γ B_op)) by (simpl;omega).
+      eapply v_under_var_shift. eapply has_vtype_is_under_ctx. 
+      all: omega || eauto.
+  * assert (S(ctx_len Γ)=ctx_len (CtxU Γ B_op)) by (simpl;omega).
     assert (S(i+ctx_len Γ+tctx_len Z)=i+ctx_len (CtxU Γ B_op)+tctx_len Z).
-    simpl. omega. rewrite H0, H. eapply handle_tmpl_no_var; eauto.
+    simpl. omega. simpl. rewrite H0, H. eapply handle_t_no_var; eauto.
 Qed.
 
-Lemma handle_tmpl_sub Γ' Γ Z h T Σ D i v_s:
-  wf_tmpl Γ Z T Σ -> has_htype Γ' h Σ D ->
-  handle_tmpl (ctx_len Γ) (tctx_len Z) (Sub.h_sub h (i, v_s)) T
-  = 
-  Sub.c_sub 
-    (handle_tmpl (ctx_len Γ) (tctx_len Z) h T)
-    (i+ctx_len Γ+tctx_len Z, Sub.v_shift v_s (ctx_len Γ+tctx_len Z) 0).
+
+Lemma handle_t_sub Γ' Γ Z h T Σ D i v_s:
+  wf_t Γ Z T Σ -> has_htype Γ' h Σ D ->
+    handle_t (ctx_len Γ) (tctx_len Z) (Sub.h_sub h (i, v_s)) T
+  = Sub.c_sub (handle_t (ctx_len Γ) (tctx_len Z) h T)
+      (i+ctx_len Γ+tctx_len Z, Sub.v_shift v_s (ctx_len Γ+tctx_len Z) 0).
 Proof.
 revert Γ h i. induction T; intros Γ h i wf types; simpl; inv wf.
 all: assert (i+ctx_len Γ+tctx_len Z=tctx_len Z+(i+ctx_len Γ)) as comm by omega.
@@ -293,26 +248,21 @@ all: assert (i+ctx_len Γ+tctx_len Z=tctx_len Z+(i+ctx_len Γ)) as comm by omega
     * rewrite H. reflexivity.
     * rewrite comm. rewrite v_sub_too_high.
       reflexivity. apply v_under_var_shift. 2: omega.
-      eapply v_under_var_weaken. eapply has_vtype_is_under_ctx.
-      eauto. omega.
+      eapply v_under_var_weaken. eapply has_vtype_is_under_ctx. eauto. omega.
 + f_equal. apply eq_sym. eapply v_sub_too_high.
-    apply has_vtype_is_under_ctx in H2.
-    rewrite comm. apply v_under_var_shift.
+    apply has_vtype_is_under_ctx in H2. rewrite comm. apply v_under_var_shift.
     eapply v_under_var_weaken. eauto. all: omega.
 + f_equal.
-  - apply eq_sym. eapply v_sub_too_high. 
-    apply has_vtype_is_under_ctx in H6.
+  - apply eq_sym. eapply v_sub_too_high. apply has_vtype_is_under_ctx in H6.
     rewrite comm. apply v_under_var_shift.
     eapply v_under_var_weaken. eauto. all: omega.
   - assert 
       (S(S(i+ctx_len Γ+tctx_len Z))=i+ctx_len(CtxU(CtxU Γ A) B)+tctx_len Z)
     as clen by (simpl; omega).
     assert (S(S(ctx_len Γ)) = ctx_len (CtxU(CtxU Γ A) B)) as clen' by omega.
-    rewrite clen, clen', IHT, v_shift_shift; auto.
-    do 3 f_equal. simpl. omega.
+    rewrite clen, clen', IHT, v_shift_shift; auto. do 3 f_equal. simpl. omega.
 + f_equal.
-  - apply eq_sym. eapply v_sub_too_high.
-    apply has_vtype_is_under_ctx in H7.
+  - apply eq_sym. eapply v_sub_too_high. apply has_vtype_is_under_ctx in H7.
     rewrite comm. apply v_under_var_shift.
     eapply v_under_var_weaken. eauto. all: omega.
   - eapply (IHT1 _) in H8. simpl in H8.
@@ -323,58 +273,54 @@ all: assert (i+ctx_len Γ+tctx_len Z=tctx_len Z+(i+ctx_len Γ)) as comm by omega
     rewrite H, H9, v_shift_shift. do 3 f_equal. omega. assumption.
 + eapply h_has_case in H6 as find. 2: exact types.
   destruct find as [x[k[cop]]]. rename H into find.
-  erewrite h_sub_find_op_Some, find. 2:eauto.
-  unfold c_subs2_out. unfold c_subs_out.
+  erewrite sub_find_Some, find. 2:eauto. unfold c_subs2_out. unfold c_subs_out.
   rewrite c_sub_subs. 2:omega. f_equal.
   * rewrite c_sub_subs. 2: omega. f_equal; simpl.
     assert (S(S(i+ctx_len Γ+tctx_len Z))=(ctx_len Γ+tctx_len Z)+S(S i))
-    as cext by omega. rewrite cext.
-    rewrite c_shift_sub. do 2 f_equal. do 3 rewrite v_shift_shift.
-    f_equal. omega. omega.
+    as cext by omega. rewrite cext. rewrite c_shift_sub.
+    do 2 f_equal. do 3 rewrite v_shift_shift. f_equal. omega. omega.
     rewrite v_shift_shift, (v_sub_too_high (Sub.v_shift v (tctx_len Z + 1) 0)).
-    reflexivity.
-    assert (S(i+ctx_len Γ+tctx_len Z)=(tctx_len Z+1)+(i+ctx_len Γ))
-    as comm' by omega. rewrite comm'.
-    apply v_under_var_shift. 2: omega.
-    apply has_vtype_is_under_ctx in H7.
-    eapply v_under_var_weaken. eauto. omega.
+    reflexivity. assert (S(i+ctx_len Γ+tctx_len Z)=(tctx_len Z+1)+(i+ctx_len Γ))
+    as comm' by omega. rewrite comm'. apply v_under_var_shift. 2: omega.
+    apply has_vtype_is_under_ctx in H7. eapply v_under_var_weaken. eauto. omega.
   * simpl. f_equal. 
     assert (S(ctx_len Γ)=ctx_len (CtxU Γ B_op)) by (simpl;omega).
     assert (S(i+ctx_len Γ+tctx_len Z)=i+ctx_len (CtxU Γ B_op)+tctx_len Z).
-    { simpl. omega. }
-    rewrite H, H0, IHT. do 2 f_equal. rewrite v_shift_shift.
+    simpl. omega. rewrite H, H0, IHT. do 2 f_equal. rewrite v_shift_shift.
     f_equal. omega. all: assumption.
 Qed.
+
+(* ==================== Safety and Shifts. ==================== *)
 
 Fixpoint v_insert_typesafe 
   Γ v A (orig : has_vtype Γ v A) A_ins i {struct orig} :
   wf_vtype A_ins ->
-  has_vtype (ctx_insert_var Γ A_ins i) (Sub.v_shift v 1 i) A
+  has_vtype (ctx_insert Γ A_ins i) (Sub.v_shift v 1 i) A
 
 with c_insert_typesafe 
   Γ c C (orig : has_ctype Γ c C) A_ins i {struct orig} :
   wf_vtype A_ins ->
-  has_ctype (ctx_insert_var Γ A_ins i) (Sub.c_shift c 1 i) C
+  has_ctype (ctx_insert Γ A_ins i) (Sub.c_shift c 1 i) C
 
 with h_insert_typesafe 
   Γ h Σ D (orig : has_htype Γ h Σ D) A_ins i {struct orig} :
   wf_vtype A_ins ->
-  has_htype (ctx_insert_var Γ A_ins i) (Sub.h_shift h 1 i) Σ D
+  has_htype (ctx_insert Γ A_ins i) (Sub.h_shift h 1 i) Σ D
 
 with respects_insert_typesafe
   Γ h Σ D E (orig: respects Γ h Σ D E) A_ins i {struct orig} :
   has_htype Γ h Σ D -> wf_vtype A_ins ->
-  respects (ctx_insert_var Γ A_ins i) (Sub.h_shift h 1 i) Σ D E
+  respects (ctx_insert Γ A_ins i) (Sub.h_shift h 1 i) Σ D E
 
 with veq_insert_typesafe
   Γ A v1 v2 (orig: veq A Γ v1 v2) A_ins i {struct orig} :
   wf_vtype A_ins ->
-  veq A (ctx_insert_var Γ A_ins i) (Sub.v_shift v1 1 i) (Sub.v_shift v2 1 i)
+  veq A (ctx_insert Γ A_ins i) (Sub.v_shift v1 1 i) (Sub.v_shift v2 1 i)
 
 with ceq_insert_typesafe
   Γ C c1 c2 (orig: ceq C Γ c1 c2) A_ins i {struct orig} :
   wf_vtype A_ins ->
-  ceq C (ctx_insert_var Γ A_ins i) (Sub.c_shift c1 1 i) (Sub.c_shift c2 1 i).
+  ceq C (ctx_insert Γ A_ins i) (Sub.c_shift c1 1 i) (Sub.c_shift c2 1 i).
 
 Proof.
 all: rename v_insert_typesafe into V; rename c_insert_typesafe into CI.
@@ -393,8 +339,7 @@ inv orig. destruct H1.
     assumption. apply leb_complete in cmp. omega.
   - apply TypeVar. rewrite <-get_ctx_insert_unchanged.
     assumption. apply leb_iff_conv in cmp. assumption.
-+ specialize (V _ _ _ H1) as IHv1.
-  specialize (V _ _ _ H2) as IHv2.
++ specialize (V _ _ _ H1) as IHv1. specialize (V _ _ _ H2) as IHv2.
   clear V CI HC R VE CE. simpl. apply TypePair; auto.
 + specialize (V _ _ _ H1) as IHv.
   clear V CI HC R VE CE. simpl. apply TypeInl. auto.
@@ -403,8 +348,7 @@ inv orig. destruct H1.
 + specialize (CI _ _ _ H1) as IHc.
   clear V CI HC R VE CE.
   simpl. apply TypeFun. rewrite ctx_insert_extend. auto.
-+ specialize (HC _ _ _ _ H2) as IHh.
-  specialize (CI _ _ _ H1) as IHc.
++ specialize (HC _ _ _ _ H2) as IHh. specialize (CI _ _ _ H1) as IHc.
   specialize (R _ _ _ _ _ H3) as IHres.
   clear V CI HC R VE CE.
   simpl. apply TypeHandler. rewrite ctx_insert_extend. all: auto. 
@@ -419,32 +363,26 @@ inv orig. destruct H1.
   clear V CI HC R VE CE. simpl. apply TypeRet. auto.
 + specialize (V _ _ _ H1) as IHv.
   clear V CI HC R VE CE. simpl. apply TypeAbsurd. auto.
-+ specialize (V _ _ _ H1) as IHv.
-  specialize (CI _ _ _ H2) as IHc.
++ specialize (V _ _ _ H1) as IHv. specialize (CI _ _ _ H2) as IHc.
   clear V CI HC R VE CE. simpl. eapply TypeΠMatch. auto.
   rewrite ctx_insert_extend. rewrite ctx_insert_extend. auto.
-+ specialize (V _ _ _ H1) as IHv.
-  specialize (CI _ _ _ H2) as IHc1.
++ specialize (V _ _ _ H1) as IHv. specialize (CI _ _ _ H2) as IHc1.
   specialize (CI _ _ _ H3) as IHc2.
   clear V CI HC R VE CE.
   simpl. eapply TypeΣMatch. auto. all: rewrite ctx_insert_extend; auto.
-+ specialize (CI _ _ _ H1) as IHc1.
-  specialize (CI _ _ _ H2) as IHc2.
++ specialize (CI _ _ _ H1) as IHc1. specialize (CI _ _ _ H2) as IHc2.
   clear V CI HC R VE CE.
   simpl. eapply TypeDoBind. auto. rewrite ctx_insert_extend. auto.
-+ specialize (V _ _ _ H1) as IHv.
-  specialize (V _ _ _ H2) as IHv0.
++ specialize (V _ _ _ H1) as IHv. specialize (V _ _ _ H2) as IHv0.
   clear V CI HC R VE CE. simpl. eapply TypeApp; auto.
-+ specialize (V _ _ _ H1) as IHv.
-  specialize (CI _ _ _ H2) as IHc.
++ specialize (V _ _ _ H1) as IHv. specialize (CI _ _ _ H2) as IHc.
   clear V CI HC R VE CE. simpl. eapply TypeHandle; auto.
 + specialize (CI _ _ _ H1) as IHc1.
   specialize (CI _ _ _ H2) as IHc2.
   clear V CI HC R VE CE. simpl. eapply TypeLetRec.
   - do 2 rewrite ctx_insert_extend. auto.
   - rewrite ctx_insert_extend. auto.
-+ specialize (V _ _ _ H2) as IHv.
-  specialize (CI _ _ _ H3) as IHc.
++ specialize (V _ _ _ H2) as IHv. specialize (CI _ _ _ H3) as IHc.
   clear V CI HC R VE CE.
   simpl. eapply TypeOp. 3: rewrite ctx_insert_extend. all: eauto.
 + specialize (CI _ _ _ H1) as IHc.
@@ -452,30 +390,24 @@ inv orig. destruct H1.
 }{
 intros wfins. apply TypeH.
 { apply ctx_insert_wf. inv orig. all: assumption. }
-{ inv orig. assumption. }
-{ inv orig. assumption. }
+all: try (inv orig; assumption).
 inv orig. destruct H2.
 + simpl. clear V CI HC R VE CE. apply TypeCasesØ.
-+ specialize (HC _ _ _ _ H3) as IHh.
-  specialize (CI _ _ _ H4) as IHc.
++ specialize (HC _ _ _ _ H3) as IHh. specialize (CI _ _ _ H4) as IHc.
   clear V CI HC R VE CE.
   simpl. apply TypeCasesU. 2: auto.
-  - apply h_shift_find_op_None. assumption.
+  - apply shift_find_None. assumption.
   - do 2 rewrite ctx_insert_extend. auto.
 }{
 intros types wfins. apply Respects.
-{ clear V CI HC R VE CE.
-  apply ctx_insert_wf. inv orig. all: assumption. }
-{ inv orig. assumption. }
-{ inv orig. assumption. }
-{ inv orig. assumption. }
+{ clear V CI HC R VE CE. apply ctx_insert_wf. inv orig. all: assumption. }
+all: try (inv orig; assumption).
 inv orig. destruct H3.
 + clear V CI HC R VE CE. apply RespectEqsØ.
-+ specialize (R _ _ _ _ _ H3) as IHres.
-  specialize (CE _ _ _ _ H4) as IHeq.
++ specialize (R _ _ _ _ _ H3) as IHres. specialize (CE _ _ _ _ H4) as IHeq.
   clear V CI HC R VE CE. apply RespectEqsU. auto.
-  rewrite join_ctxs_insert_var, join_ctx_tctx_insert_var.
-  erewrite handle_tmpl_shift. erewrite handle_tmpl_shift.
+  rewrite join_ctxs_insert, join_ctx_tctx_insert.
+  erewrite handle_t_shift. erewrite handle_t_shift.
   assert (tctx_len Z+(ctx_len Γ'+i) = i+ctx_len Γ'+tctx_len Z) by omega.
   rewrite H5. apply IHeq.
   all: inv H2. all: try eassumption.
@@ -513,7 +445,7 @@ with ceq_shift_typesafe Γ C c1 c2 A0 :
 
 Proof.
 all: intros orig;
-assert (ctx_insert_var Γ A0 0 = CtxU Γ A0) by (destruct Γ; auto);
+assert (ctx_insert Γ A0 0 = CtxU Γ A0) by (destruct Γ; auto);
 rewrite <-H.
 apply v_insert_typesafe. assumption.
 apply c_insert_typesafe. assumption.
@@ -522,6 +454,7 @@ apply respects_insert_typesafe. assumption.
 apply veq_insert_typesafe. assumption.
 apply ceq_insert_typesafe. assumption.
 Qed.
+
 
 Lemma v_join_ctx_tctx_typesafe Γ Z D v A :
   has_vtype Γ v A -> wf_tctx Z -> wf_ctype D ->
@@ -534,6 +467,7 @@ intros; induction Z; simpl.
   all: inv H0; try apply WfTyFun; auto.
 Qed.
 
+
 Lemma v_join_ctxs_typesafe Γ Γ' v A :
   has_vtype Γ v A -> wf_ctx Γ' -> 
   has_vtype (join_ctxs Γ Γ') (Sub.v_shift v (ctx_len Γ') 0) A.
@@ -543,6 +477,7 @@ intros; induction Γ'; simpl.
 + assert (S(ctx_len Γ')=ctx_len Γ'+1) by omega. rewrite H1.
   rewrite <-v_shift_shift. apply v_shift_typesafe; inv H0; auto.
 Qed.
+
 
 Lemma v_join_all_ctxs_typesafe Γ Γ' Z D v A :
   has_vtype Γ v A -> wf_ctx Γ' -> wf_tctx Z -> wf_ctype D ->
@@ -562,32 +497,32 @@ Qed.
 Fixpoint v_remove_typesafe 
   Γ v A (orig : has_vtype Γ v A) i {struct orig} :
   v_no_var v i ->
-  has_vtype (ctx_remove_var Γ i) (Sub.v_negshift v 1 i) A
+  has_vtype (ctx_remove Γ i) (Sub.v_negshift v 1 i) A
 
 with c_remove_typesafe 
   Γ c C (orig : has_ctype Γ c C) i {struct orig} :
   c_no_var c i ->
-  has_ctype (ctx_remove_var Γ i) (Sub.c_negshift c 1 i) C
+  has_ctype (ctx_remove Γ i) (Sub.c_negshift c 1 i) C
 
 with h_remove_typesafe 
   Γ h Σ D (orig : has_htype Γ h Σ D) i {struct orig} :
   h_no_var h i ->
-  has_htype (ctx_remove_var Γ i) (Sub.h_negshift h 1 i) Σ D
+  has_htype (ctx_remove Γ i) (Sub.h_negshift h 1 i) Σ D
 
 with respects_remove_typesafe
   Γ h Σ D E (orig: respects Γ h Σ D E) A_ins i {struct orig} :
   has_htype Γ h Σ D -> h_no_var h i -> wf_vtype A_ins ->
-  respects (ctx_remove_var Γ i) (Sub.h_negshift h 1 i) Σ D E
+  respects (ctx_remove Γ i) (Sub.h_negshift h 1 i) Σ D E
 
 with veq_remove_typesafe
   Γ A v1 v2 (orig: veq A Γ v1 v2) A_ins i {struct orig} :
   wf_vtype A_ins -> v_no_var v1 i -> v_no_var v2 i ->
-  veq A (ctx_remove_var Γ i) (Sub.v_negshift v1 1 i) (Sub.v_negshift v2 1 i)
+  veq A (ctx_remove Γ i) (Sub.v_negshift v1 1 i) (Sub.v_negshift v2 1 i)
 
 with ceq_remove_typesafe
   Γ C c1 c2 (orig: ceq C Γ c1 c2) A_ins i {struct orig} :
   wf_vtype A_ins -> c_no_var c1 i -> c_no_var c2 i ->
-  ceq C (ctx_remove_var Γ i) (Sub.c_negshift c1 1 i) (Sub.c_negshift c2 1 i).
+  ceq C (ctx_remove Γ i) (Sub.c_negshift c1 1 i) (Sub.c_negshift c2 1 i).
 Proof.
 all: rename v_remove_typesafe into V; rename c_remove_typesafe into CI.
 all: rename h_remove_typesafe into HC; rename respects_remove_typesafe into R.
@@ -597,33 +532,32 @@ intros no_var. simpl in no_var. apply TypeV; inv orig.
 { apply ctx_remove_wf. assumption. }
 { assumption. }
 destruct H1.
-+ clear V CI HC R VE CE. simpl. apply TypeUnit.
-+ clear V CI HC R VE CE. simpl. apply TypeInt.
-+ clear V CI HC R VE CE. simpl. destruct (i <=? n) eqn:cmp.
++ clear V CI HC R VE CE. simpl. 
+  apply TypeUnit.
++ clear V CI HC R VE CE. simpl. 
+  apply TypeInt.
++ clear V CI HC R VE CE. simpl. 
+  destruct (i <=? n) eqn:cmp.
   - apply TypeVar. rewrite <-get_ctx_remove_changed; apply leb_complete in cmp.
     * destruct n. destruct no_var. omega.
       simpl. assert (n-0=n) by omega. rewrite H2. assumption.
     * destruct cmp. destruct no_var. reflexivity. omega.
   - apply TypeVar. rewrite <-get_ctx_remove_unchanged.
     assumption. apply leb_iff_conv in cmp. assumption.
-+ specialize (V _ _ _ H1) as IHv1.
-  specialize (V _ _ _ H2) as IHv2.
++ specialize (V _ _ _ H1) as IHv1. specialize (V _ _ _ H2) as IHv2.
   clear V CI HC R VE CE. simpl. destruct no_var. apply TypePair; auto.
-+ specialize (V _ _ _ H1) as IHv.
-  clear V CI HC R VE CE. simpl. apply TypeInl. auto.
-+ specialize (V _ _ _ H1) as IHv.
-  clear V CI HC R VE CE. simpl. apply TypeInr. auto.
++ specialize (V _ _ _ H1) as IHv. clear V CI HC R VE CE. apply TypeInl. auto.
++ specialize (V _ _ _ H1) as IHv. clear V CI HC R VE CE. apply TypeInr. auto.
 + specialize (CI _ _ _ H1) as IHc.
-  clear V CI HC R VE CE.
-  simpl. apply TypeFun. rewrite ctx_remove_extend. auto.
-+ specialize (HC _ _ _ _ H2) as IHh.
+  clear V CI HC R VE CE. simpl. 
+  apply TypeFun. rewrite ctx_remove_extend. auto.
++ specialize (HC _ _ _ _ H2) as IHh. 
   specialize (CI _ _ _ H1) as IHc.
   specialize (R _ _ _ _ _ H3) as IHr.
   clear V CI HC R VE CE. simpl. destruct no_var.
   apply TypeHandler. rewrite ctx_remove_extend. all: eauto.
 + specialize (V _ _ _ H1) as IHv.
-  clear V CI HC R VE CE.
-  eapply TypeVSubtype; auto.
+  clear V CI HC R VE CE. eapply TypeVSubtype; auto.
 }{
 intros no_var. simpl in no_var. apply TypeC; inv orig.
 { apply ctx_remove_wf. assumption. }
@@ -635,32 +569,29 @@ destruct H1.
   clear V CI HC R VE CE. simpl. apply TypeAbsurd. apply IHv; assumption.
 + specialize (V _ _ _ H1) as IHv.
   specialize (CI _ _ _ H2) as IHc.
-  clear V CI HC R VE CE. simpl. destruct no_var. eapply TypeΠMatch.
-  - apply IHv. assumption.
-  - do 2 rewrite ctx_remove_extend. auto.
-+ specialize (V _ _ _ H1) as IHv.
+  clear V CI HC R VE CE. simpl. destruct no_var. eapply TypeΠMatch; auto.
+  do 2 rewrite ctx_remove_extend. auto.
++ specialize (V _ _ _ H1) as IHv. 
   specialize (CI _ _ _ H2) as IHc1.
   specialize (CI _ _ _ H3) as IHc2.
   clear V CI HC R VE CE. simpl. destruct no_var. destruct H5.
   eapply TypeΣMatch; try rewrite ctx_remove_extend; auto.
-+ specialize (CI _ _ _ H1) as IHc1.
++ specialize (CI _ _ _ H1) as IHc1. 
   specialize (CI _ _ _ H2) as IHc2.
-  clear V CI HC R VE CE. simpl. destruct no_var. eapply TypeDoBind.
-  - auto.
-  - rewrite ctx_remove_extend. auto.
-+ specialize (V _ _ _ H1) as IHv.
+  clear V CI HC R VE CE. simpl. destruct no_var. eapply TypeDoBind; auto.
+  rewrite ctx_remove_extend. auto.
++ specialize (V _ _ _ H1) as IHv. 
   specialize (V _ _ _ H2) as IHv0.
   clear V CI HC R VE CE. simpl. destruct no_var. eapply TypeApp; auto.
-+ specialize (V _ _ _ H1) as IHv.
++ specialize (V _ _ _ H1) as IHv. 
   specialize (CI _ _ _ H2) as IHc.
-  clear V CI HC R VE CE.
-  simpl. destruct no_var. eapply TypeHandle; auto.
-+ specialize (CI _ _ _ H1) as IHc1.
+  clear V CI HC R VE CE. simpl. destruct no_var. eapply TypeHandle; auto.
++ specialize (CI _ _ _ H1) as IHc1. 
   specialize (CI _ _ _ H2) as IHc2.
   clear V CI HC R VE CE. simpl. destruct no_var. eapply TypeLetRec.
   - do 2 rewrite ctx_remove_extend. auto.
   - rewrite ctx_remove_extend. auto.
-+ specialize (V _ _ _ H2) as IHv.
++ specialize (V _ _ _ H2) as IHv. 
   specialize (CI _ _ _ H3) as IHc.
   clear V CI HC R VE CE. simpl. destruct no_var. eapply TypeOp; eauto.
   rewrite ctx_remove_extend. auto.
@@ -670,34 +601,32 @@ destruct H1.
 intros no_var; simpl; apply TypeH; inv orig.
 apply ctx_remove_wf. all: auto. destruct H2.
 + simpl. clear V CI HC R VE CE. apply TypeCasesØ.
-+ specialize (HC _ _ _ _ H3) as IHh.
++ specialize (HC _ _ _ _ H3) as IHh. 
   specialize (CI _ _ _ H4) as IHc.
   clear V CI HC R VE CE. simpl. apply TypeCasesU; inv no_var; auto.
-  - apply h_negshift_find_op_None. auto.
+  - apply negshift_find_None. auto.
   - do 2 rewrite ctx_remove_extend. auto.
 }{
 intros types no_var wfins. apply Respects.
 { clear V CI HC R VE CE. apply ctx_remove_wf. inv types. assumption. }
-{ inv orig. assumption. }
-{ inv orig. assumption. }
-{ inv orig. assumption. }
+all: try (inv orig; assumption).
 inv orig. destruct H3.
 + clear V CI HC R VE CE. apply RespectEqsØ.
-+ specialize (R _ _ _ _ _ H3) as IHres.
++ specialize (R _ _ _ _ _ H3) as IHres. 
   specialize (CE _ _ _ _ H4) as IHeq.
   clear V CI HC R VE CE. apply RespectEqsU. eauto.
-  rewrite join_ctxs_remove_var. rewrite join_ctx_tctx_remove_var.
-  erewrite handle_tmpl_negshift. erewrite handle_tmpl_negshift.
+  rewrite join_ctxs_remove. rewrite join_ctx_tctx_remove.
+  erewrite handle_t_negshift. erewrite handle_t_negshift.
   all: eauto; inv H2; auto.
   assert (tctx_len Z+(ctx_len Γ'+i) = i+ctx_len Γ'+tctx_len Z) by omega.
-  rewrite H2. eapply IHeq. eauto.
-  all: eapply handle_tmpl_no_var; eauto.
+  rewrite H2. eapply IHeq. eauto. all: eapply handle_t_no_var; eauto.
 }{
   clear V CI HC R VE CE. inv orig. inv H1.
 }{
   clear V CI HC R VE CE. inv orig. inv H1.
 }
 Qed.
+
 
 Fixpoint v_sub_typesafe 
   Γ v A (orig: has_vtype Γ v A) i v_s A_s {struct orig}:
@@ -735,138 +664,96 @@ all: rename veq_sub_typesafe into VE; rename ceq_sub_typesafe into CE.
 {
 intros gets vsty. apply TypeV; inv orig.
 assumption. assumption. destruct H1.
-+ clear V CI HC R VE CE.
++ clear V CI HC R VE CE. 
   simpl. apply TypeUnit.
-+ clear V CI HC R VE CE.
++ clear V CI HC R VE CE. 
   simpl. apply TypeInt.
 + clear V CI HC R VE CE.
   simpl. destruct (n =? i) eqn:cmp.
   - apply Nat.eqb_eq in cmp. rewrite cmp in *. rewrite H1 in gets.
     injection gets. intro. subst. inv vsty. assumption.
   - apply TypeVar. assumption.
-+ specialize (V _ _ _ H1) as IHv1.
++ specialize (V _ _ _ H1) as IHv1. 
   specialize (V _ _ _ H2) as IHv2.
-  clear V CI HC R VE CE.
-  simpl. apply TypePair.
-  eapply IHv1; eauto.
-  eapply IHv2; eauto.
-+ specialize (V _ _ _ H1) as IHv.
-  clear V CI HC R VE CE.
-  simpl. apply TypeInl. eapply IHv; eauto.
-+ specialize (V _ _ _ H1) as IHv.
-  clear V CI HC R VE CE.
-  simpl. apply TypeInr. eapply IHv; eauto.
-+ specialize (CI _ _ _ H1) as IHc.
+  clear V CI HC R VE CE. simpl. apply TypePair; eauto.
++ specialize (V _ _ _ H1) as IHv. clear V CI HC R VE CE. apply TypeInl; eauto.
++ specialize (V _ _ _ H1) as IHv. clear V CI HC R VE CE. apply TypeInr; eauto.
++ specialize (CI _ _ _ H1) as IHc. 
   specialize (V _ _ _ vsty) as IHvs.
-  clear V CI HC R VE CE.
-  simpl. apply TypeFun. eapply IHc. eauto.
-  apply v_shift_typesafe. assumption. inv H0. assumption.
-+ specialize (HC _ _ _ _ H2) as IHh.
+  clear V CI HC R VE CE. simpl.
+  apply TypeFun. eapply IHc. eauto. inv H0. apply v_shift_typesafe; auto.
++ specialize (HC _ _ _ _ H2) as IHh. 
   specialize (CI _ _ _ H1) as IHc.
   specialize (R _ _ _ _ _ H3) as IHr.
-  clear V CI HC R VE CE.
-  simpl. apply TypeHandler.
-  - eapply IHc. exact gets.
-    apply v_shift_typesafe. assumption. inv H0. inv H6. assumption.
-  - eauto.
-  - eauto.
+  clear V CI HC R VE CE. simpl. apply TypeHandler; eauto. eapply IHc. 
+  exact gets. inv H0. inv H6. apply v_shift_typesafe; assumption.
 + specialize (V _ _ _ H1) as IHv.
-  clear V CI HC R VE CE.
-  eapply TypeVSubtype.
-  - eapply IHv; eauto.
-  - assumption. 
+  clear V CI HC R VE CE. eapply TypeVSubtype; eauto.
 }{
 intros gets vsty. apply TypeC; inv orig.
 assumption. assumption. destruct H1.
-+ specialize (V _ _ _ H1) as IHv.
-  clear V CI HC R VE CE.
-  simpl. apply TypeRet. eapply IHv; eauto.
-+ specialize (V _ _ _ H1) as IHv.
-  clear V CI HC R VE CE.
-  simpl. apply TypeAbsurd. eapply IHv; eauto.
-+ specialize (V _ _ _ H1) as IHv.
++ specialize (V _ _ _ H1) as IHv. 
+  clear V CI HC R VE CE. apply TypeRet; eauto.
++ specialize (V _ _ _ H1) as IHv. 
+  clear V CI HC R VE CE. apply TypeAbsurd; eauto.
++ specialize (V _ _ _ H1) as IHv. 
   specialize (CI _ _ _ H2) as IHc.
-  clear V CI HC R VE CE.
-  simpl. eapply TypeΠMatch.
-  - eauto.
-  - eapply IHc. exact gets. 
-    rewrite <-(v_shift_shift 1 1 0).
+  clear V CI HC R VE CE. simpl. eapply TypeΠMatch; eauto.
+  - eapply IHc. exact gets. rewrite <-(v_shift_shift 1 1 0).
     apply v_shift_typesafe. apply v_shift_typesafe. assumption.
     all: inv H1; inv H4; assumption.
-+ specialize (V _ _ _ H1) as IHv.
++ specialize (V _ _ _ H1) as IHv. 
   specialize (CI _ _ _ H2) as IHc1.
   specialize (CI _ _ _ H3) as IHc2.
-  clear V CI HC R VE CE.
-  simpl. eapply TypeΣMatch.
-  - eauto.
-  - eapply IHc1. exact gets.
-    apply v_shift_typesafe. assumption.
-    inv H1. inv H5. assumption. 
-  - eapply IHc2. exact gets.
-    apply v_shift_typesafe. assumption.
-    inv H1. inv H5. assumption. 
-+ specialize (CI _ _ _ H1) as IHc1.
+  clear V CI HC R VE CE. simpl. eapply TypeΣMatch. eauto.
+  - eapply IHc1. exact gets. inv H1. inv H5. apply v_shift_typesafe; auto. 
+  - eapply IHc2. exact gets. inv H1. inv H5. apply v_shift_typesafe; auto. 
++ specialize (CI _ _ _ H1) as IHc1. 
   specialize (CI _ _ _ H2) as IHc2.
-  clear V CI HC R VE CE.
-  simpl. eapply TypeDoBind.
-  - eauto.
-  - eapply IHc2. exact gets.
-    apply v_shift_typesafe. assumption.
-    inv H1. inv H4. assumption.
-+ specialize (V _ _ _ H1) as IHv.
+  clear V CI HC R VE CE. simpl. eapply TypeDoBind. eauto.
+  eapply IHc2. exact gets. inv H1. inv H4. apply v_shift_typesafe; auto. 
++ specialize (V _ _ _ H1) as IHv. 
   specialize (V _ _ _ H2) as IHv0.
-  clear V CI HC R VE CE.
-  simpl. eapply TypeApp; eauto.
-+ specialize (V _ _ _ H1) as IHv.
+  clear V CI HC R VE CE. simpl. eapply TypeApp; eauto.
++ specialize (V _ _ _ H1) as IHv. 
   specialize (CI _ _ _ H2) as IHc.
-  clear V CI HC R VE CE.
-  simpl. eapply TypeHandle; eauto.
-+ specialize (CI _ _ _ H1) as IHc1.
+  clear V CI HC R VE CE. simpl. eapply TypeHandle; eauto.
++ specialize (CI _ _ _ H1) as IHc1. 
   specialize (CI _ _ _ H2) as IHc2.
-  clear V CI HC R VE CE.
-  simpl. eapply TypeLetRec.
-  - eapply IHc1. exact gets.
-    rewrite <-(v_shift_shift 1 1 0).
+  clear V CI HC R VE CE. simpl. eapply TypeLetRec.
+  - eapply IHc1. exact gets. rewrite <-(v_shift_shift 1 1 0).
     apply v_shift_typesafe. apply v_shift_typesafe. assumption.
     all: inv H1; inv H3. 2: assumption. inv H7. assumption. 
-  - eapply IHc2. exact gets.
-    apply v_shift_typesafe. assumption.
-    inv H1. inv H3. assumption.
-+ specialize (V _ _ _ H2) as IHv.
+  - eapply IHc2. exact gets. inv H1. inv H3. apply v_shift_typesafe; auto.
++ specialize (V _ _ _ H2) as IHv. 
   specialize (CI _ _ _ H3) as IHc.
-  clear V CI HC R VE CE.
-  simpl. eapply TypeOp. exact H1.
-  - eauto.
-  - eapply IHc. exact gets. 
-    apply v_shift_typesafe. assumption.
-    inv H3. inv H4. assumption.
+  clear V CI HC R VE CE. simpl. eapply TypeOp; eauto.
+  eapply IHc. exact gets. inv H3. inv H4. apply v_shift_typesafe; auto.
 + specialize (CI _ _ _ H1) as IHc.
-  clear V CI HC R VE CE.
-  eapply TypeCSubtype; eauto.
+  clear V CI HC R VE CE. eapply TypeCSubtype; eauto.
 }{
 intros gets vsty; simpl; apply TypeH; inv orig.
-assumption. assumption. assumption.
+all: try assumption.
 destruct H2.
-+ clear V CI HC R VE CE. apply TypeCasesØ.
-+ specialize (HC _ _ _ _ H3) as IHh.
++ clear V CI HC R VE CE. 
+  apply TypeCasesØ.
++ specialize (HC _ _ _ _ H3) as IHh. 
   specialize (CI _ _ _ H4) as IHc.
-  clear V CI HC R VE CE.
-  simpl. apply TypeCasesU.
-  - rewrite h_sub_find_op_None; auto.
-  - eauto.
-  - eapply IHc. exact gets.
-    rewrite <-(v_shift_shift 1 1 0).
+  clear V CI HC R VE CE. simpl. apply TypeCasesU; eauto.
+  - rewrite sub_find_None; auto.
+  - eapply IHc. exact gets. rewrite <-(v_shift_shift 1 1 0).
     apply v_shift_typesafe. apply v_shift_typesafe. assumption.
     all: inv H0. 2: assumption. apply WfTyFun; assumption.
 }{
 intros htys gets vsty; simpl. apply Respects; inv orig.
 all: try assumption.
 destruct H3.
-+ clear V CI HC R VE CE. apply RespectEqsØ.
-+ specialize (CE _ _ _ _ H4) as IHc.
++ clear V CI HC R VE CE. 
+  apply RespectEqsØ.
++ specialize (CE _ _ _ _ H4) as IHc. 
   specialize (R _ _ _ _ _ H3) as IHr.
   clear V CI HC R VE CE.
-  apply RespectEqsU. eauto. erewrite handle_tmpl_sub. erewrite handle_tmpl_sub.
+  apply RespectEqsU. eauto. erewrite handle_t_sub. erewrite handle_t_sub.
   eapply IHc. all: inv H2; eauto. clear IHc IHr.
   * erewrite <-get_join_ctx_tctx, <-get_join_ctxs. eauto.
   * eapply v_join_all_ctxs_typesafe; auto.
