language_formalisation/type_system/type_lemmas.v
@@ -1,16 +1,16 @@
-(* Add LoadPath "C:\Users\Ziga\Documents\Ziga_podatki\PHD\language_formalisation\syntax". *)
-(* Add LoadPath "C:\Users\Ziga\Documents\Ziga_podatki\PHD\language_formalisation\substitution". *)
-(* Add LoadPath "C:\Users\Ziga\Documents\Ziga_podatki\PHD\language_formalisation\type_system". *)
-(* Add LoadPath "C:\Users\Ziga\Documents\Ziga_podatki\PHD\language_formalisation\operational_semantics". *)
-Add LoadPath "E:\Ziga_Podatki\faks\PHD\language_formalisation\syntax".
-Add LoadPath "E:\Ziga_Podatki\faks\PHD\language_formalisation\substitution".
-Add LoadPath "E:\Ziga_Podatki\faks\PHD\language_formalisation\type_system".
-Add LoadPath "E:\Ziga_Podatki\faks\PHD\language_formalisation\operational_semantics".
-Require Export declarational subtyping_lemmas substitution_lemmas 
-  type_aux_lemmas operational_semantics.
-
+Add LoadPath "C:\Users\Ziga\Documents\Ziga_podatki\PHD\language_formalisation\syntax".
+Add LoadPath "C:\Users\Ziga\Documents\Ziga_podatki\PHD\language_formalisation\substitution".
+Add LoadPath "C:\Users\Ziga\Documents\Ziga_podatki\PHD\language_formalisation\type_system".
+Add LoadPath "C:\Users\Ziga\Documents\Ziga_podatki\PHD\language_formalisation\operational_semantics".
+(* Add LoadPath "E:\Ziga_Podatki\faks\PHD\language_formalisation\syntax". *)
+(* Add LoadPath "E:\Ziga_Podatki\faks\PHD\language_formalisation\substitution". *)
+(* Add LoadPath "E:\Ziga_Podatki\faks\PHD\language_formalisation\type_system". *)
+(* Add LoadPath "E:\Ziga_Podatki\faks\PHD\language_formalisation\operational_semantics". *)
+Require Export type_aux_lemmas operational_semantics.
 
 Ltac inv H := inversion H; clear H; subst.
+
+(* ==================== Substitution Lemma ==================== *)
 
 Fixpoint v_subs_out_typesafe Γ v A v_s A_s {struct v}:
   has_vtype (CtxU Γ A_s) v A -> has_vtype Γ v_s A_s ->
@@ -26,91 +26,78 @@ with h_subs_out_typesafe Γ h Σ D v_s A_s {struct h}:
 Proof.
 {
 intros orig sub. unfold v_subs_out.
-assert (Γ = ctx_remove_var (CtxU Γ A_s) 0) by auto.
+assert (Γ = ctx_remove (CtxU Γ A_s) 0) by auto.
 rewrite H. apply v_remove_typesafe.
 - eapply v_sub_typesafe. assumption. simpl. reflexivity.
   apply v_shift_typesafe. assumption. inv sub. assumption.
-- apply v_no_var_subbed. apply v_shift_makes_no_var.
+- apply v_sub_makes_no_var. apply v_shift_makes_no_var.
 }{
 intros orig sub. unfold c_subs_out.
-assert (Γ = ctx_remove_var (CtxU Γ A_s) 0) by auto.
+assert (Γ = ctx_remove (CtxU Γ A_s) 0) by auto.
 rewrite H. apply c_remove_typesafe.
 - eapply c_sub_typesafe. assumption. simpl. reflexivity.
   apply v_shift_typesafe. assumption. inv sub. assumption.
-- apply c_no_var_subbed. apply v_shift_makes_no_var.
+- apply c_sub_makes_no_var. apply v_shift_makes_no_var.
 }{
 intros orig sub. unfold h_subs_out.
-assert (Γ = ctx_remove_var (CtxU Γ A_s) 0) by auto.
+assert (Γ = ctx_remove (CtxU Γ A_s) 0) by auto.
 rewrite H. apply h_remove_typesafe.
 - eapply h_sub_typesafe. assumption. simpl. reflexivity.
   apply v_shift_typesafe. assumption. inv sub. assumption.
-- apply h_no_var_subbed. apply v_shift_makes_no_var.
+- apply h_sub_makes_no_var. apply v_shift_makes_no_var.
 }
 Qed.
 
+(* ==================== Preservation ==================== *)
 
-Lemma preservation Γ c c' C:
+Theorem preservation Γ c c' C:
   has_ctype Γ c C -> step c c' -> has_ctype Γ c' C.
 Proof.
 intros orig step. revert C orig. 
 induction step; intros C orig.
 + unfold c_subs2_out. apply shape_prodmatch in orig.
-  destruct orig as [A [B [pair]]].
-  eapply c_subs_out_typesafe.
-  eapply c_subs_out_typesafe. exact H.
-  apply v_shift_typesafe.
-  - apply shape_pair in pair. destruct pair. assumption. 
-  - inv pair. inv H1. assumption.
-  - apply shape_pair in pair. destruct pair. assumption.
+  destruct orig as [A [B [pair]]]. apply shape_pair in pair. destruct pair.
+  eapply c_subs_out_typesafe. eapply c_subs_out_typesafe.
+  all: eauto. inv H0. apply v_shift_typesafe; auto.
 + unfold c_subs2_out. apply shape_summatch in orig.
-  destruct orig as [A [B [vtyped [inl]]]].
-  eapply c_subs_out_typesafe. exact inl.
-  apply shape_sum_inl in vtyped. assumption.
+  destruct orig as [A [B [vty [inl]]]].
+  eapply c_subs_out_typesafe. exact inl. apply shape_sum_inl in vty. auto.
 + unfold c_subs2_out. apply shape_summatch in orig.
-  destruct orig as [A [B [vtyped [inl]]]].
-  eapply c_subs_out_typesafe. exact H.
-  apply shape_sum_inr in vtyped. assumption.
+  destruct orig as [A [B [vty [_]]]].
+  eapply c_subs_out_typesafe. exact H. apply shape_sum_inr in vty. auto.
 + apply shape_app in orig. destruct orig as [A [f]].
-  eapply c_subs_out_typesafe. exact f. assumption.
+  eapply c_subs_out_typesafe; eauto.
 + apply shape_letrec in orig. destruct orig as [A [C' [c1ty]]].
-  eapply c_subs_out_typesafe. exact H.
-  apply TypeV. inv c1ty.
+  eapply c_subs_out_typesafe; eauto. apply TypeV. inv c1ty.
   inv H. inv H3. assumption. inv H. inv H0. assumption.  
   apply TypeFun. apply TypeC. 
   - inv c1ty. inv H0. assumption.
   - inv c1ty. assumption.
   - eapply TypeLetRec. 2: exact c1ty.
     assert (CtxU (CtxU (CtxU Γ A) A) (TyFun A C') 
-      = ctx_insert_var (CtxU (CtxU Γ A) (TyFun A C')) A 2)
-    as insertion.
-    { simpl. destruct Γ; auto. }
-    rewrite insertion.
-    apply c_insert_typesafe. assumption.
+      = ctx_insert (CtxU (CtxU Γ A) (TyFun A C')) A 2)
+    as insertion. { simpl. destruct Γ; auto. }
+    rewrite insertion. apply c_insert_typesafe. assumption.
     inv H. inv H0. inv H5. assumption.
 + destruct C as (A, Σ, E) eqn:e. apply shape_dobind in orig.
   destruct orig as [A' [c1ty]].
-  apply TypeC. inv c1ty. assumption. inv H. assumption.
-  eapply TypeDoBind. 2: exact H. auto.
+  apply TypeC. inv c1ty. 3 : eapply TypeDoBind. all: eauto. inv H. auto.
 + destruct C as (A, Σ, E) eqn:e. apply shape_dobind in orig.
-  destruct orig as [A' [c1ty]].
-  eapply c_subs_out_typesafe. exact H.
+  destruct orig as [A' [c1ty]]. eapply c_subs_out_typesafe. eauto.
   apply shape_ret in c1ty. assumption.
 + destruct C as (A, Σ, E) eqn:e. apply shape_dobind in orig.
   destruct orig as [A' [c1ty]]. eapply shape_op in c1ty.
-  destruct c1ty as [Aop [Bop [gets [vty]]]].
-  apply TypeC.
+  destruct c1ty as [Aop [Bop [gets [vty]]]]. apply TypeC.
   - inv H. inv H1. assumption.
   - inv H. assumption.
-  - eapply TypeOp. exact gets. assumption.
-    eapply TypeC. inv H0. assumption. inv H. assumption.
+  - eapply TypeOp; eauto. eapply TypeC. inv H0. assumption. inv H. assumption.
     eapply TypeDoBind. exact H0.
-    assert (CtxU (CtxU Γ Bop) A' = ctx_insert_var (CtxU Γ A') Bop 1).
+    assert (CtxU (CtxU Γ Bop) A' = ctx_insert (CtxU Γ A') Bop 1).
     { simpl. destruct Γ; auto. }
-    rewrite H1. apply c_insert_typesafe. assumption.
-    inv H0. inv H2. assumption.
+    rewrite H1. apply c_insert_typesafe. assumption. inv H0. inv H2. assumption.
 + eapply shape_handle in orig. destruct orig as [C' [hty]]. 
   apply TypeC. inv hty. assumption. inv hty. inv H1. assumption.
-  eapply TypeHandle. exact hty.  apply IHstep. assumption.
+  eapply TypeHandle; eauto.
 + eapply shape_handle in orig. rename C into D. destruct orig as [C[hty]].
   destruct C as (A, Σ, E). eapply shape_handler in hty as hty'. 
   destruct hty' as [Σ'[D'[retty[hcty[r[st]]]]]]. eapply shape_ret in H.
@@ -133,54 +120,52 @@ induction step; intros C orig.
   instantiate (1:= TyFun Bop D').
   unfold c_subs2_out. eapply c_subs_out_typesafe.
   instantiate (1:= Aop).
-  - eapply sig_subtype_gets_Some in gets; eauto.
+  - eapply sig_subtype_get_Some in gets; eauto.
     destruct gets as [A'[B'[gets']]]. inv H8.
     eapply ctx_subtype_ctype. eapply case_has_type; eauto.
     * apply WfCtxU. apply WfCtxU. 2: apply WfTyFun. all: auto.
     * apply SubtypeCtxU. apply SubtypeCtxU.
       apply ctx_subtype_refl; auto. apply SubtypeTyFun; auto.
       apply csubtype_refl. all: auto.
-  - assert (CtxU Γ (TyFun Bop D') = ctx_insert_var Γ (TyFun Bop D') 0).
+  - assert (CtxU Γ (TyFun Bop D') = ctx_insert Γ (TyFun Bop D') 0).
     { destruct Γ; simpl; reflexivity. }
-    rewrite H8. eapply v_insert_typesafe. assumption.
-    apply WfTyFun; assumption.
-  - apply TypeV. assumption. apply WfTyFun; assumption.
-    eapply TypeFun. apply TypeC. apply WfCtxU. all: try assumption.
+    rewrite H8. eapply v_insert_typesafe. auto. apply WfTyFun; auto.
+  - apply TypeV. auto. apply WfTyFun; auto.
+    eapply TypeFun. apply TypeC. apply WfCtxU. all: auto.
     eapply TypeHandle. 2: exact H5.
-    assert (CtxU Γ Bop = ctx_insert_var Γ Bop 0).
-    { destruct Γ; simpl; reflexivity. }
-    rewrite H8. eapply v_insert_typesafe. 2: assumption.
-    apply TypeV. assumption. apply WfTyHandler. inv H0. assumption. assumption.
+    assert (CtxU Γ Bop = ctx_insert Γ Bop 0) by (destruct Γ; simpl; auto).
+    rewrite H8. eapply v_insert_typesafe. 2: auto.
+    apply TypeV. auto. apply WfTyHandler. inv H0. auto. auto.
     eapply TypeVSubtype. instantiate (1:=(TyHandler (CTy A Σ' E) D'));
     inv H5; inv H10; inv H0.
-    * apply TypeV. assumption. apply WfTyHandler. apply WfCTy; auto.
-      inv hcty. assumption. eapply wf_eqs_sig_subtype; eauto.
-      inv hcty. assumption. inv hcty. assumption.
-      apply TypeHandler; auto.
-    * apply SubtypeTyHandler. apply SubtypeCTy. 2: assumption.
-      apply vsubtype_refl. inv H5. inv H10. assumption.
+    * apply TypeV. auto. apply WfTyHandler. apply WfCTy; auto.
+      all: try (inv hcty; assumption). eapply wf_eqs_sig_subtype; eauto.
+      inv hcty. assumption. apply TypeHandler; auto.
+    * apply SubtypeTyHandler. apply SubtypeCTy. 2: auto.
+      apply vsubtype_refl. inv H5. inv H10. auto.
       eapply eqs_subtype_refl. inv H5. inv H10. eauto.
       apply csubtype_refl. assumption.
 Qed.
 
+(* ==================== Progress ==================== *)
 
-Lemma progress c C:
+Theorem progress c C:
   has_ctype CtxØ c C ->
   (exists v, c = Ret v) \/
   (exists o v y c', c = Op o v y c') \/
   (exists c', step c c'). 
 Proof.
 revert C. induction c; intros C orig.
-+ left. exists v. reflexivity.
++ left. eauto.
 + apply shape_absurd in orig. apply shape_empty in orig as shape. 
-  destruct shape as [x [i]]. subst. apply shape_var_empty_ctx in orig.
+  destruct shape as [x [i]]. subst. apply shape_var_ctx_empty in orig.
   destruct orig.
 + rename v0 into x. rename v1 into y. right. right. clear IHc.
   eapply shape_prodmatch in orig. destruct orig as [A [B [vty]]].
   eapply shape_prod_full in vty as shape. 2: reflexivity.
   destruct shape.
   - destruct H0 as [name [db_i]]. rewrite H0 in *.
-    apply shape_var_empty_ctx in vty. destruct vty.
+    apply shape_var_ctx_empty in vty. destruct vty.
   - destruct H0 as [v1[v2[same[ty1]]]]. subst.
     eexists. apply Step_ΠMatch.
 + right. right. rename v0 into x. rename v1 into y. clear IHc1 IHc2.
@@ -188,7 +173,7 @@ revert C. induction c; intros C orig.
   eapply shape_sum_full in vty as shape. 2: reflexivity.
   destruct shape. 2: destruct H0.
   - destruct H0 as [name [db_i]]. rewrite H0 in *.
-    apply shape_var_empty_ctx in vty. destruct vty.
+    apply shape_var_ctx_empty in vty. destruct vty.
   - destruct H0 as [v' [same]]. rewrite same. eexists. apply Step_ΣMatch_Inl.
   - destruct H0 as [v' [same]]. rewrite same. eexists. apply Step_ΣMatch_Inr.
 + right. right.
@@ -196,9 +181,9 @@ revert C. induction c; intros C orig.
   destruct orig as [A [fty]]. eapply shape_tyfun_full in fty as ffty.
   2: reflexivity. destruct ffty.
   - destruct H0 as [name [db_i]]. rewrite H0 in *.
-    apply shape_var_empty_ctx in fty. destruct fty.
+    apply shape_var_ctx_empty in fty. destruct fty.
   - destruct H0 as [x [c [same]]]. subst. eexists. apply Step_App.
-+ right. left. exists o. exists v. exists v0. exists c. reflexivity.
++ right. left. eauto.
 + right. right. rename v into f. rename v0 into x. clear IHc1 IHc2.
   eexists. apply Step_LetRec.
 + right. right. rename v into x. clear IHc2. destruct C as (A, Σ, E). 
@@ -213,13 +198,13 @@ revert C. induction c; intros C orig.
   destruct C as (A, Σ, E). eapply shape_tyhandler_full in hty as shape.
   2: reflexivity. destruct shape.
   { destruct H0 as [x [i]]. subst.
-    apply shape_var_empty_ctx in hty. contradiction. }
+    apply shape_var_ctx_empty in hty. contradiction. }
   destruct H0 as [x[c_r[h[Σ'[D'[same[crty]]]]]]]. subst.
   destruct H'. 2: destruct H1.
   - destruct H1 as [v]. subst. eexists. apply Step_Handle_Ret.   
   - destruct H1 as [op[v[y[c']]]]. subst. destruct H0 as [hcsty[r[sigsty]]].
     apply shape_op in H. destruct H as [A_op[B_op[gets]]].
-    eapply sig_subtype_gets_Some in gets. 2: exact sigsty.
+    eapply sig_subtype_get_Some in gets. 2: exact sigsty.
     destruct gets as [A'[B'[gets']]].
     eapply h_has_case in hcsty. 2: exact gets'.
     destruct hcsty as [x'[k'[c_op]]].
