language_formalisation/type_system/wf_lemmas.v
@@ -1,69 +1,59 @@
-(* Add LoadPath "C:\Users\Ziga\Documents\Ziga_podatki\PHD\language_formalisation\syntax". *)
-(* Add LoadPath "C:\Users\Ziga\Documents\Ziga_podatki\PHD\language_formalisation\type_system". *)
-(* Add LoadPath "C:\Users\Ziga\Documents\Ziga_podatki\PHD\language_formalisation\substitution". *)
-Add LoadPath "E:\Ziga_Podatki\faks\PHD\language_formalisation\syntax".
-Add LoadPath "E:\Ziga_Podatki\faks\PHD\language_formalisation\type_system".
-Add LoadPath "E:\Ziga_Podatki\faks\PHD\language_formalisation\substitution".
+Add LoadPath "C:\Users\Ziga\Documents\Ziga_podatki\PHD\language_formalisation\syntax".
+Add LoadPath "C:\Users\Ziga\Documents\Ziga_podatki\PHD\language_formalisation\type_system".
+Add LoadPath "C:\Users\Ziga\Documents\Ziga_podatki\PHD\language_formalisation\substitution".
+(* Add LoadPath "E:\Ziga_Podatki\faks\PHD\language_formalisation\syntax". *)
+(* Add LoadPath "E:\Ziga_Podatki\faks\PHD\language_formalisation\type_system". *)
+(* Add LoadPath "E:\Ziga_Podatki\faks\PHD\language_formalisation\substitution". *)
 
 Require Export syntax_lemmas declarational substitution_lemmas.
 
-Lemma ctx_gets_wf Γ num A : 
+
+Lemma get_vtype_wf Γ num A : 
     wf_ctx Γ -> get_vtype Γ num = Some A -> wf_vtype A.
 Proof.
-intros wf. revert num. induction wf; intros num gets.
-+ simpl in gets. discriminate.
-+ simpl in gets. destruct num.
-  - inv gets. assumption.
-  - eapply IHwf. exact gets.
+intros wf. revert num. induction wf; intros num gets; simpl in *.
+discriminate. destruct num.
+- inv gets. assumption.
+- eapply IHwf. exact gets.
 Qed.
+
 
 Lemma ctx_insert_wf Γ A i:
-  wf_ctx Γ -> wf_vtype A -> wf_ctx (ctx_insert_var Γ A i).
+  wf_ctx Γ -> wf_vtype A -> wf_ctx (ctx_insert Γ A i).
 Proof.
-revert i A; induction Γ; intros i A orig wfv.
-+ induction i; simpl.
-  * apply WfCtxU; assumption.
-  * apply WfCtxØ.
-+ induction i; simpl.
-  * apply WfCtxU; assumption.
-  * inv orig. apply WfCtxU; try apply IHΓ; assumption.
+revert i A; induction Γ; intros i A orig wfv; induction i; simpl.
+all: (try inv orig); apply WfCtxU || apply WfCtxØ; auto.
+all: apply WfCtxU || apply WfCtxØ; auto.
 Qed.
 
+
 Lemma ctx_remove_wf Γ i:
-  wf_ctx Γ -> wf_ctx (ctx_remove_var Γ i).
+  wf_ctx Γ -> wf_ctx (ctx_remove Γ i).
 Proof.
-revert i; induction Γ; intros i orig.
-+ induction i; simpl; apply WfCtxØ.
-+ induction i; simpl; inv orig.
-  * assumption.
-  * apply WfCtxU; try apply IHΓ; assumption.
+revert i; induction Γ; intros i orig; induction i; simpl.
+all: apply WfCtxØ || (inv orig; apply WfCtxU || auto); auto.
 Qed.
+
 
 Lemma get_op_type_wf Σ op A_op B_op:
   wf_sig Σ -> get_op_type Σ op = Some (A_op, B_op) ->
   wf_vtype A_op /\ wf_vtype B_op.
 Proof.
-induction Σ; intros orig gets; constructor.
-+ simpl in gets. discriminate.
-+ simpl in gets. discriminate.
-+ simpl in *. destruct (op == o).
-  - inv gets. inv orig. assumption.
-  - inv orig. apply IHΣ; assumption.
-+ simpl in *. destruct (op == o).
-  - inv gets. inv orig. assumption.
-  - inv orig. apply IHΣ; assumption.
+induction Σ; intros orig gets; constructor; simpl in *; try discriminate.
+all: destruct (op == o); inv orig; try inv gets; auto; apply IHΣ; auto.
 Qed.
+
 
 Lemma join_ctxs_wf Γ Γ' :
   wf_ctx Γ -> wf_ctx Γ' -> wf_ctx (join_ctxs Γ Γ').
 Proof.
-intros wf wf'. induction wf'; simpl; auto.
-apply WfCtxU; auto.
+intros wf wf'. induction wf'; simpl; auto. apply WfCtxU; auto.
 Qed.
+
 
 Lemma join_ctx_tctx_wf Γ Z D:
   wf_ctx Γ -> wf_tctx Z -> wf_ctype D -> wf_ctx (join_ctx_tctx Γ Z D).
 Proof.
-intros wfctx wfZ wfD. induction wfZ; simpl. auto.
+intros wfctx wfZ wfD. induction wfZ; simpl. auto. 
 apply WfCtxU. auto. apply WfTyFun; auto.
 Qed.
